# Saved by TopBraid on Wed Apr 06 16:25:54 CDT 2011
# baseURI: http://mdacc.org/ClinicalLatha
# imports: http://www.isi.edu/~pan/damltime/time-entry.owl
# imports: http://mdacc.org/Organization
# imports: http://mdacc.org/exam
# imports: http://mdacc.org/Archive
# imports: http://swan.mindinformatics.org/ontologies/1.2/collections.owl
# imports: http://mdacc.org/Temporal
# imports: http://www.w3.org/2009/08/skos-reference/skos.rdf
# imports: http://mdacc.org/Sample
# imports: http://xmlns.com/foaf/0.1/
# imports: http://mdacc.org/Drug
# imports: http://www.w3.org/TR/skos-reference/skos-xl.rdf
# imports: http://spinrdf.org/spl

@prefix archive:  <http://mdacc.org/Archive#> .
@prefix clinical:  <http://mdacc.org/Clinical#> .
@prefix collections:  <http://swan.mindinformatics.org/ontologies/1.2/collections/> .
@prefix dc:      <http://purl.org/dc/elements/1.1/> .
@prefix foaf:    <http://xmlns.com/foaf/0.1/> .
@prefix label:   <http://mdacc.org/Label#> .
@prefix mage:    <http://mged.sourceforge.net/ontologies/MGEDOntology.owl#> .
@prefix nco:     <http://www.semanticdesktop.org/ontologies/2007/03/22/nco#> .
@prefix organization:  <http://mdacc.org/Organization#> .
@prefix owl:     <http://www.w3.org/2002/07/owl#> .
@prefix pav:     <http://swan.mindinformatics.org/ontologies/1.2/pav/> .
@prefix rdf:     <http://www.w3.org/1999/02/22-rdf-syntax-ns#> .
@prefix rdfs:    <http://www.w3.org/2000/01/rdf-schema#> .
@prefix sample:  <http://mdacc.org/Sample#> .
@prefix skos:    <http://www.w3.org/2004/02/skos/core#> .
@prefix skos-xl:  <http://www.w3.org/2008/05/skos-xl#> .
@prefix sp:      <http://spinrdf.org/sp#> .
@prefix spin:    <http://spinrdf.org/spin#> .
@prefix tcga:    <http://mdacc.org/TCGAArchive#> .
@prefix temporal:  <http://mdacc.org/Temporal#> .
@prefix time-entry:  <http://www.isi.edu/~pan/damltime/time-entry.owl#> .
@prefix xsd:     <http://www.w3.org/2001/XMLSchema#> .

<http://mdacc.org/ClinicalLatha>
      rdf:type owl:Ontology ;
      owl:imports <http://www.w3.org/2009/08/skos-reference/skos.rdf> , <http://mdacc.org/Archive> , <http://mdacc.org/exam> , <http://www.w3.org/TR/skos-reference/skos-xl.rdf> , <http://mdacc.org/Sample> , foaf: , <http://mdacc.org/Drug> , <http://mdacc.org/Temporal> , <http://swan.mindinformatics.org/ontologies/1.2/collections.owl> , <http://www.isi.edu/~pan/damltime/time-entry.owl> , <http://mdacc.org/Organization> , <http://spinrdf.org/spl> ;
      owl:versionInfo "Created with TopBraid Composer"^^xsd:string .

<http://mdacc.org/ClinicalLatha#AJCCScoringForSarcoma>
      rdf:type owl:Class ;
      rdfs:comment "Scoring system for sarcoma specified by the American Joint Committee on Cancer (AJCC)"^^xsd:string ;
      rdfs:subClassOf <http://mdacc.org/ClinicalLatha#DiseaseScoringSystem> ;
      label:correspondsTo label:AJCCScoreForSarcoma_NCIURI ;
      label:designNote "This concept may demoted to instance"^^xsd:string , "This concept is directly related to the concept of AJCC Score From Sarcoma in NCI Thesaurus"^^xsd:string ;
      dc:creator foaf:JimLomax .

<http://mdacc.org/ClinicalLatha#Absorbance260Nm>
      rdf:type owl:Class ;
      rdfs:comment "The quantity of 260nm light that is not transmitted through a substance or solution."^^xsd:string ;
      rdfs:subClassOf <http://mdacc.org/ClinicalLatha#Quantity> ;
      label:correspondsTo label:Absorbance260NM_NCIURI ;
      label:designNote "This concept is directly related to the Absorbance 260 nm concept in NCI Thesaurus."^^xsd:string ;
      dc:creator foaf:JimLomax .

<http://mdacc.org/ClinicalLatha#Absorbance260To280Nm>
      rdf:type owl:Class ;
      rdfs:comment "There is no corresponding entity in the BioPortal for 260-280 nm absorbance value."^^xsd:string , "This ratio reveals the purity of nucleic acids. The A260A280 ratio is a quality assurance test on an analyte, post-extraction. The ratio will indicate the purity of the analyte."^^xsd:string ;
      rdfs:subClassOf <http://mdacc.org/ClinicalLatha#PurityMeasurment> ;
      dc:creator foaf:JimLomax .

<http://mdacc.org/ClinicalLatha#Absorbance280Nm>
      rdf:type owl:Class ;
      rdfs:comment "The quantity of 280nm light that is not transmitted through a substance or solution."^^xsd:string ;
      rdfs:subClassOf <http://mdacc.org/ClinicalLatha#Quantity> ;
      label:correspondsTo label:Absorbance280NM_NCIURI ;
      label:designNote "This concept is directly related to the Absorbance 260 nm concept in NCI Thesaurus."^^xsd:string ;
      dc:creator foaf:JimLomax .

<http://mdacc.org/ClinicalLatha#AcuteMyeloidLeukemia_Leukemia>
      rdf:type <http://mdacc.org/ClinicalLatha#Leukemia> ;
      rdfs:comment "A clonal expansion of myeloid blasts in the bone marrow, blood or other tissues. The classification of acute myeloid leukemias (AMLs) encompasses four major categories: 1) AML with recurrent genetic abnormalities 2) AML with multilineage dysplasia 3) Therapy-related AML 4) AML not otherwise categorized. The required bone marrow or peripheral blood blast percentage for the diagnosis of AML has been recently reduced from 30% to 20%."^^xsd:string ;
      label:correspondsTo label:AcuteMyeloidLeukemia_NCIURI ;
      label:creator foaf:JimLomax ;
      skos-xl:prefLabel label:AcuteMyeloidLeukemia_LeukemiaDiseaseLabel .

<http://mdacc.org/ClinicalLatha#AdditonalChemotherapyExistentialEvent>
      rdf:type owl:Class ;
      rdfs:comment "This concept represents the existential nature of an additional chemotherapy; the concept is not concerned with spatio-temporal aspects of the event, only that it occurred."^^xsd:string ;
      rdfs:subClassOf <http://mdacc.org/ClinicalLatha#TherapeuticProcedureExistentialEvent> ;
      label:designNote "This existential concept is a product of TCGA's need to capture just the existence of an additional chemotherapy beyond the first"^^xsd:string , "This concept is related to chemotherapy under Therapeutic Procedure"^^xsd:string , "This concept may be domeoted to an instance"^^xsd:string ;
      dc:creator foaf:JimLomax .

<http://mdacc.org/ClinicalLatha#AdditonalDrugTherapyExistentialEvent>
      rdf:type owl:Class ;
      rdfs:comment "This concept represents the existential nature of an additional Drug Therapy; the concept is not concerned with spatio-temporal aspects of the event, only that it occurred."^^xsd:string ;
      rdfs:subClassOf <http://mdacc.org/ClinicalLatha#TherapeuticProcedureExistentialEvent> ;
      label:designNote "This concept is related to Drug Therapy under Therapeutic Procedure"^^xsd:string , "This concept may be demoted to an instance"^^xsd:string , "This existential concept is a product of TCGA's need to capture just the existence of an additional Drug Therapy beyond the first"^^xsd:string ;
      dc:creator foaf:JimLomax .

<http://mdacc.org/ClinicalLatha#AdditonalHormoneTherapyExistentialEvent>
      rdf:type owl:Class ;
      rdfs:comment "This concept represents the existential nature of an additional hormone therapy; the concept is not concerned with spatio-temporal aspects of the event, only that it occurred."^^xsd:string ;
      rdfs:subClassOf <http://mdacc.org/ClinicalLatha#TherapeuticProcedureExistentialEvent> ;
      label:designNote "This concept is related to Hormone Therapy under Therapeutic Procedure"^^xsd:string , "This concept may be demoted to an instance"^^xsd:string , "This existential concept is a product of TCGA's need to capture just the existence of an additional hormone therapy beyond the first"^^xsd:string ;
      dc:creator foaf:JimLomax .

<http://mdacc.org/ClinicalLatha#AdditonalImmunotherapyExistentialEvent>
      rdf:type owl:Class ;
      rdfs:comment "This concept represents the existential nature of an additional immunotherapy; the concept is not concerned with spatio-temporal aspects of the event, only that it occurred."^^xsd:string ;
      rdfs:subClassOf <http://mdacc.org/ClinicalLatha#TherapeuticProcedureExistentialEvent> ;
      label:designNote "This concept is related to immunotherapy under Therapeutic Procedure"^^xsd:string , "This concept may be demoted to an instance"^^xsd:string , "This existential concept is a product of TCGA's need to capture just the existence of an additional immunotherapy beyond the first"^^xsd:string ;
      dc:creator foaf:JimLomax .

<http://mdacc.org/ClinicalLatha#AdditonalRadiationTherapyExistentialEvent>
      rdf:type owl:Class ;
      rdfs:comment "This concept represents the existential nature of an additional radiatio therapy; the concept is not concerned with spatio-temporal aspects of the event, only that it occurred."^^xsd:string ;
      rdfs:subClassOf <http://mdacc.org/ClinicalLatha#TherapeuticProcedureExistentialEvent> ;
      label:designNote "This existential concept is a product of TCGA's need to capture just the existence of an additional radiation therapy beyond the first"^^xsd:string , "This concept is related to the Radiation Therapy under Therapeutic Procedure"^^xsd:string , "This concept may be domeoted to an instance"^^xsd:string ;
      dc:creator foaf:JimLomax .

<http://mdacc.org/ClinicalLatha#Adipocyte>
      rdf:type owl:Class ;
      rdfs:comment "Cells in the body that store fats, usually in the form of triglyceride. White adipocytes are the predominant type and found mostly in the abdominal cavity and subcutaneous tissue. Brown adipocytes are thermogenic cells that can be found in newborns of some species and hibernating mammals"^^xsd:string ;
      rdfs:subClassOf <http://mdacc.org/ClinicalLatha#ConnectiveTissueCell> ;
      label:correspondsTo label:Adipocyte_MESHURI ;
      label:designNote "This concept is extensible."^^xsd:string , "This concept is directly related to the Adipocyte concept in MESH."^^xsd:string , "This concept may have instances of it's own (brown adipocyte and white adipocytes, for example) or may be a superclass for concept refinements."^^xsd:string ;
      dc:creator foaf:JimLomax .

<http://mdacc.org/ClinicalLatha#AdiposeTissue>
      rdf:type owl:Class ;
      rdfs:comment "A specialized form of connective tissue consisting primarily of adipocytes (fat cells), surrounded by a meshwork of collagen fibers"^^xsd:string ;
      rdfs:subClassOf <http://mdacc.org/ClinicalLatha#ConnectiveTissue> ;
      rdfs:subClassOf
              [ rdf:type owl:Restriction ;
                owl:onProperty <http://mdacc.org/ClinicalLatha#composedOf> ;
                owl:someValuesFrom <http://mdacc.org/ClinicalLatha#Adipocyte>
              ] ;
      label:correspondsTo label:AdiposeTissue_NCIURI ;
      label:designNote "This concept is directly related to the Adipose Tissue  concept in NCI Thesaurus."^^xsd:string , "Adispose tissues are composed of adipocytes of the same type."^^xsd:string ;
      dc:creator foaf:JimLomax .

<http://mdacc.org/ClinicalLatha#AdjuvantRegimen>
      rdf:type owl:Class ;
      rdfs:comment "An adjuvant regimen includes any secondary treatment for cancer given after the primary treatment (such as surgery) in order to remove residual microscopic disease"^^xsd:string ;
      rdfs:subClassOf <http://mdacc.org/ClinicalLatha#Regimen> ;
      label:architect foaf:MoSanyang ;
      label:creator foaf:JimLomax ;
      label:developer foaf:PradheepRaju , foaf:DawitGebremichael .

<http://mdacc.org/ClinicalLatha#AliquotExample_Volume>
      rdf:type <http://mdacc.org/ClinicalLatha#Volume> ;
      <http://mdacc.org/ClinicalLatha#units>
              <http://mdacc.org/ClinicalLatha#Milliliter_VolumeUnits> ;
      <http://mdacc.org/ClinicalLatha#value>
              "1.0"^^xsd:string .

<http://mdacc.org/ClinicalLatha#AliquotQuantity>
      rdf:type owl:Class ;
      rdfs:comment "The quantity measurement of an aliquot; perspectives may vary on how quantities are represented, particularly units of measurement."^^xsd:string ;
      rdfs:subClassOf <http://mdacc.org/ClinicalLatha#Quantity> ;
      label:designNote "There is no corresponding concept in BioPortal"^^xsd:string ;
      dc:creator foaf:JimLomax .

<http://mdacc.org/ClinicalLatha#AliquotQuantityUnits>
      rdf:type owl:Class ;
      rdfs:subClassOf <http://mdacc.org/ClinicalLatha#Units> ;
      label:creator foaf:JimLomax .

<http://mdacc.org/ClinicalLatha#AmericanIndian_Race>
      rdf:type <http://mdacc.org/ClinicalLatha#Race> ;
      label:correspondsTo label:AmericanIndian_NCIURI ;
      label:designNote "This concept is directly related to the American Indian Race concept in NCI Thesaurus."^^xsd:string ;
      dc:creator foaf:JimLomax .

<http://mdacc.org/ClinicalLatha#AnalyteExample_Volume>
      rdf:type <http://mdacc.org/ClinicalLatha#Volume> ;
      <http://mdacc.org/ClinicalLatha#units>
              <http://mdacc.org/ClinicalLatha#Milliliter_VolumeUnits> ;
      <http://mdacc.org/ClinicalLatha#value>
              "1.0"^^xsd:string .

<http://mdacc.org/ClinicalLatha#AnaplasiaFinding>
      rdf:type owl:Class ;
      rdfs:comment "Anaplasia refers to a reversion of differentiation (dediiferentiation or a reversal in maturity) in cells and is characteristic of malignant neoplasms (tumors)."^^xsd:string ;
      rdfs:subClassOf <http://mdacc.org/ClinicalLatha#Finding> ;
      rdfs:subClassOf
              [ rdf:type owl:Restriction ;
                owl:onProperty skos-xl:prefLabel ;
                owl:someValuesFrom label:AnaplasiaLabel
              ] ;
      label:correspondsTo label:Anaplasia_MESHURI ;
      label:designNote "This concept is directly related to the Anaplasia concept in MESH."^^xsd:string ;
      dc:creator foaf:JimLomax .

<http://mdacc.org/ClinicalLatha#AnaplasticAstrocytoma>
      rdf:type owl:Class ;
      rdfs:comment "A diffusely infiltrating, WHO grade III astrocytoma with focal or dispersed anaplasia, and a marked proliferative potential. It may arise from a low-grade astrocytoma, but it can also be diagnosed at first biopsy, without indication of a less malignant precursor lesion. It has an intrinsic tendency for malignant progression to glioblastoma."^^xsd:string ;
      rdfs:subClassOf <http://mdacc.org/ClinicalLatha#Astrocytoma> ;
      rdfs:subClassOf
              [ rdf:type owl:Restriction ;
                owl:onProperty <http://mdacc.org/ClinicalLatha#anaplasia> ;
                owl:someValuesFrom <http://mdacc.org/ClinicalLatha#AnaplasiaFinding>
              ] ;
      label:correspondsTo label:AnaplasticAstrocytoma_SNOMEDURI ;
      label:designNote "This concept is extensible."^^xsd:string , "This concept is directly related to the Anaplastic Astrocytoma  concept in SNOMED."^^xsd:string , "This concept may have instances of it's own or may be a superclass for concept refinements."^^xsd:string ;
      dc:creator foaf:JimLomax .

<http://mdacc.org/ClinicalLatha#AnatomicSite>
      rdf:type owl:Class ;
      rdfs:comment "Body tissue, region, surface, cavity, fluid, organ, or collection of organs."^^xsd:string ;
      rdfs:subClassOf skos:Concept , <http://mdacc.org/ClinicalLatha#ClinicalPackage> ;
      rdfs:subClassOf
              [ rdf:type owl:Restriction ;
                owl:onProperty skos-xl:prefLabel ;
                owl:someValuesFrom label:AnatomicSiteLabel
              ] ;
      label:correspondsTo label:AnatomicSite_NCIURI ;
      label:designNote "This concept is extensible."^^xsd:string , "This concept is directly related to the Anatomic Site concept in NCI Thesaurus."^^xsd:string , "This concept may have instances of it's own or may be a superclass for concept refinements."^^xsd:string ;
      dc:creator foaf:JimLomax .

<http://mdacc.org/ClinicalLatha#ArachnoidMatter_LeptomeningesMeninges>
      rdf:type <http://mdacc.org/ClinicalLatha#Leptomeninges> , <http://mdacc.org/ClinicalLatha#Meninges> ;
      label:correspondsTo label:CerebralArachnoidMatter_NCIURI ;
      label:creator foaf:JimLomax .

<http://mdacc.org/ClinicalLatha#Ashkenazi_JewishOrigin>
      rdf:type <http://mdacc.org/ClinicalLatha#JewishOrigin> ;
      label:correspondsTo label:Ashkenazi_NCIURI ;
      label:creator foaf:JimLomax ;
      label:designNote "The concept directly corresponds to the Ashkenazi Jew concept in NCI Thesaurus."^^xsd:string ;
      skos-xl:prefLabel label:Ashkenazi_JewishOriginLabel .

<http://mdacc.org/ClinicalLatha#Asian_Race>
      rdf:type <http://mdacc.org/ClinicalLatha#Race> ;
      label:correspondsTo label:Asian_NCIURI ;
      label:designNote "This concept is directly related to the Asian  Race concept in NCI Thesaurus."^^xsd:string ;
      dc:creator foaf:JimLomax .

<http://mdacc.org/ClinicalLatha#Astrocyte>
      rdf:type owl:Class ;
      rdfs:comment "The largest and most numerous neuroglial cells in the brain and spinal cord. Astrocytes are irregularly shaped with many long processes, including those with \"end feet\" which form the glial (limiting) membrane and directly and indirectly contribute to the blood brain barrier. They regulate the extracellular ionic and chemical environment, and \"reactive astrocytes\" (along with microglia) respond to injury. Astrocytes have high- affinity transmitter uptake systems, voltage-dependent and transmitter-gated ion channels, and can release transmitter, but their role in signaling (as in many other functions) is not well understood"^^xsd:string ;
      rdfs:subClassOf <http://mdacc.org/ClinicalLatha#GlialCell> ;
      label:correspondsTo label:Astrocyte_NCIURI ;
      label:designNote "This concept is extensible."^^xsd:string , "This concept is directly related to the Astrocyte concept in NCI Thesaurus"^^xsd:string , "This concept may have instances of it's own or may be a superclass for concept refinements."^^xsd:string ;
      dc:creator foaf:JimLomax .

<http://mdacc.org/ClinicalLatha#Astrocytoma>
      rdf:type owl:Class ;
      rdfs:comment "A tumor of the brain or spinal cord showing astrocytic differentiation. It includes the following clinicopathological entities: pilocytic astrocytoma, diffuse astrocytoma, anaplastic astrocytoma, pleomorphic xanthoastrocytoma, and subependymal giant cell astrocytoma."^^xsd:string ;
      rdfs:subClassOf <http://mdacc.org/ClinicalLatha#Glioma> ;
      rdfs:subClassOf
              [ rdf:type owl:Restriction ;
                owl:onProperty <http://mdacc.org/ClinicalLatha#cellularDifferentiation> ;
                owl:someValuesFrom <http://mdacc.org/ClinicalLatha#Astrocyte>
              ] ;
      label:correspondsTo label:Astrocytoma_NCIURI ;
      label:designNote "This concept is extensible."^^xsd:string , "This concept may have instances of it's own or may be a superclass for concept refinements."^^xsd:string , "This concept is directly related to the Astrocytoma  concept in NCI Thesaurus."^^xsd:string ;
      dc:creator foaf:JimLomax .

<http://mdacc.org/ClinicalLatha#BCell>
      rdf:type owl:Class ;
      rdfs:comment "The principal functions of B cells are to make antibodies against antigens, perform the role of antigen-presenting cells (APCs) and eventually develop into memory B cells after activation by antigen interaction. B cells are an essential component of the adaptive immune system."^^xsd:string ;
      rdfs:subClassOf <http://mdacc.org/ClinicalLatha#Lymphocyte> ;
      label:correspondsTo label:BCell_MESHURI ;
      label:designNote "This concept is extensible."^^xsd:string , "This concept is directly related to the B Cell concept in MESH"^^xsd:string , "This concept may have instances of it's own or may be a superclass for concept refinements."^^xsd:string ;
      dc:creator foaf:JimLomax .

<http://mdacc.org/ClinicalLatha#BarcodeImage1_BarcodeImage>
      rdf:type archive:BarcodeImage ;
      dc:identifier "123456"^^xsd:string .

<http://mdacc.org/ClinicalLatha#Batch1UploadComplete>
      rdf:type time-entry:Instant ;
      time-entry:inCalendarClockDataType
              "2010-11-02T00:23:08.7"^^xsd:dateTime .

<http://mdacc.org/ClinicalLatha#BioMaterial>
      rdf:type owl:Class ;
      rdfs:comment "TCGA specific representation of BioMaterial that incorporates any material that is biological in nature."^^xsd:string ;
      rdfs:subClassOf skos:Concept , <http://mdacc.org/ClinicalLatha#ClinicalPackage> ;
      rdfs:subClassOf
              [ rdf:type owl:Restriction ;
                owl:onProperty skos-xl:prefLabel ;
                owl:someValuesFrom label:BioMaterialLabel
              ] ;
      label:correspondsTo label:BiologicallyDerivedMaterial_NCIURI ;
      label:creator foaf:JimLomax ;
      label:designNote "This concept is extensible."^^xsd:string , "This concept is directly related to the Biologically Derived Material concept in NCI Thesaurus."^^xsd:string , "The concepts in BioMaterial actually belong in a molecular namespace"^^xsd:string , "This concept may have instances of it's own or may be a superclass for concept refinements."^^xsd:string ;
      label:domainQuestion
              "Should we put this concept hierarchy in a molecular or tissue based package?  Yes"^^xsd:string .

<http://mdacc.org/ClinicalLatha#Biomarker>
      rdf:type owl:Class ;
      rdfs:comment "A variation in cellular or biochemical components or processes, structures, or functions that is objectively measurable in a biological system and that characterizes normal biologic processes, pathogenic processes, an organism's state of health or disease, likelihood of developing a disease, prognosis, or response to a particular therapeutic intervention."^^xsd:string ;
      rdfs:subClassOf <http://mdacc.org/ClinicalLatha#Indicator> ;
      label:correspondsTo label:Biomarker_NCIURI ;
      label:designNote "This concept is extensible."^^xsd:string , "This concept is directly related to the Biomarker concept in NCI Thesaurus."^^xsd:string , "This concept may have instances of it's own or may be a superclass for concept refinements."^^xsd:string ;
      dc:creator foaf:JimLomax .

<http://mdacc.org/ClinicalLatha#BiomarkerIndicator>
      rdf:type owl:Class ;
      rdfs:subClassOf <http://mdacc.org/ClinicalLatha#Indicator> ;
      owl:equivalentClass <http://mdacc.org/ClinicalLatha#Biomarker> .

<http://mdacc.org/ClinicalLatha#Biospecimen>
      rdf:type owl:Class ;
      rdfs:comment "Any material sample taken from a biological entity for testing, diagnostic, propagation, treatment or research purposes, including a sample obtained from a living organism or taken from the biological object after halting of all its life functions. Biospecimen can contain one or more components including but not limited to cellular molecules, cells, tissues, organs, body fluids, embryos, and body excretory products."^^xsd:string ;
      rdfs:subClassOf <http://mdacc.org/ClinicalLatha#ClinicalPackage> ;
      label:correspondsTo label:Biospecimen_NCIURI ;
      label:designNote "This concept is extensible."^^xsd:string , "This concept is directly related to the Biospecimen concept in NCI Thesaurus."^^xsd:string , "This concept may have instances of it's own or may be a superclass for concept refinements."^^xsd:string ;
      dc:creator foaf:JimLomax .

<http://mdacc.org/ClinicalLatha#BirthExistentialEvent>
      rdf:type owl:Class ;
      rdfs:comment "This concept represents the existential nature of a birth; the concept is not concerned with spatio-temporal aspects of the event, only that it occurred."^^xsd:string ;
      rdfs:subClassOf <http://mdacc.org/ClinicalLatha#ExistentialEvent> ;
      label:correspondsTo label:Birth_NCIURI ;
      label:designNote "This existential concept is a product of TCGA's need to capture just the existence of a birth; this is due in part to the fact that specific birth details such as date and place may not be available (or necessary)."^^xsd:string , "This concept may be domeoted to an instance"^^xsd:string , "This concept is directly related to the Birth concept in NCI Thesaurus."^^xsd:string ;
      dc:creator foaf:JimLomax .

<http://mdacc.org/ClinicalLatha#Black_Race>
      rdf:type <http://mdacc.org/ClinicalLatha#Race> ;
      label:correspondsTo label:BlackRace_NCIURI ;
      label:designNote "This concept is directly related to the Black Race concept in NCI Thesaurus."^^xsd:string ;
      dc:creator foaf:JimLomax .

<http://mdacc.org/ClinicalLatha#BladderAnatomicSite>
      rdf:type owl:Class ;
      rdfs:comment "The distensible sac-like organ that functions as a reservoir of urine, collecting from the kidneys and eliminating via the urethra."^^xsd:string ;
      rdfs:subClassOf <http://mdacc.org/ClinicalLatha#AnatomicSite> ;
      label:architect foaf:MoSanyang ;
      label:correspondsTo label:Bladder_NCIURI ;
      label:designNote "This concept is directly related to the Bladder concept in NCI Thesaurus."^^xsd:string , "This concept is extensible; more specific anatomic location within the bladder."^^xsd:string , "This concept may have specific instances."^^xsd:string ;
      label:developer foaf:PradheepRaju , foaf:DawitGebremichael ;
      dc:creator foaf:JimLomax .

<http://mdacc.org/ClinicalLatha#BladderCancer>
      rdf:type owl:Class ;
      rdfs:subClassOf <http://mdacc.org/ClinicalLatha#Cancer> ;
      rdfs:subClassOf
              [ rdf:type owl:Restriction ;
                owl:onProperty <http://mdacc.org/ClinicalLatha#anatomicLocation> ;
                owl:someValuesFrom <http://mdacc.org/ClinicalLatha#BladderAnatomicSite>
              ] ;
      label:correspondsTo label:BladderCancer_MEDRAURI ;
      label:creator foaf:JimLomax .

<http://mdacc.org/ClinicalLatha#BladderCancerTumorStage>
      rdf:type owl:Class ;
      rdfs:subClassOf <http://mdacc.org/ClinicalLatha#TumorStage> .

<http://mdacc.org/ClinicalLatha#BladderCancer_BladderCancer>
      rdf:type <http://mdacc.org/ClinicalLatha#BladderCancer> ;
      rdf:type
              [ rdf:type owl:Restriction ;
                owl:onProperty <http://mdacc.org/ClinicalLatha#manifests> ;
                owl:someValuesFrom <http://mdacc.org/ClinicalLatha#BladderTumor>
              ] ;
      <http://mdacc.org/ClinicalLatha#anatomicLocation>
              <http://mdacc.org/ClinicalLatha#Bladder_BladderAnatomicSite> ;
      <http://mdacc.org/ClinicalLatha#manifests>
              <http://mdacc.org/ClinicalLatha#BladderTumor_BladderTumor> ;
      label:correspondsTo label:BladderCancer_MEDRAURI ;
      label:creator foaf:JimLomax ;
      label:designNote "This instance of Bladder Cancer represents a diagnosis of Bladder Cancer with no further details."^^xsd:string ;
      skos-xl:prefLabel label:BladderCancer_BladderCancerDiseaseLabel .

<http://mdacc.org/ClinicalLatha#BladderTumor>
      rdf:type owl:Class ;
      rdfs:comment "Tumor anatomically located within the bladder"^^xsd:string ;
      rdfs:subClassOf <http://mdacc.org/ClinicalLatha#TumorType> ;
      rdfs:subClassOf
              [ rdf:type owl:Restriction ;
                owl:onProperty <http://mdacc.org/ClinicalLatha#anatomicLocation> ;
                owl:someValuesFrom <http://mdacc.org/ClinicalLatha#BladderAnatomicSite>
              ] ;
      label:designNote "This concept is extensible."^^xsd:string , "This concept may have instances of it's own or may be a superclass for concept refinements."^^xsd:string ;
      dc:creator foaf:JimLomax .

<http://mdacc.org/ClinicalLatha#BladderTumor_BladderTumor>
      rdf:type <http://mdacc.org/ClinicalLatha#BladderTumor> ;
      <http://mdacc.org/ClinicalLatha#anatomicLocation>
              <http://mdacc.org/ClinicalLatha#Bladder_BladderAnatomicSite> ;
      <http://mdacc.org/ClinicalLatha#manifestedBy>
              <http://mdacc.org/ClinicalLatha#BladderCancer_BladderCancer> ;
      label:creator foaf:JimLomax ;
      label:designNote "This instance of Bladder Tumor is a general representation of a Bladder Tumor with no further details."^^xsd:string .

<http://mdacc.org/ClinicalLatha#BladderUrothelialCarcinoma_BladderTumor>
      rdf:type <http://mdacc.org/ClinicalLatha#BladderTumor> ;
      rdfs:comment "An invasive or non-invasive papillary transitional cell carcinoma of the urinary bladde"^^xsd:string ;
      <http://mdacc.org/ClinicalLatha#anatomicLocation>
              <http://mdacc.org/ClinicalLatha#Bladder_BladderAnatomicSite> ;
      <http://mdacc.org/ClinicalLatha#manifestedBy>
              <http://mdacc.org/ClinicalLatha#BladderCancer_BladderCancer> ;
      label:correspondsTo label:BladderUrothelialCancer_NCIURI ;
      label:creator foaf:JimLomax ;
      label:designNote "This instance of Bladder Urothelial Carcinoma represents a more specific diagnosis of Bladder Cancer "^^xsd:string ;
      skos-xl:prefLabel label:BladderUrothelialCarcinoma_BladderTumorLabel .

<http://mdacc.org/ClinicalLatha#BladderUrothelialNonPapillaryCarcinoma_BladderTumor>
      rdf:type <http://mdacc.org/ClinicalLatha#BladderTumor> ;
      rdfs:comment "An invasive or non-invasive non papillary transitional cell carcinoma of the urinary bladder"^^xsd:string ;
      <http://mdacc.org/ClinicalLatha#anatomicLocation>
              <http://mdacc.org/ClinicalLatha#Bladder_BladderAnatomicSite> ;
      <http://mdacc.org/ClinicalLatha#manifestedBy>
              <http://mdacc.org/ClinicalLatha#BladderCancer_BladderCancer> ;
      label:creator foaf:JimLomax ;
      label:designNote "This instance of Bladder Urothelial Non Papillary Carcinoma represents a more specific diagnosis of Bladder Tumor "^^xsd:string ;
      skos-xl:prefLabel label:BladderUrothelialNonPapillaryCancer_BladderTumorLabel .

<http://mdacc.org/ClinicalLatha#BladderUrothelialPapillaryCarcinoma_BladderTumor>
      rdf:type <http://mdacc.org/ClinicalLatha#BladderTumor> ;
      rdfs:comment "An invasive or non-invasive papillary transitional cell carcinoma of the urinary bladder"^^xsd:string ;
      <http://mdacc.org/ClinicalLatha#anatomicLocation>
              <http://mdacc.org/ClinicalLatha#Bladder_BladderAnatomicSite> ;
      <http://mdacc.org/ClinicalLatha#manifestedBy>
              <http://mdacc.org/ClinicalLatha#BladderCancer_BladderCancer> ;
      label:correspondsTo label:BladderUrothelialPapillaryCancer_NCIURI ;
      label:creator foaf:JimLomax ;
      label:designNote "This instance of Bladder Urothelial Papillary Carcinoma represents a more specific type of Bladder Tumor "^^xsd:string ;
      skos-xl:prefLabel label:BladderUrothelialPapillaryCarcinoma_BladderTumorLabel .

<http://mdacc.org/ClinicalLatha#Bladder_BladderAnatomicSite>
      rdf:type <http://mdacc.org/ClinicalLatha#BladderAnatomicSite> ;
      label:correspondsTo label:Bladder_NCIURI ;
      label:creator foaf:JimLomax ;
      skos-xl:prefLabel label:Bladder_AnatomicSiteLabel .

<http://mdacc.org/ClinicalLatha#Bottom_Side>
      rdf:type <http://mdacc.org/ClinicalLatha#Side> ;
      label:creator foaf:JimLomax ;
      skos-xl:prefLabel label:Bottom_SideLabel .

<http://mdacc.org/ClinicalLatha#BrainAnatomicSite>
      rdf:type owl:Class ;
      rdfs:comment "An organ composed of grey and white matter containing billions of neurons that is the center for intelligence and reasoning. It is protected by the bony cranium."^^xsd:string ;
      rdfs:subClassOf <http://mdacc.org/ClinicalLatha#AnatomicSite> ;
      label:correspondsTo label:Brain_NCIURI ;
      label:designNote "This concept is directly related to the Brain concept in NCI Thesaurus."^^xsd:string , "This concept may have specific instances; (left brain, right brain) as an example."^^xsd:string , "This concept is extensible; more specific anatomic location within the brain."^^xsd:string ;
      dc:creator foaf:JimLomax .

<http://mdacc.org/ClinicalLatha#BrainCancer>
      rdf:type owl:Class ;
      rdfs:subClassOf <http://mdacc.org/ClinicalLatha#Cancer> ;
      rdfs:subClassOf
              [ rdf:type owl:Restriction ;
                owl:onProperty <http://mdacc.org/ClinicalLatha#anatomicLocation> ;
                owl:someValuesFrom <http://mdacc.org/ClinicalLatha#BrainAnatomicSite>
              ] ;
      <http://mdacc.org/ClinicalLatha#manifests>
              <http://mdacc.org/ClinicalLatha#GlioblastomaMultiforme_Glioblastoma> ;
      label:correspondsTo label:BrainCancer_NCIURI ;
      dc:creator foaf:JimLomax .

<http://mdacc.org/ClinicalLatha#BrainCancer_BrainCancer>
      rdf:type <http://mdacc.org/ClinicalLatha#BrainCancer> ;
      <http://mdacc.org/ClinicalLatha#anatomicLocation>
              <http://mdacc.org/ClinicalLatha#Brain_BrainAnatomicSite> ;
      label:correspondsTo label:BrainCancer_NCIURI ;
      label:creator foaf:JimLomax ;
      label:designNote "This instance of Brain Cancer represents a diagnosis of Brain Cancer with no further details."^^xsd:string .

<http://mdacc.org/ClinicalLatha#BrainLowerGradeGlioma_Glioma>
      rdf:type <http://mdacc.org/ClinicalLatha#Glioma> ;
      <http://mdacc.org/ClinicalLatha#anatomicLocation>
              <http://mdacc.org/ClinicalLatha#Brain_BrainAnatomicSite> ;
      <http://mdacc.org/ClinicalLatha#manifestedBy>
              <http://mdacc.org/ClinicalLatha#BrainCancer_BrainCancer> ;
      label:correspondsTo label:BrainLowGradeGlioma_SNOMEDURI ;
      label:creator foaf:JimLomax ;
      skos-xl:prefLabel label:BrainLowGradeGlioma_BrainTumorLabel .

<http://mdacc.org/ClinicalLatha#BrainMembrane>
      rdf:type owl:Class ;
      rdfs:subClassOf <http://mdacc.org/ClinicalLatha#Membrane> ;
      rdfs:subClassOf
              [ rdf:type owl:Restriction ;
                owl:onProperty <http://mdacc.org/ClinicalLatha#anatomicLocation> ;
                owl:someValuesFrom <http://mdacc.org/ClinicalLatha#BrainAnatomicSite>
              ] ;
      label:correspondsTo label:BrainMembrane_NCIURI ;
      label:designNote "This concept is directly related to the Brain Membrane concept in NCI Thesaurus."^^xsd:string , "This concept is extensible; there are different types of brain membranes each of which will have different properties."^^xsd:string , "This concept may have instances of it's own or may be a superclass for concept refinements."^^xsd:string ;
      dc:creator foaf:JimLomax .

<http://mdacc.org/ClinicalLatha#Brain_BrainAnatomicSite>
      rdf:type <http://mdacc.org/ClinicalLatha#BrainAnatomicSite> ;
      label:correspondsTo label:Brain_NCIURI ;
      label:creator foaf:JimLomax ;
      skos-xl:prefLabel label:Brain_AnatomicSiteLabel .

<http://mdacc.org/ClinicalLatha#BreastAnatomicSite>
      rdf:type owl:Class ;
      rdfs:subClassOf <http://mdacc.org/ClinicalLatha#AnatomicSite> ;
      label:designNote "This concept is extensible; more specific anatomic location within the breast."^^xsd:string , "This concept may have specific instances."^^xsd:string ;
      dc:creator foaf:JimLomax .

<http://mdacc.org/ClinicalLatha#BreastCancer>
      rdf:type owl:Class ;
      rdfs:subClassOf <http://mdacc.org/ClinicalLatha#Cancer> ;
      rdfs:subClassOf
              [ rdf:type owl:Restriction ;
                owl:onProperty <http://mdacc.org/ClinicalLatha#anatomicLocation> ;
                owl:someValuesFrom <http://mdacc.org/ClinicalLatha#BreastAnatomicSite>
              ] ;
      label:correspondsTo label:BreastCancer_NCIURI ;
      label:creator foaf:JimLomax .

<http://mdacc.org/ClinicalLatha#BreastCancer_BreastCancer>
      rdf:type <http://mdacc.org/ClinicalLatha#BreastCancer> ;
      <http://mdacc.org/ClinicalLatha#anatomicLocation>
              <http://mdacc.org/ClinicalLatha#Breast_BreastAnatomicSite> ;
      label:creator foaf:JimLomax ;
      skos-xl:prefLabel label:BreastCancer_BreastCancerDiseaseLabel .

<http://mdacc.org/ClinicalLatha#BreastInvasiveCarcinoma_BreastTumor>
      rdf:type <http://mdacc.org/ClinicalLatha#BreastTumor> ;
      <http://mdacc.org/ClinicalLatha#anatomicLocation>
              <http://mdacc.org/ClinicalLatha#Breast_BreastAnatomicSite> ;
      <http://mdacc.org/ClinicalLatha#manifestedBy>
              <http://mdacc.org/ClinicalLatha#BreastCancer_BreastCancer> ;
      label:creator foaf:JimLomax ;
      skos-xl:prefLabel label:BreastInvasiveCarcinoma_BreastTumorLabel .

<http://mdacc.org/ClinicalLatha#BreastTumor>
      rdf:type owl:Class ;
      rdfs:comment "Tumor anatomically located within the breast"^^xsd:string ;
      rdfs:subClassOf <http://mdacc.org/ClinicalLatha#TumorType> ;
      rdfs:subClassOf
              [ rdf:type owl:Restriction ;
                owl:onProperty <http://mdacc.org/ClinicalLatha#anatomicLocation> ;
                owl:someValuesFrom <http://mdacc.org/ClinicalLatha#BreastAnatomicSite>
              ] ;
      <http://mdacc.org/ClinicalLatha#manifestedBy>
              <http://mdacc.org/ClinicalLatha#BreastCancer_BreastCancer> ;
      label:designNote "This concept is extensible."^^xsd:string , "This concept may have instances of it's own or may be a superclass for concept refinements."^^xsd:string ;
      dc:creator foaf:JimLomax .

<http://mdacc.org/ClinicalLatha#Breast_BreastAnatomicSite>
      rdf:type <http://mdacc.org/ClinicalLatha#BreastAnatomicSite> ;
      rdfs:comment "LR: skos: prefLabel is incorrect"^^xsd:string ;
      label:creator foaf:JimLomax ;
      skos-xl:prefLabel label:Brain_AnatomicSiteLabel .

<http://mdacc.org/ClinicalLatha#Brown_Adipocyte>
      rdf:type <http://mdacc.org/ClinicalLatha#Adipocyte> ;
      rdfs:comment "Fat cells with dark coloration due to the densely packed Mitochondria. They contain numerous small lipid droplets or vacuoles. Their stored lipids can be converted directly to energy as heat by the mitochondria."^^xsd:string ;
      label:correspondsTo label:BrownAdipocyte_MESHURI ;
      label:creator foaf:JimLomax ;
      label:designNote "This instance directly corresponds to the Brown Apidocyte concept in MESH."^^xsd:string .

<http://mdacc.org/ClinicalLatha#BuccalCell>
      rdf:type owl:Class ;
      rdfs:comment "A Buccal cell is a cell from the epithelial layer of the mouth, most notable from the cheek."^^xsd:string ;
      rdfs:subClassOf <http://mdacc.org/ClinicalLatha#EpithelialCell> ;
      rdfs:subClassOf
              [ rdf:type owl:Restriction ;
                owl:onProperty <http://mdacc.org/ClinicalLatha#anatomicLocation> ;
                owl:someValuesFrom <http://mdacc.org/ClinicalLatha#OralCavityAnatomicSite>
              ] ;
      label:correspondsTo label:BuccalCell_PMAURI ;
      label:designNote "This concept is directly related to the Buccal Cell concept in PMA"^^xsd:string , "This concept may have instances of it's own or may be a superclass for concept refinements."^^xsd:string ;
      dc:creator foaf:JimLomax .

<http://mdacc.org/ClinicalLatha#BuccalMucosa>
      rdf:type owl:Class ;
      rdfs:comment "The mucosal membranes located on the inside of the cheek, in the oral cavity."^^xsd:string ;
      rdfs:subClassOf <http://mdacc.org/ClinicalLatha#Mucosa> ;
      label:correspondsTo label:BuccalMucosa_NCIURI ;
      label:designNote "We cannot find reason to further refine this concept."^^xsd:string , "This concept is directly related to the Buccal Mucosa  concept in NCI Thesaurus."^^xsd:string ;
      label:domainQuestion
              "Are there specific instances of buccal mucosa or is buccal mucosa an instance of mucosa"^^xsd:string ;
      dc:creator foaf:JimLomax .

<http://mdacc.org/ClinicalLatha#CalendarClockDescription_29OfMonth>
      rdf:type time-entry:CalendarClockDescription ;
      time-entry:day "---29"^^xsd:gDay ;
      time-entry:dayOfWeekField
              "0"^^xsd:nonNegativeInteger .

<http://mdacc.org/ClinicalLatha#Cancer>
      rdf:type owl:Class ;
      rdfs:comment "The concept of Cancer. This could to reference a taxonomy of cancer types however, the question of which taxonomy is currently under discussion."^^xsd:string ;
      rdfs:subClassOf <http://mdacc.org/ClinicalLatha#Disease> ;
      rdfs:subClassOf
              [ rdf:type owl:Restriction ;
                owl:onProperty <http://mdacc.org/ClinicalLatha#manifests> ;
                owl:someValuesFrom <http://mdacc.org/ClinicalLatha#TumorType>
              ] ;
      label:correspondsTo label:Cancer_SNOMEDURI ;
      label:designNote "This concept is extensible."^^xsd:string , "This concept is directly related to the Cancer concept in SNOMED."^^xsd:string , "This concept may have instances of it's own or may be a superclass for concept refinements."^^xsd:string ;
      dc:creator foaf:JimLomax .

<http://mdacc.org/ClinicalLatha#CancerProgressionDiagnosis>
      rdf:type owl:Class ;
      rdfs:subClassOf <http://mdacc.org/ClinicalLatha#Diagnosis> ;
      rdfs:subClassOf
              [ rdf:type owl:Restriction ;
                owl:onProperty skos-xl:prefLabel ;
                owl:someValuesFrom label:CancerProgressionDiagnosisLabel
              ] ;
      label:creator foaf:JimLomax ;
      label:designNote "This concept is extensible."^^xsd:string , "This concept may have instances of it's own or may be a superclass for concept refinements."^^xsd:string ;
      label:domainQuestion
              "Is there a concept in Bio Portal corresponding to Cancer Progression Diagnonis. If so, we need the instances as well, these will be referenced within the ontology."^^xsd:string .

<http://mdacc.org/ClinicalLatha#CancerProgressionDiagnosis1_PatientEvent>
      rdf:type <http://mdacc.org/ClinicalLatha#CancerProgressionDiagnosisPatientEvent> ;
      <http://mdacc.org/ClinicalLatha#diagnosis>
              <http://mdacc.org/ClinicalLatha#GeneralCancerProgression_CancerProgressionDiagnosis> ;
      time-entry:inCalendarClockDataType
              "2010-05-29T20:15:20.198"^^xsd:dateTime .

<http://mdacc.org/ClinicalLatha#CancerProgressionDiagnosisPatientEvent>
      rdf:type owl:Class ;
      rdfs:comment "Diagnosis: cancer worsening over time."^^xsd:string ;
      rdfs:subClassOf <http://mdacc.org/ClinicalLatha#DiagnosisPatientEvent> ;
      dc:creator foaf:JimLomax .

<http://mdacc.org/ClinicalLatha#CancerProgressionIndicator>
      rdf:type owl:Class ;
      rdfs:comment "Any indicator of cancer progression"^^xsd:string ;
      rdfs:subClassOf <http://mdacc.org/ClinicalLatha#Indicator> ;
      rdfs:subClassOf
              [ rdf:type owl:Restriction ;
                owl:onProperty <http://mdacc.org/ClinicalLatha#indicates> ;
                owl:someValuesFrom <http://mdacc.org/ClinicalLatha#CancerProgressionDiagnosisPatientEvent>
              ] ;
      dc:creator foaf:JimLomax .

<http://mdacc.org/ClinicalLatha#Carcinoma>
      rdf:type owl:Class ;
      rdfs:comment "A malignant tumor arising from epithelial cells"^^xsd:string ;
      rdfs:subClassOf <http://mdacc.org/ClinicalLatha#MalignantTumor> ;
      rdfs:subClassOf
              [ rdf:type owl:Restriction ;
                owl:onProperty <http://mdacc.org/ClinicalLatha#cellularDifferentiation> ;
                owl:someValuesFrom <http://mdacc.org/ClinicalLatha#EpithelialCell>
              ] ;
      label:correspondsTo label:Carcinoma_NCIURI ;
      label:designNote "This concept is extensible."^^xsd:string , "This concept is directly related to the Carcinoma concept in NCI Thesaurus."^^xsd:string , "This concept may have instances of it's own or may be a superclass for concept refinements."^^xsd:string .

<http://mdacc.org/ClinicalLatha#Cell>
      rdf:type owl:Class ;
      rdfs:comment "This is an alternative perspective of a Cell; a class that allows further extension (and variation) of Cell outside of a TCGA perspective. "^^xsd:string ;
      rdfs:subClassOf <http://mdacc.org/ClinicalLatha#BioMaterial> ;
      label:correspondsTo label:Cell_NCIURI ;
      label:designNote "This concept is extensible."^^xsd:string , "This concept may have instances of it's own or may be a superclass for concept refinements."^^xsd:string , "This concept is directly related to the Cell concept in NCI Thesaurus."^^xsd:string ;
      dc:creator foaf:JimLomax .

<http://mdacc.org/ClinicalLatha#Cell1_Cell>
      rdf:type <http://mdacc.org/ClinicalLatha#Cell> .

<http://mdacc.org/ClinicalLatha#CellLysate>
      rdf:type owl:Class ;
      rdfs:comment "This is an alternative perspective of a CellLysate."^^xsd:string ;
      rdfs:subClassOf <http://mdacc.org/ClinicalLatha#BioMaterial> ;
      label:correspondsTo label:Lysate_NCIURI ;
      label:designNote "This concept is extensible."^^xsd:string , "This concept may have instances of it's own or may be a superclass for concept refinements."^^xsd:string , "This concept is directly related to the Cell concept in NCI Thesaurus."^^xsd:string .

<http://mdacc.org/ClinicalLatha#Centimeter_LengthUnits>
      rdf:type <http://mdacc.org/ClinicalLatha#LengthUnits> ;
      skos-xl:prefLabel label:Centimeter_UnitsLabel .

<http://mdacc.org/ClinicalLatha#CervicalCancer>
      rdf:type owl:Class ;
      rdfs:subClassOf <http://mdacc.org/ClinicalLatha#Cancer> ;
      rdfs:subClassOf
              [ rdf:type owl:Restriction ;
                owl:onProperty <http://mdacc.org/ClinicalLatha#anatomicLocation> ;
                owl:someValuesFrom <http://mdacc.org/ClinicalLatha#CervixAnatomicSite>
              ] ;
      label:correspondsTo label:CervicalCancer_NCIURI ;
      label:designNote "This concept is directly related to the Cervical Cancer concept in NCI."^^xsd:string ;
      dc:creator foaf:JimLomax .

<http://mdacc.org/ClinicalLatha#CervicalCancer_CervicalCancer>
      rdf:type <http://mdacc.org/ClinicalLatha#CervicalCancer> ;
      <http://mdacc.org/ClinicalLatha#anatomicLocation>
              <http://mdacc.org/ClinicalLatha#Cervix_CervixAnatomicSite> ;
      label:creator foaf:JimLomax ;
      skos-xl:prefLabel label:CervicalCancer_CervicalCancerDiseaseLabel .

<http://mdacc.org/ClinicalLatha#CervicalSquamousCellCarcinoma_CervicalTumor>
      rdf:type <http://mdacc.org/ClinicalLatha#CervicalTumor> ;
      <http://mdacc.org/ClinicalLatha#anatomicLocation>
              <http://mdacc.org/ClinicalLatha#Cervix_CervixAnatomicSite> ;
      <http://mdacc.org/ClinicalLatha#manifestedBy>
              <http://mdacc.org/ClinicalLatha#CervicalCancer_CervicalCancer> ;
      label:creator foaf:JimLomax ;
      skos-xl:prefLabel label:CervicalSquamousCellCarcinoma_CervicalTumorLabel .

<http://mdacc.org/ClinicalLatha#CervicalTumor>
      rdf:type owl:Class ;
      rdfs:comment "Tumor anatomically located within the cervix"^^xsd:string ;
      rdfs:subClassOf <http://mdacc.org/ClinicalLatha#TumorType> ;
      rdfs:subClassOf
              [ rdf:type owl:Restriction ;
                owl:onProperty <http://mdacc.org/ClinicalLatha#anatomicLocation> ;
                owl:someValuesFrom <http://mdacc.org/ClinicalLatha#CervixAnatomicSite>
              ] ;
      <http://mdacc.org/ClinicalLatha#manifestedBy>
              <http://mdacc.org/ClinicalLatha#CervicalCancer_CervicalCancer> ;
      label:designNote "This concept is extensible."^^xsd:string , "This concept may have instances of it's own or may be a superclass for concept refinements."^^xsd:string ;
      dc:creator foaf:JimLomax .

<http://mdacc.org/ClinicalLatha#CervixAnatomicSite>
      rdf:type owl:Class ;
      rdfs:comment "The lower part of the uterus occupying the region between the isthmus of the uterus and the vagina. It is divided into supravaginal and vaginal portions."^^xsd:string ;
      rdfs:subClassOf <http://mdacc.org/ClinicalLatha#AnatomicSite> ;
      label:correspondsTo label:Cervix_NCIURI ;
      label:designNote "This concept is directly related to the Cervix concept in NCI Thesaurus."^^xsd:string , "This concept may have specific instances."^^xsd:string , "This concept is extensible; more specific anatomic location within the cervix."^^xsd:string ;
      dc:creator foaf:JimLomax .

<http://mdacc.org/ClinicalLatha#Cervix_CervixAnatomicSite>
      rdf:type <http://mdacc.org/ClinicalLatha#CervixAnatomicSite> ;
      label:correspondsTo label:Cervix_NCIURI ;
      label:creator foaf:JimLomax ;
      skos-xl:prefLabel label:Cervix_AnatomicSiteLabel .

<http://mdacc.org/ClinicalLatha#Chemotherapy>
      rdf:type owl:Class ;
      rdfs:comment "The use of synthetic or naturally-occurring chemicals for the treatment of diseases. Although this term is used to describe any therapy involving the use of chemical-based agents, it is particularly used to refer to the use of chemical-based agents to treat cancer."^^xsd:string ;
      rdfs:subClassOf <http://mdacc.org/ClinicalLatha#DrugTherapy> ;
      rdfs:subClassOf
              [ rdf:type owl:Restriction ;
                owl:onProperty <http://mdacc.org/ClinicalLatha#administersTherapeuticAgent> ;
                owl:someValuesFrom <http://mdacc.org/Drug#ChemotherapyDrug>
              ] ;
      label:correspondsTo label:Chemotherapy_NCIURI ;
      label:designNote "This concept is extensible."^^xsd:string , "This concept is directly related to the Chemotherapy concept in NCI Thesaurus."^^xsd:string , "This concept may have instances of it's own or may be a superclass for concept refinements."^^xsd:string ;
      dc:contributor foaf:JimLomax .

<http://mdacc.org/ClinicalLatha#ChemotherapyExistentialEvent>
      rdf:type owl:Class ;
      rdfs:comment "This concept represents the existential nature of a chemotherapy procedure; the concept is not concerned with spatio-temporal aspects of the event, only that it occurred."^^xsd:string ;
      rdfs:subClassOf <http://mdacc.org/ClinicalLatha#TherapeuticProcedureExistentialEvent> ;
      label:designNote "This concept is related to the Chemotherapy under TherapeuticProcedure"^^xsd:string , "This concept may be domeoted to an instance"^^xsd:string , "This existential concept is a product of TCGA's need to capture just the existence of a chemotherapy."^^xsd:string ;
      dc:creator foaf:JimLomax .

<http://mdacc.org/ClinicalLatha#ChemotherapyNoChange_TherapeuticProcedureOutcome>
      rdf:type <http://mdacc.org/ClinicalLatha#TherapeuticProcedureOutcome> .

<http://mdacc.org/ClinicalLatha#ChronicLymphocyticLeukemia_Leukemia>
      rdf:type <http://mdacc.org/ClinicalLatha#Leukemia> ;
      rdfs:comment "The most common type of chronic lymphoid leukemia. It comprises 90% of chronic lymphoid leukemias in the United States. Morphologically, the neoplastic cells are small, round B-lymphocytes. This type of leukemia is not considered to be curable with available therapy"^^xsd:string ;
      label:correspondsTo label:ChronicLymphocyticLeukemia_NCIURI ;
      label:creator foaf:JimLomax ;
      skos-xl:prefLabel label:ChronicLymphocyticLeukemia_LeukemiaDiseaseLabel .

<http://mdacc.org/ClinicalLatha#ClinicalPackage>
      rdf:type owl:Class ;
      rdfs:comment "The Clinical Package is a organizational entity for containing the classes and properties that are most relevant to the observation and treatment of patients."^^xsd:string ;
      rdfs:subClassOf owl:Thing ;
      dc:creator foaf:JimLomax .

<http://mdacc.org/ClinicalLatha#ClinicalProcurementStatus_Completed>
      rdf:type archive:ClinicalProcurementStatus ;
      rdfs:comment "The data resource is available, has been requested and received."^^xsd:string ;
      dc:creator foaf:JimLomax ;
      dc:identifier "Completed"^^xsd:string .

<http://mdacc.org/ClinicalLatha#ClinicalProcurementStatus_Discrepancy>
      rdf:type archive:ClinicalProcurementStatus ;
      rdfs:comment "The name of the data resource has been received but is validity is in question."^^xsd:string ;
      dc:creator foaf:JimLomax ;
      dc:identifier "Discrepancy"^^xsd:string .

<http://mdacc.org/ClinicalLatha#ClinicalProcurementStatus_NotApplicable>
      rdf:type archive:ClinicalProcurementStatus ;
      rdfs:comment "The name of the data resource was not found."^^xsd:string ;
      dc:creator foaf:JimLomax ;
      dc:identifier "Not Applicable"^^xsd:string .

<http://mdacc.org/ClinicalLatha#ClinicalProcurementStatus_NotAvailable>
      rdf:type archive:ClinicalProcurementStatus ;
      rdfs:comment "The name of the data resource was not found and it will never be found (TCGA quote)."^^xsd:string ;
      dc:creator foaf:JimLomax ;
      dc:identifier "Not Available"^^xsd:string .

<http://mdacc.org/ClinicalLatha#ClinicalProcurementStatus_NotRequested>
      rdf:type archive:ClinicalProcurementStatus ;
      rdfs:comment "The data resource was not requested."^^xsd:string ;
      dc:creator foaf:JimLomax ;
      dc:identifier "Not Requested"^^xsd:string .

<http://mdacc.org/ClinicalLatha#ClinicalProcurementStatus_Pending>
      rdf:type archive:ClinicalProcurementStatus ;
      rdfs:comment "The name of the data resource has not yet been received but it is expected."^^xsd:string ;
      dc:creator foaf:JimLomax ;
      dc:identifier "Pending"^^xsd:string .

<http://mdacc.org/ClinicalLatha#ColonAdenocarcinoma_ColonCancer>
      rdf:type <http://mdacc.org/ClinicalLatha#ColonTumor> ;
      <http://mdacc.org/ClinicalLatha#anatomicLocation>
              <http://mdacc.org/ClinicalLatha#Colon_ColonAnatomicSite> ;
      <http://mdacc.org/ClinicalLatha#manifestedBy>
              <http://mdacc.org/ClinicalLatha#ColonCancer_ColonCancer> ;
      label:creator foaf:JimLomax ;
      skos-xl:prefLabel label:ColonAdenocarcinoma_ColonTumorLabel .

<http://mdacc.org/ClinicalLatha#ColonAnatomicSite>
      rdf:type owl:Class ;
      rdfs:comment "The part of the large intestine measured from the cecum to the rectum consisting of ascending, transverse, descending and sigmoid portions. The purpose of the colon is to remove water from digested food prior to excretion."^^xsd:string ;
      rdfs:subClassOf <http://mdacc.org/ClinicalLatha#AnatomicSite> ;
      label:correspondsTo label:Colon_NCIURI ;
      label:designNote "This concept is directly related to the Colon concept in NCI Thesaurus."^^xsd:string , "This concept is extensible; more specific anatomic location within the colon."^^xsd:string , "This concept may have specific instances"^^xsd:string ;
      dc:creator foaf:JimLomax .

<http://mdacc.org/ClinicalLatha#ColonCancer>
      rdf:type owl:Class ;
      rdfs:subClassOf <http://mdacc.org/ClinicalLatha#Cancer> ;
      rdfs:subClassOf
              [ rdf:type owl:Restriction ;
                owl:onProperty <http://mdacc.org/ClinicalLatha#anatomicLocation> ;
                owl:someValuesFrom <http://mdacc.org/ClinicalLatha#ColonAnatomicSite>
              ] ;
      dc:creator foaf:JimLomax .

<http://mdacc.org/ClinicalLatha#ColonCancer_ColonCancer>
      rdf:type <http://mdacc.org/ClinicalLatha#ColonCancer> ;
      <http://mdacc.org/ClinicalLatha#anatomicLocation>
              <http://mdacc.org/ClinicalLatha#Colon_ColonAnatomicSite> ;
      label:creator foaf:JimLomax .

<http://mdacc.org/ClinicalLatha#ColonTumor>
      rdf:type owl:Class ;
      rdfs:comment "Tumor anatomically located within the colon"^^xsd:string ;
      rdfs:subClassOf <http://mdacc.org/ClinicalLatha#TumorType> ;
      rdfs:subClassOf
              [ rdf:type owl:Restriction ;
                owl:onProperty <http://mdacc.org/ClinicalLatha#anatomicLocation> ;
                owl:someValuesFrom <http://mdacc.org/ClinicalLatha#ColonAnatomicSite>
              ] ;
      label:designNote "This concept is extensible."^^xsd:string , "This concept may have instances of it's own or may be a superclass for concept refinements."^^xsd:string ;
      dc:creator foaf:JimLomax .

<http://mdacc.org/ClinicalLatha#Colon_ColonAnatomicSite>
      rdf:type <http://mdacc.org/ClinicalLatha#ColonAnatomicSite> ;
      label:correspondsTo label:Colon_NCIURI ;
      label:creator foaf:JimLomax ;
      skos-xl:prefLabel label:Colon_ColonLabel .

<http://mdacc.org/ClinicalLatha#CombinationRadiation>
      rdf:type owl:Class ;
      rdfs:subClassOf <http://mdacc.org/Drug#Radiation> .

<http://mdacc.org/ClinicalLatha#CombinationRadiationTherapy>
      rdf:type owl:Class ;
      rdfs:subClassOf <http://mdacc.org/ClinicalLatha#RadiationTherapy> ;
      label:designNote "This concept is extensible."^^xsd:string , "This concept may have instances of it's own or may be a superclass for concept refinements."^^xsd:string ;
      dc:creator foaf:JimLomax .

<http://mdacc.org/ClinicalLatha#CompleteResponse_PrimaryTherapyOutcome>
      rdf:type <http://mdacc.org/ClinicalLatha#PrimaryTherapyOutcome> ;
      label:creator foaf:JimLomax ;
      skos-xl:prefLabel label:CompleteResponse_OutcomeLabel .

<http://mdacc.org/ClinicalLatha#Concentration>
      rdf:type owl:Class ;
      rdfs:comment "The quantity of a substance per volume or unit of weight."^^xsd:string ;
      rdfs:subClassOf <http://mdacc.org/ClinicalLatha#Quantity> ;
      rdfs:subClassOf
              [ rdf:type owl:Restriction ;
                owl:onProperty skos-xl:prefLabel ;
                owl:someValuesFrom label:ConcentrationLabel
              ] ;
      label:correspondsTo label:Concentration_NCIURI ;
      label:designNote "This concept directly corresponds to the Concentration concept in BioPortal"^^xsd:string ;
      dc:creator foaf:JimLomax .

<http://mdacc.org/ClinicalLatha#ConcentrationUnits>
      rdf:type owl:Class ;
      rdfs:subClassOf <http://mdacc.org/ClinicalLatha#Units> ;
      label:creator foaf:JimLomax .

<http://mdacc.org/ClinicalLatha#ConnectiveTissue>
      rdf:type owl:Class ;
      rdfs:comment "Tissue that supports and binds other tissues. It consists of conenctive tissue cells embedded in a large amount of extracellular matrix."^^xsd:string ;
      rdfs:subClassOf <http://mdacc.org/ClinicalLatha#Tissue> ;
      rdfs:subClassOf
              [ rdf:type owl:Restriction ;
                owl:onProperty <http://mdacc.org/ClinicalLatha#composedOf> ;
                owl:someValuesFrom <http://mdacc.org/ClinicalLatha#ConnectiveTissueCell>
              ] ;
      label:correspondsTo label:ConnectiveTissue_MESHURI ;
      label:designNote "This concept is extensible; there are different types of connective tissues each of which will have different properties."^^xsd:string , "This concept is directly related to the ConnectiveTissue concept in MESH."^^xsd:string , "Connective tissues are composed of connective tissue cells of the same type."^^xsd:string ;
      dc:creator foaf:JimLomax .

<http://mdacc.org/ClinicalLatha#ConnectiveTissueCell>
      rdf:type owl:Class ;
      rdfs:comment "As the name implies, connective tissue cells compose connective tissue which serves a \"connecting\" function. It supports and binds other tissues. Unlike epithelial tissue, connective tissue typically has cells scattered throughout an extracellular matrix."^^xsd:string ;
      rdfs:subClassOf <http://mdacc.org/ClinicalLatha#Cell> ;
      label:correspondsTo label:ConnectiveTissueCell_MESHURI ;
      label:designNote "This concept is extensible."^^xsd:string , "This concept is directly related to the Connective Tissue Cell concept in MESH."^^xsd:string , "This concept may have instances of it's own or may be a superclass for concept refinements."^^xsd:string ;
      dc:creator foaf:JimLomax .

<http://mdacc.org/ClinicalLatha#Cytology_DiagnosticProcedure>
      rdf:type <http://mdacc.org/ClinicalLatha#DiagnosticProcedure> ;
      label:creator foaf:JimLomax ;
      skos-xl:prefLabel label:Cytology_DiagnosticProcedureLabel .

<http://mdacc.org/ClinicalLatha#DNA>
      rdf:type owl:Class ;
      rdfs:comment "DNA is a double-stranded molecule held together by weak bonds between base pairs of nucleotides. DNA contain the four nucleotide bases adenine (A), guanine (G), cytosine (C), and thymine (T). In nature, base pairs form only between A and T and between G and C; thus the base sequence of each single strand can be deduced from that of its partner."^^xsd:string ;
      rdfs:label "DNA is a double-stranded molecule held together by weak bonds between base pairs of nucleotides. DNA contain the four nucleotide bases adenine (A), guanine (G), cytosine (C), and thymine (T). In nature, base pairs form only between A and T and between G and C; thus the base sequence of each single strand can be deduced from that of its partner."^^xsd:string ;
      rdfs:subClassOf <http://mdacc.org/ClinicalLatha#BioMaterial> ;
      label:correspondsTo label:DNA_NCIURI ;
      label:creator foaf:JimLomax ;
      label:designNote "This concept is extensible; there are different types of DNA (single stranded, double stranded) each of which could have different properties."^^xsd:string , "This concept may have instances of it's own or may be a superclass for concept refinements."^^xsd:string , "This concept is directly related to the DNA concept in NCI Thesaurus."^^xsd:string .

<http://mdacc.org/ClinicalLatha#DNAAmplicationSuccessful>
      rdf:type owl:Class ;
      rdfs:comment "Indicates if the PCR amplification was succesful for this dna analyte of a tissue sample"^^xsd:string ;
      rdfs:subClassOf <http://mdacc.org/ClinicalLatha#ClinicalPackage> ;
      label:designNote "This concept is most likely better represented as a property of the process of DNA Amplification and within a molecular domain."^^xsd:string , "This concept could not be found in BioPortal"^^xsd:string .

<http://mdacc.org/ClinicalLatha#DNAMethylationBioAssayAffymetrix>
      rdf:type mage:PhysicalBioAssay .

<http://mdacc.org/ClinicalLatha#DeathExistentialEvent>
      rdf:type owl:Class ;
      rdfs:comment "This existential concept is a product of TCGA's need to capture just the existence of a death; this is due in part to the fact that specific death details such as date and place may not be available (or necessary)."^^xsd:string ;
      rdfs:subClassOf <http://mdacc.org/ClinicalLatha#ExistentialEvent> ;
      label:correspondsTo label:Death_NCIURI ;
      label:designNote "This concept may be demoted to an instance"^^xsd:string , "This concept is directly related to the Death concept in NCI Thesaurus."^^xsd:string , "This existential concept is a product of TCGA's need to capture just the existence of a death; this is due in part to the fact that specific death details such as date and place may not be available (or necessary)."^^xsd:string ;
      dc:creator foaf:JimLomax .

<http://mdacc.org/ClinicalLatha#Deceased_VitalStatus>
      rdf:type <http://mdacc.org/ClinicalLatha#VitalStatus> ;
      label:correspondsTo label:Death_NCIURI ;
      label:designNote "This concept is directly related to the Death concept in NCI Thesaurus."^^xsd:string .

<http://mdacc.org/ClinicalLatha#DedifferentiatedLiposarcoma_Liposarcoma>
      rdf:type <http://mdacc.org/ClinicalLatha#Liposarcoma> ;
      rdfs:comment "A liposarcoma of any histologic subtype mixed with a non-lipomatous, high grade sarcomatous component. The non-lipomatous component may be present in the primary lesion or at the site of metastasis."^^xsd:string ;
      label:correspondsTo label:DedifferentiatedLiposarcoma_NCIURI ;
      label:creator foaf:JimLomax ;
      skos-xl:prefLabel label:DedifferentiatedLiposarcoma_LiposarcomaTumorLabel .

<http://mdacc.org/ClinicalLatha#Diagnosis>
      rdf:type owl:Class ;
      rdfs:comment "The investigation, analysis and recognition of the presence and nature of disease, condition, or injury from expressed signs and symptoms; also, the scientific determination of any kind; the concise results of such an investigation."^^xsd:string ;
      rdfs:subClassOf skos:Concept , <http://mdacc.org/ClinicalLatha#ClinicalPackage> ;
      rdfs:subClassOf
              [ rdf:type owl:Restriction ;
                owl:onProperty skos-xl:prefLabel ;
                owl:someValuesFrom label:DiagnosisLabel
              ] ;
      rdfs:subClassOf
              [ rdf:type owl:Restriction ;
                owl:onProperty <http://mdacc.org/ClinicalLatha#indicates> ;
                owl:someValuesFrom <http://mdacc.org/ClinicalLatha#Finding>
              ] ;
      label:correspondsTo label:Diagnosis_NCIURI ;
      label:designNote "This concept is extensible."^^xsd:string , "A diagnosis indicates some finding as the result of investigation or observation."^^xsd:string , "This concept is directly related to the Diagnosis concept in NCI Thesaurus."^^xsd:string , "This concept may have instances of it's own or may be a superclass for concept refinements."^^xsd:string ;
      dc:creator foaf:JimLomax .

<http://mdacc.org/ClinicalLatha#DiagnosisPatient1_PatientEvent>
      rdf:type <http://mdacc.org/ClinicalLatha#DiagnosisPatientEvent> ;
      <http://mdacc.org/ClinicalLatha#diagnosis>
              <http://mdacc.org/ClinicalLatha#ExampleInitialDiagnosis_Diagnosis> ;
      time-entry:inCalendarClockDataType
              "2010-03-05T00:56:50.76"^^xsd:dateTime .

<http://mdacc.org/ClinicalLatha#DiagnosisPatientEvent>
      rdf:type owl:Class ;
      rdfs:comment "The investigation, analysis and recognition of the presence and nature of disease, condition, or injury from expressed signs and symptoms; also, the scientific determination of any kind; the concise results of such an investigation."^^xsd:string ;
      rdfs:subClassOf skos:Concept ;
      dc:creator foaf:JimLomax .

<http://mdacc.org/ClinicalLatha#DiagnosticProcedure>
      rdf:type owl:Class ;
      rdfs:comment "Methods, procedures, and tests performed to diagnose disease, disordered function, or disability."^^xsd:string ;
      rdfs:subClassOf skos:Concept , <http://mdacc.org/ClinicalLatha#ClinicalPackage> ;
      rdfs:subClassOf
              [ rdf:type owl:Restriction ;
                owl:onProperty skos-xl:prefLabel ;
                owl:someValuesFrom label:DiagnosticProcedureLabel
              ] ;
      label:correspondsTo label:DiagnosticProcedure_NCIURI ;
      label:designNote "This concept is extensible."^^xsd:string , "This concept is directly related to the Diagnostic Procedure concept in NCI Thesaurus."^^xsd:string , "This concept may have instances of it's own or may be a superclass for concept refinements."^^xsd:string ;
      dc:creator foaf:JimLomax .

<http://mdacc.org/ClinicalLatha#DiffuseAnaplasia_AnaplasiaFinding>
      rdf:type <http://mdacc.org/ClinicalLatha#AnaplasiaFinding> ;
      rdfs:comment "Diffuse anaplasia is not focused in a particular area, it is wdespread within a anatomical region."^^xsd:string ;
      label:correspondsTo label:DiffuseAnaplasia_SNOMEDURI ;
      label:designNote "Thsi concept directly corresponds to the Diffuse Anaplasia concept in SNOMED."^^xsd:string ;
      dc:creator foaf:JimLomax ;
      skos-xl:prefLabel label:DiffuseAnaplasia_AnaplasiaLabel .

<http://mdacc.org/ClinicalLatha#DiffuseLargeBCellLymphoma_LymphoidCancer>
      rdf:type <http://mdacc.org/ClinicalLatha#LymphoidCancer> ;
      label:correspondsTo label:DiffuseLargeBCellLymphoma_NCIURI ;
      label:creator foaf:JimLomax ;
      skos-xl:prefLabel label:DiffuseLargeBCellLymphoma_LymphocyticCancerDiseaseLabel .

<http://mdacc.org/ClinicalLatha#Disease>
      rdf:type owl:Class ;
      rdfs:subClassOf skos:Concept , <http://mdacc.org/ClinicalLatha#ClinicalPackage> ;
      rdfs:subClassOf
              [ rdf:type owl:Restriction ;
                owl:onProperty skos-xl:prefLabel ;
                owl:someValuesFrom label:DiseaseLabel
              ] ;
      label:correspondsTo label:Disease_NCIURI ;
      label:designNote "This concept is extensible."^^xsd:string , "This concept is directly related to the Disease concept in NCI Thesaurus."^^xsd:string , "This concept may have instances of it's own or may be a superclass for concept refinements."^^xsd:string ;
      dc:creator foaf:JimLomax .

<http://mdacc.org/ClinicalLatha#DiseaseMarker>
      rdf:type owl:Class ;
      rdfs:comment "Specific molecular signature of disease, physiological measurement, genotype structural or functional characteristic, metabolic changes, or other determinant that may simplify the diagnostic process, make diagnoses more accurate, distinguish different causes of disease, or enable physicians to make diagnoses before symptoms appear and to track disease progression."^^xsd:string ;
      rdfs:subClassOf <http://mdacc.org/ClinicalLatha#Biomarker> ;
      label:correspondsTo label:DiseaseMarker_NCIURI ;
      label:designNote "This concept is extensible."^^xsd:string , "This concept is directly related to the Disease Marker concept in NCI Thesaurus."^^xsd:string , "This concept may have instances of it's own or may be a superclass for concept refinements."^^xsd:string ;
      dc:creator foaf:JimLomax .

<http://mdacc.org/ClinicalLatha#DiseaseOutcome>
      rdf:type owl:Class ;
      rdfs:comment "The outcome of a disease. There are most likely members to this concept that are defined by NCI Thesaurus. The likely candidates are Vital Status"^^xsd:string ;
      rdfs:subClassOf <http://mdacc.org/ClinicalLatha#Outcome> ;
      rdfs:subClassOf
              [ rdf:type owl:Restriction ;
                owl:onProperty <http://mdacc.org/ClinicalLatha#outcomeOf> ;
                owl:someValuesFrom <http://mdacc.org/ClinicalLatha#Disease>
              ] ;
      label:correspondsTo label:DiseaseOutcome_NCIURI ;
      label:designNote "This concept is extensible."^^xsd:string , "This concept is directly related to the Disease Outcome concept in NCI Thesaurus."^^xsd:string , "This concept may have instances of it's own or may be a superclass for concept refinements."^^xsd:string ;
      dc:creator foaf:JimLomax .

<http://mdacc.org/ClinicalLatha#DiseaseScoringSystem>
      rdf:type owl:Class ;
      rdfs:comment "The concept of a scoring system for a disease. A disease scoring system is a methodology for rating disease state (or porgression). Typically, but not always, a disease scoring system is confined to a particular disease, such as Ovarian Cancer."^^xsd:string ;
      rdfs:subClassOf <http://mdacc.org/ClinicalLatha#ClinicalPackage> ;
      label:designNote "This concept is extensible."^^xsd:string , "This concept could not be found in BioPortal"^^xsd:string , "This concept may have instances of it's own or may be a superclass for concept refinements."^^xsd:string ;
      dc:creator foaf:JimLomax .

<http://mdacc.org/ClinicalLatha#DiseaseStagingSystem>
      rdf:type owl:Class ;
      rdfs:comment "A systematic method for clinicopathologic evaluation of tumors."^^xsd:string ;
      rdfs:subClassOf <http://mdacc.org/ClinicalLatha#ClinicalPackage> ;
      label:designNote "This concept is extensible."^^xsd:string , "This concept could not be found in BioPortal"^^xsd:string , "This concept may have instances of it's own or may be a superclass for concept refinements."^^xsd:string ;
      dc:creator foaf:JimLomax .

<http://mdacc.org/ClinicalLatha#Dosage>
      rdf:type owl:Class ;
      rdfs:comment "A quantity of an agent (such as substance or energy) administered, taken, or absorbed at one time."^^xsd:string ;
      rdfs:subClassOf <http://mdacc.org/ClinicalLatha#Quantity> ;
      rdfs:subClassOf
              [ rdf:type owl:Restriction ;
                owl:onProperty skos-xl:prefLabel ;
                owl:someValuesFrom label:DosageLabel
              ] ;
      label:correspondsTo label:Dosage_SNOMEDURI ;
      label:designNote "This concept is extensible."^^xsd:string , "This concept directly corresponds to the Dosage concept in SNOMED."^^xsd:string , "This concept may have instances of it's own or may be a superclass for concept refinements."^^xsd:string ;
      dc:creator foaf:JimLomax .

<http://mdacc.org/ClinicalLatha#DosageUnits>
      rdf:type owl:Class ;
      rdfs:subClassOf <http://mdacc.org/ClinicalLatha#Units> ;
      dc:creator foaf:JimLomax .

<http://mdacc.org/ClinicalLatha#DrugDosage>
      rdf:type owl:Class ;
      rdfs:subClassOf <http://mdacc.org/ClinicalLatha#Dosage> ;
      rdfs:subClassOf
              [ rdf:type owl:Restriction ;
                owl:onProperty skos-xl:prefLabel ;
                owl:someValuesFrom label:DosageLabel
              ] ;
      dc:creator foaf:JimLomax .

<http://mdacc.org/ClinicalLatha#DrugDosageUnits>
      rdf:type owl:Class ;
      rdfs:subClassOf <http://mdacc.org/ClinicalLatha#DosageUnits> ;
      dc:creator foaf:JimLomax .

<http://mdacc.org/ClinicalLatha#DrugTherapy>
      rdf:type owl:Class ;
      rdfs:comment "Administration of medication"^^xsd:string ;
      rdfs:subClassOf <http://mdacc.org/ClinicalLatha#TherapeuticProcedure> ;
      rdfs:subClassOf
              [ rdf:type owl:Restriction ;
                owl:onProperty <http://mdacc.org/ClinicalLatha#dosage> ;
                owl:someValuesFrom <http://mdacc.org/Drug#Dosage>
              ] ;
      rdfs:subClassOf
              [ rdf:type owl:Restriction ;
                owl:maxCardinality "1"^^xsd:int ;
                owl:onProperty <http://mdacc.org/ClinicalLatha#dosage>
              ] ;
      rdfs:subClassOf
              [ rdf:type owl:Restriction ;
                owl:onProperty <http://mdacc.org/ClinicalLatha#administersTherapeuticAgent> ;
                owl:someValuesFrom <http://mdacc.org/Drug#Drug>
              ] ;
      label:correspondsTo label:DrugTherapy_SNOMEDURI ;
      label:designNote "This concept is extensible."^^xsd:string , "This concept is directly related to the Drug Therapy concept in NCI Thesaurus."^^xsd:string , "This concept may have instances of it's own or may be a superclass for concept refinements."^^xsd:string ;
      dc:creator foaf:JimLomax .

<http://mdacc.org/ClinicalLatha#DukeBrainBankOwner>
      rdf:type mage:Person .

<http://mdacc.org/ClinicalLatha#DuraMater_LeptomeningesMeninges>
      rdf:type <http://mdacc.org/ClinicalLatha#Leptomeninges> , <http://mdacc.org/ClinicalLatha#Meninges> ;
      label:correspondsTo label:DuraMater_NCIURI ;
      label:creator foaf:JimLomax .

<http://mdacc.org/ClinicalLatha#DurationDescription_30Days>
      rdf:type time-entry:DurationDescription ;
      time-entry:days "30"^^xsd:decimal .

<http://mdacc.org/ClinicalLatha#EBVImmortalizedBCell>
      rdf:type owl:Class ;
      rdfs:comment "There is no corresponding concept in Bioportal"^^xsd:string , "A B Cell that has been immortalized by EBV"^^xsd:string ;
      rdfs:subClassOf <http://mdacc.org/ClinicalLatha#ImmortalizedBCell> ;
      rdfs:subClassOf
              [ rdf:type owl:Restriction ;
                owl:onProperty <http://mdacc.org/ClinicalLatha#immortalizingAgent> ;
                owl:someValuesFrom <http://mdacc.org/ClinicalLatha#EpsteinBarrVirus>
              ] ;
      label:designNote "This concept may have instances of it's own or may be a superclass for concept refinements."^^xsd:string ;
      dc:creator foaf:JimLomax .

<http://mdacc.org/ClinicalLatha#EndocrineTherapy>
      rdf:type owl:Class ;
      rdfs:comment "Treatment that adds, blocks, or removes hormones"^^xsd:string ;
      rdfs:subClassOf <http://mdacc.org/ClinicalLatha#DrugTherapy> ;
      rdfs:subClassOf
              [ rdf:type owl:Restriction ;
                owl:onProperty <http://mdacc.org/ClinicalLatha#administersTherapeuticAgent> ;
                owl:someValuesFrom <http://mdacc.org/Drug#EndocrineTherapyDrug>
              ] ;
      label:correspondsTo label:HormoneTherapy_NCIURI ;
      label:designNote "This concept is extensible."^^xsd:string , "This concept is directly related to the Hormone Therapy concept in NCI Thesaurus."^^xsd:string , "This concept may have instances of it's own or may be a superclass for concept refinements."^^xsd:string ;
      dc:creator foaf:JimLomax .

<http://mdacc.org/ClinicalLatha#EndocrineTherapyExistentialEvent>
      rdf:type owl:Class ;
      rdfs:comment "This concept represents the existential nature of an endocrine therapeutic procedure; the concept is not concerned with spatio-temporal aspects of the event, only that it occurred."^^xsd:string ;
      rdfs:subClassOf <http://mdacc.org/ClinicalLatha#TherapeuticProcedureExistentialEvent> ;
      label:designNote "This existential concept is a product of TCGA's need to capture just the existence of a endocrine therapy."^^xsd:string , "This concept may be domoted to an instance"^^xsd:string , "This concept is related to the Endocrine Therapy under Therapeutic Procedure"^^xsd:string ;
      dc:creator foaf:JimLomax .

<http://mdacc.org/ClinicalLatha#EpithelialCell>
      rdf:type owl:Class ;
      rdfs:comment "Cells that line the inner and outer surfaces of the body by forming cellular layers, epithelium, or masses. Epithelial cells lining the skin; the mouth; the nose; and the anal canal derive from ectoderm; those lining the respitory system and the digestive system derive from endoderm; others (cardiovascular system and lymphatic system) from mesoderm."^^xsd:string ;
      rdfs:subClassOf <http://mdacc.org/ClinicalLatha#Cell> ;
      label:correspondsTo label:EpithelialCell_NCIURI , label:EpithelialCell_MESHURI ;
      label:designNote "This concept is extensible."^^xsd:string , "This concept is directly related to the Epithelial Cell concept in MESH and NCI Thesaurus"^^xsd:string , "This concept may have instances of it's own or may be a superclass for concept refinements."^^xsd:string ;
      dc:creator foaf:JimLomax .

<http://mdacc.org/ClinicalLatha#EpithelialCell1_EpithelialCell>
      rdf:type <http://mdacc.org/ClinicalLatha#EpithelialCell> .

<http://mdacc.org/ClinicalLatha#Epithelium>
      rdf:type owl:Class ;
      rdfs:comment "One or more layers of epithelial cells, supported by the basal lamina, which covers the inner or outer surfaces of the body."^^xsd:string ;
      rdfs:subClassOf <http://mdacc.org/ClinicalLatha#Tissue> ;
      rdfs:subClassOf
              [ rdf:type owl:Restriction ;
                owl:onProperty <http://mdacc.org/ClinicalLatha#composedOf> ;
                owl:someValuesFrom <http://mdacc.org/ClinicalLatha#EpithelialCell>
              ] ;
      label:correspondsTo label:Epithelium_MESHURI ;
      label:designNote "This concept is directly related to the Epithelial Tissue concept in MESH."^^xsd:string , "This concept may have instances of it's own or may be a superclass for concept refinements."^^xsd:string , "This concept is extensible; there are different types of epithelial  tissues each of which will have different properties."^^xsd:string ;
      dc:creator foaf:JimLomax .

<http://mdacc.org/ClinicalLatha#EpsteinBarrVirus>
      rdf:type owl:Class ;
      rdfs:comment "The Epstein-Barr virus (EBV), also called human herpesvirus 4 (HHV-4), is a cancer-causing virus of the herpes family, which includes herpes simplex virus 1 and 2, and is one of the most common viruses in humans"^^xsd:string ;
      rdfs:subClassOf <http://mdacc.org/ClinicalLatha#Virus> , skos:Concept ;
      rdfs:subClassOf
              [ rdf:type owl:Restriction ;
                owl:onProperty skos-xl:prefLabel ;
                owl:someValuesFrom label:EpsteinBarrVirusLabel
              ] ;
      label:correspondsTo label:EpsteinBarrVirus_NCIURI ;
      dc:creator foaf:JimLomax .

<http://mdacc.org/ClinicalLatha#Equipment>
      rdf:type owl:Class ;
      rdfs:subClassOf <http://mdacc.org/ClinicalLatha#ClinicalPackage> ;
      label:correspondsTo label:Equipment_NCIURI ;
      label:designNote "This concept is extensible."^^xsd:string , "This concept is directly related to the Equipment concept in NCI Thesaurus."^^xsd:string , "This concept may have instances of it's own or may be a superclass for concept refinements."^^xsd:string ;
      dc:creator foaf:JimLomax .

<http://mdacc.org/ClinicalLatha#Ethnicity>
      rdf:type owl:Class ;
      rdfs:comment "The US Census Bureau makes use of both race and ethnicity in surveys, however there are no race or ethnicity vocabularies or taxonomies used."^^xsd:string , "http://en.wikipedia.org/wiki/Race_and_ethnicity_in_the_United_States_Census"^^xsd:string ;
      rdfs:subClassOf <http://mdacc.org/ClinicalLatha#PopulationCharacteristic> ;
      rdfs:subClassOf
              [ rdf:type owl:Restriction ;
                owl:onProperty skos-xl:prefLabel ;
                owl:someValuesFrom label:EthnicityLabel
              ] ;
      label:correspondsTo label:Ethnicity_SNOMEDURI ;
      label:designNote "This concept is extensible."^^xsd:string , "This concept directly corresponds to the concept of Ethnicity in SNOMED."^^xsd:string ;
      dc:creator foaf:JimLomax .

<http://mdacc.org/ClinicalLatha#ExampleBrain_Tumor>
      rdf:type <http://mdacc.org/ClinicalLatha#Tumor> ;
      <http://mdacc.org/ClinicalLatha#tumorClassification>
              <http://mdacc.org/ClinicalLatha#Glioblastoma_Glioblastoma> .

<http://mdacc.org/ClinicalLatha#ExampleFalse_AdditonalHormoneTherapyExistentialEvent>
      rdf:type <http://mdacc.org/ClinicalLatha#AdditonalHormoneTherapyExistentialEvent> ;
      <http://mdacc.org/ClinicalLatha#occurred>
              "false"^^xsd:boolean .

<http://mdacc.org/ClinicalLatha#ExampleFalse_EndocrineExistentialEvent>
      rdf:type <http://mdacc.org/ClinicalLatha#EndocrineTherapyExistentialEvent> ;
      <http://mdacc.org/ClinicalLatha#occurred>
              "false"^^xsd:boolean ;
      label:creator foaf:JimLomax .

<http://mdacc.org/ClinicalLatha#ExampleFalse_RadiationExistentialEvent>
      rdf:type <http://mdacc.org/ClinicalLatha#RadiationTherapyExistentialEvent> ;
      label:creator foaf:JimLomax .

<http://mdacc.org/ClinicalLatha#ExampleGrade1A_BladderCancerTumorGrade>
      rdf:type <http://mdacc.org/ClinicalLatha#TumorGrade> ;
      <http://mdacc.org/ClinicalLatha#cancer>
              <http://mdacc.org/ClinicalLatha#BladderCancer_BladderCancer> ;
      dc:identifier "1A"^^xsd:string .

<http://mdacc.org/ClinicalLatha#ExampleInitialDiagnosis_Diagnosis>
      rdf:type <http://mdacc.org/ClinicalLatha#Diagnosis> ;
      <http://mdacc.org/ClinicalLatha#establishedBy>
              <http://mdacc.org/ClinicalLatha#IncisionBioposy_DiagnosticProcedure> ;
      <http://mdacc.org/ClinicalLatha#indicates>
              <http://mdacc.org/ClinicalLatha#BladderCancer_BladderCancer> ;
      label:creator foaf:JimLomax ;
      temporal:dateTime "2010-11-23"^^xsd:string .

<http://mdacc.org/ClinicalLatha#ExamplePatient_Patient>
      rdf:type <http://mdacc.org/ClinicalLatha#Patient> ;
      rdfs:comment "Here is an example of a Patient that received an External Beam Radiation Therapy session with more than existential information."^^xsd:string , "Here is an example of a Patient that received Chemotherapy but the treatment is only existential; it occurred but no detail has been collected. This level of detail can still be useful in cohort studies."^^xsd:string ;
      <http://mdacc.org/ClinicalLatha#ethnicity>
              <http://mdacc.org/ClinicalLatha#NotHispanicOrLatino_Ethnicity> ;
      <http://mdacc.org/ClinicalLatha#examinationApplied>
              <http://mdacc.org/exam#Example_Examination> ;
      <http://mdacc.org/ClinicalLatha#finding>
              <http://mdacc.org/ClinicalLatha#GeneralTumorProgression_TumorProgressionFinding> , <http://mdacc.org/ClinicalLatha#Example_ResidualTumorFinding> ;
      <http://mdacc.org/ClinicalLatha#initialDiagnosis>
              <http://mdacc.org/ClinicalLatha#ExampleInitialDiagnosis_Diagnosis> ;
      <http://mdacc.org/ClinicalLatha#outcome>
              <http://mdacc.org/ClinicalLatha#PartialResponse_PrimaryTherapyOutcome> ;
      <http://mdacc.org/ClinicalLatha#patientId>
              sample:Patient1_PatientId ;
      <http://mdacc.org/ClinicalLatha#therapyApplied>
              <http://mdacc.org/ClinicalLatha#Temozolomide_Chemotherapy> , <http://mdacc.org/ClinicalLatha#Taxomifen_Chemotherapy> , <http://mdacc.org/ClinicalLatha#TargetedMolecularTherapy_TherapeuticProcedure> ;
      <http://mdacc.org/ClinicalLatha#treatmentEventExists>
              <http://mdacc.org/ClinicalLatha#ExampleTrue_ChemotherapyExistentialEvent> , <http://mdacc.org/ClinicalLatha#ExampleFalse_EndocrineExistentialEvent> , <http://mdacc.org/ClinicalLatha#ExampleTrue_MolecularTherapyExistentialEvent> , <http://mdacc.org/ClinicalLatha#ExampleFalse_RadiationExistentialEvent> , <http://mdacc.org/ClinicalLatha#ExampleTrue_AdditonalChemotherapyExistentialEvent> .

<http://mdacc.org/ClinicalLatha#ExampleRecurrenceProgression_TumorRecurrenceFinding>
      rdf:type <http://mdacc.org/ClinicalLatha#TumorRecurrenceFinding> ;
      <http://mdacc.org/ClinicalLatha#anatomicLocation>
              <http://mdacc.org/ClinicalLatha#Colon_ColonAnatomicSite> ;
      temporal:dateTime "2010-12-14"^^xsd:string .

<http://mdacc.org/ClinicalLatha#ExampleStage1_BladderCancerTumorStage>
      rdf:type <http://mdacc.org/ClinicalLatha#BladderCancerTumorStage> ;
      <http://mdacc.org/ClinicalLatha#cancer>
              <http://mdacc.org/ClinicalLatha#BladderCancer_BladderCancer> ;
      <http://mdacc.org/ClinicalLatha#diseaseStagingSystem>
              <http://mdacc.org/ClinicalLatha#MDA_TNMDiseaseStagingSystem> ;
      dc:identifier "1"^^xsd:string .

<http://mdacc.org/ClinicalLatha#ExampleTrue_AdditonalChemotherapyExistentialEvent>
      rdf:type <http://mdacc.org/ClinicalLatha#AdditonalChemotherapyExistentialEvent> ;
      <http://mdacc.org/ClinicalLatha#occurred>
              "true"^^xsd:boolean .

<http://mdacc.org/ClinicalLatha#ExampleTrue_AdditonalDrugTherapyExistentialEvent>
      rdf:type <http://mdacc.org/ClinicalLatha#AdditonalDrugTherapyExistentialEvent> ;
      <http://mdacc.org/ClinicalLatha#occurred>
              "true"^^xsd:boolean .

<http://mdacc.org/ClinicalLatha#ExampleTrue_AdditonalImmunotherapyExistentialEvent>
      rdf:type <http://mdacc.org/ClinicalLatha#AdditonalImmunotherapyExistentialEvent> ;
      <http://mdacc.org/ClinicalLatha#occurred>
              "true"^^xsd:boolean .

<http://mdacc.org/ClinicalLatha#ExampleTrue_AdditonalRadiationTherapyExistentialEvent>
      rdf:type <http://mdacc.org/ClinicalLatha#AdditonalRadiationTherapyExistentialEvent> ;
      <http://mdacc.org/ClinicalLatha#occurred>
              "true"^^xsd:boolean .

<http://mdacc.org/ClinicalLatha#ExampleTrue_ChemotherapyExistentialEvent>
      rdf:type <http://mdacc.org/ClinicalLatha#ChemotherapyExistentialEvent> ;
      <http://mdacc.org/ClinicalLatha#occurred>
              "true"^^xsd:boolean ;
      label:creator foaf:JimLomax .

<http://mdacc.org/ClinicalLatha#ExampleTrue_MolecularTherapyExistentialEvent>
      rdf:type <http://mdacc.org/ClinicalLatha#TargetedMolecularTherapyExistentialEvent> ;
      <http://mdacc.org/ClinicalLatha#occurred>
              "true"^^xsd:boolean ;
      label:creator foaf:JimLomax .

<http://mdacc.org/ClinicalLatha#Example_Absorbance260To280Nm>
      rdf:type <http://mdacc.org/ClinicalLatha#Absorbance260To280Nm> ;
      <http://mdacc.org/ClinicalLatha#value>
              "2"^^xsd:string .

<http://mdacc.org/ClinicalLatha#Example_BirthExistentialEvent>
      rdf:type <http://mdacc.org/ClinicalLatha#BirthExistentialEvent> ;
      label:creator foaf:JimLomax .

<http://mdacc.org/ClinicalLatha#Example_CurrentWeight>
      rdf:type <http://mdacc.org/ClinicalLatha#Weight> ;
      <http://mdacc.org/ClinicalLatha#units>
              <http://mdacc.org/ClinicalLatha#Grams_WeightUnits> ;
      <http://mdacc.org/ClinicalLatha#value>
              "1.0"^^xsd:string .

<http://mdacc.org/ClinicalLatha#Example_DeathExistentialEvent>
      rdf:type <http://mdacc.org/ClinicalLatha#DeathExistentialEvent> ;
      rdfs:comment "Represents an existential death; only that a death occurred, no temporal deatils are captured"^^xsd:string ;
      label:creator foaf:JimLomax .

<http://mdacc.org/ClinicalLatha#Example_ExternalBeamRadiation>
      rdf:type <http://mdacc.org/ClinicalLatha#ExternalBeamRadiation> ;
      skos-xl:prefLabel label:ExternalBeam_RadiationLabel .

<http://mdacc.org/ClinicalLatha#Example_ExternalBeamRadiationTherapy>
      rdf:type <http://mdacc.org/ClinicalLatha#ExternalBeamRadiationTherapy> ;
      <http://mdacc.org/ClinicalLatha#dosage>
              <http://mdacc.org/ClinicalLatha#Gray44_RadiationDosage> ;
      <http://mdacc.org/ClinicalLatha#fractions>
              33 ;
      <http://mdacc.org/ClinicalLatha#ongoing>
              "true"^^xsd:boolean ;
      <http://mdacc.org/ClinicalLatha#treatmentSite>
              "treatment site"^^xsd:string ;
      label:barcode label:Example_BCRRadiationBarcode ;
      label:notes "Notes"^^xsd:string ;
      temporal:endedOn temporal:DrugTreatment1_EndDateTime ;
      temporal:numberOfDaysToTherapyEnd
              "123"^^xsd:int ;
      temporal:numberOfDaysToTherapyStart
              "21"^^xsd:int ;
      temporal:startedOn temporal:DrugTreatment1_StartDateTime .

<http://mdacc.org/ClinicalLatha#Example_InitialWeight>
      rdf:type <http://mdacc.org/ClinicalLatha#Weight> ;
      <http://mdacc.org/ClinicalLatha#units>
              <http://mdacc.org/ClinicalLatha#Grams_WeightUnits> ;
      <http://mdacc.org/ClinicalLatha#value>
              "1.2"^^xsd:string .

<http://mdacc.org/ClinicalLatha#Example_NuclearGrade>
      rdf:type <http://mdacc.org/ClinicalLatha#NuclearGrade> ;
      skos-xl:prefLabel label:Example_NuclearGradeLabel .

<http://mdacc.org/ClinicalLatha#Example_Regimen>
      rdf:type <http://mdacc.org/ClinicalLatha#Regimen> ;
      <http://mdacc.org/ClinicalLatha#therapeuticProcedure>
              <http://mdacc.org/ClinicalLatha#Temozolomide_Chemotherapy> , <http://mdacc.org/ClinicalLatha#Taxomifen_Chemotherapy> ;
      label:creator foaf:JimLomax ;
      label:notes "This is a sample note for regimen indication"^^xsd:string ;
      skos-xl:prefLabel label:DoubleChemo_RegimenLabel .

<http://mdacc.org/ClinicalLatha#Example_ResidualTumorFinding>
      rdf:type <http://mdacc.org/ClinicalLatha#ResidualTumorFinding> ;
      dc:identifier "1-10mm"^^xsd:string .

<http://mdacc.org/ClinicalLatha#Example_Slide>
      rdf:type <http://mdacc.org/ClinicalLatha#Slide> ;
      <http://mdacc.org/ClinicalLatha#numberProliferatingCells>
              12 ;
      <http://mdacc.org/ClinicalLatha#percentEosinophilInfiltration>
              "34.0"^^xsd:float ;
      <http://mdacc.org/ClinicalLatha#percentGranulocyteInfiltration>
              "3.7"^^xsd:float ;
      <http://mdacc.org/ClinicalLatha#percentInflammationInfiltration>
              "1.9"^^xsd:float ;
      <http://mdacc.org/ClinicalLatha#percentLymphocyteInfiltration>
              "22.2"^^xsd:float ;
      <http://mdacc.org/ClinicalLatha#percentMonocyteInfiltration>
              "8.5"^^xsd:float ;
      <http://mdacc.org/ClinicalLatha#percentNecrosis>
              "11.23"^^xsd:float ;
      <http://mdacc.org/ClinicalLatha#percentNeutrophilInfiltration>
              "3.78"^^xsd:float ;
      <http://mdacc.org/ClinicalLatha#percentNormalCells>
              "72.0"^^xsd:float ;
      <http://mdacc.org/ClinicalLatha#percentTumorCells>
              "20.4"^^xsd:float ;
      <http://mdacc.org/ClinicalLatha#percentTumorNuclei>
              "10.43"^^xsd:float ;
      <http://mdacc.org/ClinicalLatha#sectionLocation>
              <http://mdacc.org/ClinicalLatha#Top_Side> ;
      label:barcode label:Slide1_BCRSlideBarcode .

<http://mdacc.org/ClinicalLatha#Example_Weight>
      rdf:type <http://mdacc.org/ClinicalLatha#Weight> ;
      <http://mdacc.org/ClinicalLatha#units>
              <http://mdacc.org/ClinicalLatha#Pounds_WeightUnits> ;
      <http://mdacc.org/ClinicalLatha#value>
              "10.1"^^xsd:string .

<http://mdacc.org/ClinicalLatha#ExcisionBioposy_DiagnosticProcedure>
      rdf:type <http://mdacc.org/ClinicalLatha#DiagnosticProcedure> ;
      label:creator foaf:JimLomax ;
      skos-xl:prefLabel label:ExcisionalBiopsy_DiagnosticProcedureLabel .

<http://mdacc.org/ClinicalLatha#ExcisionSurgicalProcedure>
      rdf:type owl:Class ;
      rdfs:comment "Represents a surgical excision"^^xsd:string ;
      rdfs:subClassOf <http://mdacc.org/ClinicalLatha#SurgicalProcedure> ;
      label:correspondsTo label:Excision_NCIURI ;
      label:designNote "This concept is extensible."^^xsd:string , "This concept is directly related to the Excision concept in NCI Thesaurus."^^xsd:string , "This concept may have instances of it's own or may be a superclass for concept refinements."^^xsd:string ;
      dc:creator foaf:JimLomax .

<http://mdacc.org/ClinicalLatha#ExistentialEvent>
      rdf:type owl:Class ;
      rdfs:comment "An event for which spatio-temporal details are not relevant (or not captured); it is merely existential"^^xsd:string ;
      rdfs:subClassOf <http://mdacc.org/ClinicalLatha#ClinicalPackage> ;
      label:creator foaf:JimLomax ;
      label:designNote "There is no corresponding concept in BioPortal"^^xsd:string , "This concept may have instances of it's own or may be a superclass for concept refinements."^^xsd:string .

<http://mdacc.org/ClinicalLatha#ExternalBeamRadiation>
      rdf:type owl:Class ;
      rdfs:subClassOf <http://mdacc.org/Drug#Radiation> .

<http://mdacc.org/ClinicalLatha#ExternalBeamRadiationTherapy>
      rdf:type owl:Class ;
      rdfs:comment "Radiation therapy that uses a machine to aim high-energy rays at the cancer."^^xsd:string ;
      rdfs:subClassOf <http://mdacc.org/ClinicalLatha#RadiationTherapy> ;
      label:correspondsTo label:ExternalBeamRadiationTherapy_NCIURI ;
      label:designNote "This concept is extensible."^^xsd:string , "This concept is directly related to the External Beam Radiation Therapy concept in NCI Thesaurus."^^xsd:string , "This concept may have instances of it's own or may be a superclass for concept refinements."^^xsd:string ;
      dc:creator foaf:JimLomax .

<http://mdacc.org/ClinicalLatha#FatCell>
      rdf:type owl:Class ;
      rdfs:subClassOf <http://mdacc.org/ClinicalLatha#ConnectiveTissueCell> ;
      label:designNote "The concept is equivalent to the Adipocyte concept."^^xsd:string ;
      dc:creator foaf:JimLomax ;
      owl:equivalentClass <http://mdacc.org/ClinicalLatha#Adipocyte> .

<http://mdacc.org/ClinicalLatha#Female_Gender>
      rdf:type <http://mdacc.org/ClinicalLatha#Gender> ;
      label:correspondsTo label:Female_NCIURI ;
      label:creator foaf:JimLomax ;
      label:designNote "This concept directly corresponds to the concept of Female in NCI Thesaurus."^^xsd:string .

<http://mdacc.org/ClinicalLatha#Fibroblast>
      rdf:type owl:Class ;
      rdfs:comment "Connective tissue cells which secrete an extracellular matrix rich in collagen and other macromolecules."^^xsd:string ;
      rdfs:subClassOf <http://mdacc.org/ClinicalLatha#ConnectiveTissueCell> ;
      label:correspondsTo label:Fibroblast_MESHURI ;
      label:designNote "This concept is extensible."^^xsd:string , "This concept may have instances of it's own  or may be a superclass for concept refinements."^^xsd:string , "This concept is directly related to the Fibroblast concept in MESH."^^xsd:string ;
      dc:creator foaf:JimLomax .

<http://mdacc.org/ClinicalLatha#Finding>
      rdf:type owl:Class ;
      rdfs:comment "Objective evidence of disease perceptible to the examining physician (sign) and subjective evidence of disease perceived by the patient (symptom)."^^xsd:string ;
      rdfs:subClassOf skos:Concept , <http://mdacc.org/ClinicalLatha#ClinicalPackage> ;
      rdfs:subClassOf
              [ rdf:type owl:Restriction ;
                owl:onProperty skos-xl:prefLabel ;
                owl:someValuesFrom label:FindingLabel
              ] ;
      label:correspondsTo label:Finding_NCIURI ;
      label:designNote "This concept is extensible."^^xsd:string , "This concept may have instances of it's own or may be a superclass for concept refinements."^^xsd:string , "This concept is directly related to the Finding concept in NCI Thesaurus."^^xsd:string ;
      dc:creator foaf:JimLomax .

<http://mdacc.org/ClinicalLatha#FineNeedleAspirationBiopsy_DiagnosticProcedure>
      rdf:type <http://mdacc.org/ClinicalLatha#DiagnosticProcedure> ;
      label:creator foaf:JimLomax ;
      skos-xl:prefLabel label:FineNeedleAspirationBiopsy_DiagnosticProcedureLabel .

<http://mdacc.org/ClinicalLatha#FocalAnaplasia_AnaplasiaFinding>
      rdf:type <http://mdacc.org/ClinicalLatha#AnaplasiaFinding> ;
      rdfs:comment "Focal anaplasia applies only to tumors with anaplasia confined to one or a few discrete loci within the primary tumor, with no anaplasia or marked nuclear atypia elsewhere"^^xsd:string ;
      label:correspondsTo label:FocalAnaplasia_SNOMEDURI ;
      label:designNote "Thsi concept directly corresponds to the Focal Anaplasia concept in SNOMED."^^xsd:string ;
      dc:creator foaf:JimLomax ;
      skos-xl:prefLabel label:FocalAnaplasia_AnaplasiaLabel .

<http://mdacc.org/ClinicalLatha#Functions_1>
      rdf:type spin:Function ;
      rdfs:subClassOf spin:Functions .

<http://mdacc.org/ClinicalLatha#GBMSlide>
      rdf:type owl:Class ;
      rdfs:subClassOf <http://mdacc.org/ClinicalLatha#Slide> ;
      rdfs:subClassOf
              [ rdf:type owl:Restriction ;
                owl:onProperty <http://mdacc.org/ClinicalLatha#tumorOrigin> ;
                owl:someValuesFrom <http://mdacc.org/ClinicalLatha#Glioma>
              ] ;
      label:architect foaf:MoSanyang ;
      label:creator foaf:JimLomax ;
      label:developer foaf:PradheepRaju , foaf:DawitGebremichael .

<http://mdacc.org/ClinicalLatha#GelElectrophoresis>
      rdf:type owl:Class ;
      rdfs:comment "Gel electrophoresis is a method of separating large molecules (such as DNA fragments or proteins) from a mixture of similar molecules by electrophoretic filtration through a gelatinous matrix. Subject to an electric field, each molecule in the sample mixture migrates through the matrix at a different rate, depending mainly on electrical charge and size, resulting in spatial separation within the matrix of each molecular species in the sample mixture. Agarose and acrylamide in a cylindrical tube or slab gel are commonly used media for electrophoresis of proteins and nucleic acids."^^xsd:string ;
      rdfs:subClassOf <http://mdacc.org/ClinicalLatha#LabProcedure> ;
      label:correspondsTo label:GelElectrophoresis_NCIURI ;
      label:designNote "This concept is extensible."^^xsd:string , "This concept may have instances of it's own or may be a superclass for concept refinements."^^xsd:string , "This concept is directly related to the Gel Electrophoresis concept in NCI Thesaurus."^^xsd:string ;
      dc:creator foaf:JimLomax .

<http://mdacc.org/ClinicalLatha#Gemistocyte>
      rdf:type owl:Class ;
      rdfs:comment "A pathologic astrocyte in which the cell body swells and contains glial filaments and an eccentric nucleus; seen particularly in demyelinating and neoplastic conditions. "^^xsd:string ;
      rdfs:subClassOf <http://mdacc.org/ClinicalLatha#Astrocyte> ;
      label:correspondsTo label:Gemistocyte_NCIURI ;
      label:designNote "This concept is extensible."^^xsd:string , "This concept is directly related to the Gemistocyte concept in NCI Thesaurus"^^xsd:string , "This concept may have instances of it's own or may be a superclass for concept refinements."^^xsd:string ;
      dc:creator foaf:JimLomax .

<http://mdacc.org/ClinicalLatha#GemistocyticAstrocytoma>
      rdf:type owl:Class ;
      rdfs:comment "A gemistocytic presence in the context of of known astrocytoma is a indication of cancer progression and a worsening prognosis for the patient."^^xsd:string ;
      rdfs:subClassOf <http://mdacc.org/ClinicalLatha#CancerProgressionIndicator> ;
      label:correspondsTo label:GemistocyticAstrocytoma_NCIURI ;
      label:designNote "This concept is extensible."^^xsd:string , "This concept is directly related to the Gemistocytic Astrocytoma concept in NCI Thesaurus."^^xsd:string , "This concept may have instances of it's own or may be a superclass for concept refinements."^^xsd:string ;
      dc:creator foaf:JimLomax .

<http://mdacc.org/ClinicalLatha#Gender>
      rdf:type owl:Class ;
      rdfs:comment "Human gender"^^xsd:string ;
      rdfs:subClassOf <http://mdacc.org/ClinicalLatha#PopulationCharacteristic> ;
      rdfs:subClassOf
              [ rdf:type owl:Restriction ;
                owl:onProperty skos-xl:prefLabel ;
                owl:someValuesFrom label:GenderLabel
              ] ;
      label:correspondsTo label:Gender_NCIURI ;
      label:designNote "This concept directly corresponds  to the concept of Gender in NCI Thesaurus."^^xsd:string ;
      dc:creator foaf:JimLomax .

<http://mdacc.org/ClinicalLatha#GeneralAnaplasia_AnaplasiaFinding>
      rdf:type <http://mdacc.org/ClinicalLatha#AnaplasiaFinding> ;
      rdfs:comment "Anaplasia that is cannot be classificed as focal or diffuse"^^xsd:string ;
      label:correspondsTo label:Anaplasia_MESHURI ;
      label:designNote "This concept directly corresponds to the Anaplasia concept in MESH"^^xsd:string ;
      dc:creator foaf:JimLomax ;
      skos-xl:prefLabel label:Anaplasia_AnaplasiaLabel .

<http://mdacc.org/ClinicalLatha#GeneralCancerProgression_CancerProgressionDiagnosis>
      rdf:type <http://mdacc.org/ClinicalLatha#CancerProgressionDiagnosis> ;
      <http://mdacc.org/ClinicalLatha#indicates>
              <http://mdacc.org/ClinicalLatha#GeneralTumorProgression_TumorProgressionFinding> .

<http://mdacc.org/ClinicalLatha#GeneralTumorProgression_TumorProgressionFinding>
      rdf:type <http://mdacc.org/ClinicalLatha#TumorProgressionFinding> ;
      temporal:dateTime "2010-12-14"^^xsd:string .

<http://mdacc.org/ClinicalLatha#GiantCellGlioblastoma>
      rdf:type owl:Class ;
      rdfs:comment "A rare histological variant of glioblastoma (WHO grade IV) with a predominance of bizarre, multinucleated giant cells, an occasionally abundant stromal reticulin network, and a high frequency of TP53 mutations"^^xsd:string ;
      rdfs:subClassOf <http://mdacc.org/ClinicalLatha#Glioblastoma> ;
      label:correspondsTo label:GiantCellGlioblastoma_SNOMEDURI ;
      label:designNote "This concept is extensible."^^xsd:string , "This concept is directly related to the Giant Cell Glioblastoma concept in SNOMED."^^xsd:string , "This concept may have instances of it's own or may be a superclass for concept refinements."^^xsd:string ;
      dc:creator foaf:JimLomax .

<http://mdacc.org/ClinicalLatha#GleasonScoringForProstateCancer>
      rdf:type owl:Class ;
      rdfs:comment "The score derived from universally embraced prostate cancer grading system developed by Dr. Donald F. Gleason in 1977. The system provides a reproducible description of the glandular architecture of prostate tissue to which a pathologist assigns a score depending primarily on the microscopic patterns of cancerous glands and cell morphology. The system correlates well with behavior at the extremes: Gleason 1+1 tumors are the most well differentiated, slowly growing and rarely spread; Gleason 4+5 tumors are the most poorly differentiated, often widely metastatic at the time of diagnosis. In the commoner intermediate grade tumors, however, behavior is extremely variable."^^xsd:string ;
      rdfs:subClassOf <http://mdacc.org/ClinicalLatha#DiseaseScoringSystem> ;
      label:correspondsTo label:GleasonScoringForProstateCancer_NCIURI ;
      label:designNote "This concept may demoted to instance"^^xsd:string , "This concept is directly related to the concept ofGleason Scoring System for Prostrate Cancer in NCI Thesaurus"^^xsd:string ;
      dc:creator foaf:JimLomax .

<http://mdacc.org/ClinicalLatha#GlialCell>
      rdf:type owl:Class ;
      rdfs:comment "The non-neuronal cells of the nervous system. They not only provide physical support, but also respond to injury, regulate the ionic and chemical composition of the extracellular milieu, participate in the blood-brain and blood-retina barriers, form the myelin insulation of nervous pathways, guide neuronal migration during development, and exchange metabolites with neurons."^^xsd:string ;
      rdfs:subClassOf <http://mdacc.org/ClinicalLatha#Cell> ;
      rdfs:subClassOf
              [ rdf:type owl:Restriction ;
                owl:onProperty <http://mdacc.org/ClinicalLatha#anatomicLocation> ;
                owl:someValuesFrom <http://mdacc.org/ClinicalLatha#BrainAnatomicSite>
              ] ;
      label:correspondsTo label:GlialCell_NCIURI ;
      label:designNote "This concept is extensible."^^xsd:string , "All glial cells are located in the brain."^^xsd:string , "This concept is directly related to the Glial Cell concept in NCI Thesaurus"^^xsd:string , "This concept may have instances of it's own or may be a superclass for concept refinements."^^xsd:string ;
      dc:creator foaf:JimLomax .

<http://mdacc.org/ClinicalLatha#GlialFibrillaryAcideicProtein_Indicator>
      rdf:type <http://mdacc.org/ClinicalLatha#CancerProgressionIndicator> , <http://mdacc.org/ClinicalLatha#Protein> , <http://mdacc.org/ClinicalLatha#TumorMarker> ;
      label:correspondsTo label:GFAP_NCIURI ;
      label:creator foaf:JimLomax ;
      label:designNote "This concept is directly related to the Glial Fibrillary Acideic Protein concept in NCI Thesaurus."^^xsd:string ;
      skos-xl:prefLabel label:GlialFibrillaryAcideicProtein_IndicatorLabel .

<http://mdacc.org/ClinicalLatha#Glioblastoma>
      rdf:type owl:Class ;
      rdfs:comment "The most malignant astrocytic tumor (WHO grade IV). It is composed of poorly differentiated neoplastic astrocytes and it is characterized by the presence of cellular polymorphism, nuclear atypia, brisk mitotic activity, vascular thrombosis, microvascular proliferation and necrosis. It typically affects adults and is preferentially located in the cerebral hemispheres. It may develop from diffuse astrocytoma WHO grade II or anaplastic astrocytoma (secondary glioblastoma), but more frequently, it manifests after a short clinical history de novo, without evidence of a less malignant precursor lesion (primary glioblastoma). Two histologic variants are recognized: giant cell glioblastoma and gliosarcoma"^^xsd:string ;
      rdfs:subClassOf <http://mdacc.org/ClinicalLatha#Glioma> ;
      rdfs:subClassOf
              [ rdf:type owl:Restriction ;
                owl:onProperty skos-xl:prefLabel ;
                owl:someValuesFrom label:GlioblastomaDiseaseLabel
              ] ;
      label:correspondsTo label:Glioblastoma_SNOMEDURI ;
      label:designNote "This concept is extensible."^^xsd:string , "This concept is directly related to the Glioblastoma concept in SNOMED."^^xsd:string , "This concept may have instances of it's own or may be a superclass for concept refinements."^^xsd:string ;
      dc:creator foaf:JimLomax .

<http://mdacc.org/ClinicalLatha#GlioblastomaMultiforme_Glioblastoma>
      rdf:type <http://mdacc.org/ClinicalLatha#Glioblastoma> ;
      <http://mdacc.org/ClinicalLatha#anatomicLocation>
              <http://mdacc.org/ClinicalLatha#Brain_BrainAnatomicSite> ;
      <http://mdacc.org/ClinicalLatha#manifestedBy>
              <http://mdacc.org/ClinicalLatha#BrainCancer_BrainCancer> ;
      skos-xl:prefLabel label:GlioblastomaMulitforme_BrainTumorLabel .

<http://mdacc.org/ClinicalLatha#GlioblastomaWithOligodendroglialComponent>
      rdf:type owl:Class ;
      rdfs:subClassOf <http://mdacc.org/ClinicalLatha#Oligodendroglioma> ;
      rdfs:subClassOf
              [ rdf:type owl:Restriction ;
                owl:onProperty <http://mdacc.org/ClinicalLatha#exhibitsTumorMorphology> ;
                owl:someValuesFrom <http://mdacc.org/ClinicalLatha#Glioblastoma>
              ] ;
      label:designNote "This concept has no known corresponding concept in BioPortal."^^xsd:string ;
      dc:creator foaf:JimLomax .

<http://mdacc.org/ClinicalLatha#Glioblastoma_Glioblastoma>
      rdf:type <http://mdacc.org/ClinicalLatha#Glioblastoma> ;
      <http://mdacc.org/ClinicalLatha#anatomicLocation>
              <http://mdacc.org/ClinicalLatha#Brain_BrainAnatomicSite> ;
      <http://mdacc.org/ClinicalLatha#manifestedBy>
              <http://mdacc.org/ClinicalLatha#BrainCancer_BrainCancer> ;
      label:creator foaf:JimLomax ;
      label:designNote "This instance of Glioblastoma  represents a diagnosis of Glioblastoma with no further details."^^xsd:string .

<http://mdacc.org/ClinicalLatha#Glioma>
      rdf:type owl:Class ;
      rdfs:comment "A benign or malignant brain and spinal cord tumor that arises from glial cells (astrocytes, oligodendrocytes, ependymal cells)."^^xsd:string ;
      rdfs:subClassOf <http://mdacc.org/ClinicalLatha#TumorType> ;
      rdfs:subClassOf
              [ rdf:type owl:Restriction ;
                owl:onProperty <http://mdacc.org/ClinicalLatha#anatomicLocation> ;
                owl:someValuesFrom <http://mdacc.org/ClinicalLatha#BrainAnatomicSite>
              ] ;
      label:correspondsTo label:Glioma_NCIURI ;
      label:designNote "This concept is extensible."^^xsd:string , "This concept is directly related to the Neuroglial Tumor concept in NCI Thesaurus."^^xsd:string , "This concept may have instances of it's own or may be a superclass for concept refinements."^^xsd:string ;
      dc:creator foaf:JimLomax .

<http://mdacc.org/ClinicalLatha#Gliosarcoma>
      rdf:type owl:Class ;
      rdfs:comment "A rare histological variant of glioblastoma (WHO grade IV) characterized by a biphasic tissue pattern with alternating areas displaying glial and mesenchymal differentiation (WHO). It is associated with the molecular abnormalities seen in primary and secondary glioblastomas, except for the amplification of EGFR."^^xsd:string ;
      rdfs:subClassOf <http://mdacc.org/ClinicalLatha#Glioblastoma> ;
      label:correspondsTo label:Gliosarcoma_SNOMEDURI ;
      label:designNote "This concept is extensible."^^xsd:string , "This concept is directly related to thel Gliosarcoma concept in SNOMED."^^xsd:string , "This concept may have instances of it's own or may be a superclass for concept refinements."^^xsd:string ;
      dc:creator foaf:JimLomax .

<http://mdacc.org/ClinicalLatha#Grams_WeightUnits>
      rdf:type <http://mdacc.org/ClinicalLatha#WeightUnits> ;
      <http://mdacc.org/ClinicalLatha#value>
              "Grams"^^xsd:string .

<http://mdacc.org/ClinicalLatha#GranularLeukocyte>
      rdf:type owl:Class ;
      rdfs:subClassOf <http://mdacc.org/ClinicalLatha#Leukocyte> ;
      label:creator foaf:JimLomax ;
      owl:equivalentClass <http://mdacc.org/ClinicalLatha#Granulocyte> .

<http://mdacc.org/ClinicalLatha#Granulocyte>
      rdf:type owl:Class ;
      rdfs:subClassOf <http://mdacc.org/ClinicalLatha#Leukocyte> ;
      label:correspondsTo label:Granulocyte_NCIURI ;
      label:creator foaf:JimLomax ;
      label:designNote "This concept is extensible."^^xsd:string , "This concept may have instances of it's own or may be a superclass for concept refinements  (neutrophils, eosinophil, basophil)."^^xsd:string , "This concept is directly related to the Granulocyte concept in NCI Thesaurus"^^xsd:string .

<http://mdacc.org/ClinicalLatha#Gray44_RadiationDosage>
      rdf:type <http://mdacc.org/ClinicalLatha#RadiationDosage> ;
      <http://mdacc.org/ClinicalLatha#units>
              <http://mdacc.org/ClinicalLatha#Gray_DosageUnits> ;
      <http://mdacc.org/ClinicalLatha#value>
              "44"^^xsd:string .

<http://mdacc.org/ClinicalLatha#Gray_DosageUnits>
      rdf:type <http://mdacc.org/ClinicalLatha#RadiationDosageUnits> ;
      skos-xl:prefLabel label:Gray_UnitsLabel .

<http://mdacc.org/ClinicalLatha#HeadAnatomicSite>
      rdf:type owl:Class ;
      rdfs:subClassOf <http://mdacc.org/ClinicalLatha#AnatomicSite> ;
      label:designNote "This concept may have specific instances"^^xsd:string , "This concept is extensible; more specific anatomic location within the head."^^xsd:string ;
      dc:creator foaf:JimLomax .

<http://mdacc.org/ClinicalLatha#HeadAndNeckCancer>
      rdf:type owl:Class ;
      rdfs:subClassOf <http://mdacc.org/ClinicalLatha#Cancer> ;
      rdfs:subClassOf
              [ rdf:type owl:Restriction ;
                owl:onProperty <http://mdacc.org/ClinicalLatha#anatomicLocation> ;
                owl:someValuesFrom
                        [ rdf:type owl:Class ;
                          owl:unionOf (<http://mdacc.org/ClinicalLatha#HeadAnatomicSite> <http://mdacc.org/ClinicalLatha#NeckAnatomicSite>)
                        ]
              ] ;
      label:creator foaf:JimLomax .

<http://mdacc.org/ClinicalLatha#HeadAndNeckCancer_HeadAndNeckCancer>
      rdf:type <http://mdacc.org/ClinicalLatha#HeadAndNeckCancer> ;
      <http://mdacc.org/ClinicalLatha#anatomicLocation>
              <http://mdacc.org/ClinicalLatha#Head_HeadAnatomicSite> , <http://mdacc.org/ClinicalLatha#Neck_NeckAnatomicSite> ;
      label:creator foaf:JimLomax ;
      skos-xl:prefLabel label:HeadAndNeckCancer_HeadAndNeckDiseaseLabel .

<http://mdacc.org/ClinicalLatha#HeadAndNeckCarcinoma_HeadAndNeckTumor>
      rdf:type <http://mdacc.org/ClinicalLatha#HeadAndNeckTumor> ;
      <http://mdacc.org/ClinicalLatha#anatomicLocation>
              <http://mdacc.org/ClinicalLatha#Head_HeadAnatomicSite> , <http://mdacc.org/ClinicalLatha#Neck_NeckAnatomicSite> ;
      <http://mdacc.org/ClinicalLatha#manifestedBy>
              <http://mdacc.org/ClinicalLatha#HeadAndNeckCancer_HeadAndNeckCancer> ;
      label:correspondsTo label:HeadAndNeckCarcinoma_NCIURI ;
      label:creator foaf:JimLomax ;
      skos-xl:prefLabel label:HeadAndNeckCarcinoma_HeadAndNeckTumorLabel .

<http://mdacc.org/ClinicalLatha#HeadAndNeckSquamousCellCarcinoma_HeadAndNeckTumor>
      rdf:type <http://mdacc.org/ClinicalLatha#HeadAndNeckTumor> ;
      <http://mdacc.org/ClinicalLatha#anatomicLocation>
              <http://mdacc.org/ClinicalLatha#Head_HeadAnatomicSite> , <http://mdacc.org/ClinicalLatha#Neck_NeckAnatomicSite> ;
      <http://mdacc.org/ClinicalLatha#manifestedBy>
              <http://mdacc.org/ClinicalLatha#HeadAndNeckCancer_HeadAndNeckCancer> ;
      label:correspondsTo label:HeadAndNeckSquamousCellCarcinoma_NCIURI ;
      label:creator foaf:JimLomax ;
      skos-xl:prefLabel label:HeadAndNeckSquamousCellCarcinoma_HeadAndNeckTumorLabel .

<http://mdacc.org/ClinicalLatha#HeadAndNeckTumor>
      rdf:type owl:Class ;
      rdfs:comment "Tumor anatomically located within the colon"^^xsd:string ;
      rdfs:subClassOf <http://mdacc.org/ClinicalLatha#TumorType> ;
      rdfs:subClassOf
              [ rdf:type owl:Restriction ;
                owl:onProperty <http://mdacc.org/ClinicalLatha#anatomicLocation> ;
                owl:someValuesFrom <http://mdacc.org/ClinicalLatha#ColonAnatomicSite>
              ] ;
      label:designNote "This concept is extensible."^^xsd:string , "This concept may have instances of it's own or may be a superclass for concept refinements."^^xsd:string ;
      dc:creator foaf:JimLomax .

<http://mdacc.org/ClinicalLatha#Head_HeadAnatomicSite>
      rdf:type <http://mdacc.org/ClinicalLatha#HeadAnatomicSite> ;
      label:creator foaf:JimLomax ;
      skos-xl:prefLabel label:Head_AnatomicSiteLabel .

<http://mdacc.org/ClinicalLatha#HepatocellularCarcinoma_LiverTumor>
      rdf:type <http://mdacc.org/ClinicalLatha#LiverTumor> ;
      <http://mdacc.org/ClinicalLatha#anatomicLocation>
              <http://mdacc.org/ClinicalLatha#Liver_LiverAnatomicSite> ;
      <http://mdacc.org/ClinicalLatha#manifestedBy>
              <http://mdacc.org/ClinicalLatha#LiverCancer_LiverCancer> ;
      label:correspondsTo label:HepatocellularCarcinoma_NCIURI ;
      label:creator foaf:JimLomax ;
      skos-xl:prefLabel label:HepatocellularCarcinoma_LiverTumorLabel .

<http://mdacc.org/ClinicalLatha#HispanicOrLatino_Ethnicity>
      rdf:type <http://mdacc.org/ClinicalLatha#Ethnicity> ;
      label:creator foaf:JimLomax ;
      label:designNote "This concept is specific to TCGA"^^xsd:string ;
      skos-xl:prefLabel label:HispanicLatino_EthnicityLabel .

<http://mdacc.org/ClinicalLatha#Hispanic_Ethnicity>
      rdf:type <http://mdacc.org/ClinicalLatha#Ethnicity> ;
      label:correspondsTo label:Hispanic_NCIURI ;
      label:creator foaf:JimLomax ;
      label:designNote "This concept directly corresponds to the Hispanic concept in NCI Thesaurus."^^xsd:string ;
      skos-xl:prefLabel label:Hispanic_EthnicityLabel .

<http://mdacc.org/ClinicalLatha#Histiocyte_Macrophage>
      rdf:type <http://mdacc.org/ClinicalLatha#Macrophage> ;
      label:correspondsTo label:Histiocyte_NCIURI ;
      label:creator foaf:JimLomax ;
      skos-xl:prefLabel label:Histiocyte_BioMaterialLabel .

<http://mdacc.org/ClinicalLatha#HistologicGrade>
      rdf:type owl:Class ;
      rdfs:comment "The degree of abnormality of cancer cells, a measure of differentiation, the extent to which cancer cells are similar in appearance and function to healthy cells of the same tissue type. The degree of differentiation often relates to the clinical behavior of the particular tumor. Based on the microscopic findings, tumor grade is commonly described by one of four degrees of severity. Histopathologic grade of a tumor may be used to plan treatment and estimate the future course, outcome, and overall prognosis of disease. Certain types of cancers, such as soft tissue sarcoma, primary brain tumors, lymphomas, and breast have special grading systems"^^xsd:string ;
      rdfs:subClassOf <http://mdacc.org/ClinicalLatha#DiseaseScoringSystem> , skos:Concept ;
      rdfs:subClassOf
              [ rdf:type owl:Restriction ;
                owl:onProperty skos-xl:prefLabel ;
                owl:someValuesFrom label:HistologicalGradeLabel
              ] ;
      label:correspondsTo label:HistologicGrade_NCIURI ;
      label:designNote "This concept is extensible."^^xsd:string , "This concept is directly related to the concept of Histological Grade in NCI Thesaurus"^^xsd:string , "This concept may have instances of it's own or may be a superclass for concept refinements."^^xsd:string ;
      dc:creator foaf:JimLomax .

<http://mdacc.org/ClinicalLatha#HistologicType>
      rdf:type owl:Class ;
      rdfs:comment "Refers to the type of tissue in which a tumor originated."^^xsd:string ;
      rdfs:subClassOf skos:Concept , <http://mdacc.org/ClinicalLatha#ClinicalPackage> ;
      rdfs:subClassOf
              [ rdf:type owl:Restriction ;
                owl:onProperty skos-xl:prefLabel ;
                owl:someValuesFrom label:HistologicTypeLabel
              ] ;
      label:correspondsTo label:HistologicType_NCIURI ;
      label:designNote "This concept is extensible."^^xsd:string , "This concept is directly related to the Histological Type concept in NCI Thesaurus."^^xsd:string , "This concept may have instances of it's own or may be a superclass for concept refinements."^^xsd:string ;
      dc:creator foaf:JimLomax .

<http://mdacc.org/ClinicalLatha#ImageFormat>
      rdf:type owl:Class ;
      rdfs:comment "Storage format for an electronic image. Storage formats are produced by image compression algorithms."^^xsd:string ;
      rdfs:subClassOf skos:Concept ;
      dc:creator foaf:JimLomax .

<http://mdacc.org/ClinicalLatha#Immortalization>
      rdf:type owl:Class ;
      rdfs:comment "Laboratory methods used to generate cells that are able to reproduce indefinitely."^^xsd:string ;
      rdfs:subClassOf <http://mdacc.org/ClinicalLatha#LabProcedure> ;
      label:correspondsTo label:Immortalization_NCIURI ;
      label:designNote "This concept is extensible."^^xsd:string , "This concept is directly related to the Immortalization concept in NCI Thesaurus."^^xsd:string , "This concept may have instances of it's own or may be a superclass for concept refinements."^^xsd:string ;
      dc:creator foaf:JimLomax .

<http://mdacc.org/ClinicalLatha#ImmortalizedBCell>
      rdf:type owl:Class ;
      rdfs:comment "There is no corresponding concept in Bioportal"^^xsd:string , "B cells that are not limited by the Hayflick limit; where cells no longer divide because of DNA damage or shortened telomeres."^^xsd:string ;
      rdfs:subClassOf <http://mdacc.org/ClinicalLatha#BCell> ;
      rdfs:subClassOf
              [ rdf:type owl:Restriction ;
                owl:onProperty <http://mdacc.org/ClinicalLatha#immortalizingAgent> ;
                owl:someValuesFrom <http://mdacc.org/ClinicalLatha#Virus>
              ] ;
      rdfs:subClassOf
              [ rdf:type owl:Restriction ;
                owl:onProperty <http://mdacc.org/ClinicalLatha#transformedBy> ;
                owl:someValuesFrom <http://mdacc.org/ClinicalLatha#Immortalization>
              ] ;
      label:designNote "An immortalized B Cell is one that has been transformed by an immortalization process and agent"^^xsd:string , "This concept may have instances of it's own or may be a superclass for concept refinements."^^xsd:string ;
      dc:creator foaf:JimLomax .

<http://mdacc.org/ClinicalLatha#Immunotherapy>
      rdf:type owl:Class ;
      rdfs:comment "Therapy designed to induce changes in a patient's immune status in order to treat disease."^^xsd:string ;
      rdfs:subClassOf <http://mdacc.org/ClinicalLatha#DrugTherapy> ;
      rdfs:subClassOf
              [ rdf:type owl:Restriction ;
                owl:onProperty <http://mdacc.org/ClinicalLatha#administersTherapeuticAgent> ;
                owl:someValuesFrom <http://mdacc.org/Drug#ImmunotherapyDrug>
              ] ;
      label:correspondsTo label:Immunotherapy_NCIURI ;
      label:designNote "This concept is extensible."^^xsd:string , "This concept is directly related to the Immunotherapy concept in NCI Thesaurus."^^xsd:string , "This concept may have instances of it's own or may be a superclass for concept refinements."^^xsd:string ;
      dc:creator foaf:JimLomax .

<http://mdacc.org/ClinicalLatha#ImplantRadiationTherapy>
      rdf:type owl:Class ;
      rdfs:subClassOf <http://mdacc.org/ClinicalLatha#RadiationTherapy> ;
      label:designNote "This concept is extensible."^^xsd:string , "This concept may have instances of it's own or may be a superclass for concept refinements."^^xsd:string ;
      dc:creator foaf:JimLomax .

<http://mdacc.org/ClinicalLatha#ImplantsRadiation>
      rdf:type owl:Class ;
      rdfs:subClassOf <http://mdacc.org/Drug#Radiation> .

<http://mdacc.org/ClinicalLatha#IncisionBioposy_DiagnosticProcedure>
      rdf:type <http://mdacc.org/ClinicalLatha#DiagnosticProcedure> ;
      label:creator foaf:JimLomax ;
      skos-xl:prefLabel label:IncisionBiopsy_DiagnosticProcedureLabel .

<http://mdacc.org/ClinicalLatha#Indicator>
      rdf:type owl:Class ;
      rdfs:comment "An event, entity or condition that typically characterizes a prescribed environment or situation and determines or aids in determining whether certain stated circumstances exist or criteria are satisfied."^^xsd:string ;
      rdfs:subClassOf skos:Concept , <http://mdacc.org/ClinicalLatha#ClinicalPackage> ;
      rdfs:subClassOf
              [ rdf:type owl:Restriction ;
                owl:onProperty <http://mdacc.org/ClinicalLatha#indicates> ;
                owl:someValuesFrom owl:Thing
              ] ;
      rdfs:subClassOf
              [ rdf:type owl:Restriction ;
                owl:onProperty skos-xl:prefLabel ;
                owl:someValuesFrom label:IndicatorLabel
              ] ;
      label:correspondsTo label:Indicator_NCIURI ;
      label:designNote "This concept is extensible."^^xsd:string , "An indicator must indicate something; cinical condition, disease, prognosis, diagnosis are all possible subjects."^^xsd:string , "This concept is directly related to the Indicator concept in NCI Thesaurus."^^xsd:string , "This concept may have instances of it's own or may be a superclass for concept refinements."^^xsd:string ;
      dc:creator foaf:JimLomax .

<http://mdacc.org/ClinicalLatha#InformedConsentVerifiedExistentialEvent>
      rdf:type owl:Class ;
      rdfs:comment "In a TCGA context this represents if the patient can signed out a informed consent document and that signature has been verfied."^^xsd:string ;
      rdfs:subClassOf <http://mdacc.org/ClinicalLatha#ExistentialEvent> ;
      label:designNote "This concept may be demoted to an instance"^^xsd:string , "There is no corresponding concept in BioPortal"^^xsd:string , "This is a TCGA specific entity; should be replaced with the content of a Informed Consent, rather than a reordation of its existence."^^xsd:string ;
      dc:creator foaf:JimLomax .

<http://mdacc.org/ClinicalLatha#InitialCourseExistentialEvent>
      rdf:type owl:Class ;
      rdfs:subClassOf <http://mdacc.org/ClinicalLatha#ExistentialEvent> ;
      dc:creator foaf:JimLomax .

<http://mdacc.org/ClinicalLatha#InstantEvent_StartRegularChemo>
      rdf:type time-entry:InstantEvent ;
      time-entry:durationDescriptionOf
              <http://mdacc.org/ClinicalLatha#DurationDescription_30Days> .

<http://mdacc.org/ClinicalLatha#InstantThingPair_1>
      rdf:type time-entry:InstantThingPair ;
      time-entry:firstInstantThing
              <http://mdacc.org/ClinicalLatha#Patient1Birth_Instant> .

<http://mdacc.org/ClinicalLatha#Interval_StartStopChemoRegular>
      rdf:type time-entry:Interval ;
      time-entry:durationDescriptionOf
              <http://mdacc.org/ClinicalLatha#DurationDescription_30Days> .

<http://mdacc.org/ClinicalLatha#IntraPeritoneal_TherapeuticAgentDelivery>
      rdf:type <http://mdacc.org/ClinicalLatha#TherapeuticAgentDelivery> ;
      skos-xl:prefLabel label:IntraPeritoneal_TherapeuticAgentDeliveryLabel .

<http://mdacc.org/ClinicalLatha#Intratumoral_TherapeuticAgentDelivery>
      rdf:type <http://mdacc.org/ClinicalLatha#TherapeuticAgentDelivery> ;
      skos-xl:prefLabel label:Intratumoral_TherapeuticAgentDeliveryLabel .

<http://mdacc.org/ClinicalLatha#Intravenous_TherapeuticAgentDelivery>
      rdf:type <http://mdacc.org/ClinicalLatha#TherapeuticAgentDelivery> ;
      skos-xl:prefLabel label:Intravenous_TherapeuticAgentDeliveryLabel .

<http://mdacc.org/ClinicalLatha#JPG>
      rdf:type <http://mdacc.org/ClinicalLatha#ImageFormat> .

<http://mdacc.org/ClinicalLatha#JewishOrigin>
      rdf:type owl:Class ;
      rdfs:comment "In a TCGA context Jewish Orgin represents the patient's jewish orging type, if any. Ashkenazi, Sephardic"^^xsd:string ;
      rdfs:subClassOf <http://mdacc.org/ClinicalLatha#PopulationCharacteristic> ;
      label:designNote "There is no concept of Jewish Origin in BioPortal"^^xsd:string ;
      dc:creator foaf:JimLomax .

<http://mdacc.org/ClinicalLatha#KidneyAnatomicSite>
      rdf:type owl:Class ;
      rdfs:subClassOf <http://mdacc.org/ClinicalLatha#AnatomicSite> ;
      label:designNote "This concept may have specific instances"^^xsd:string , "This concept is extensible; more specific anatomic location within the kidney."^^xsd:string ;
      dc:creator foaf:JimLomax .

<http://mdacc.org/ClinicalLatha#KidneyCancer>
      rdf:type owl:Class ;
      rdfs:subClassOf <http://mdacc.org/ClinicalLatha#Cancer> ;
      rdfs:subClassOf
              [ rdf:type owl:Restriction ;
                owl:onProperty <http://mdacc.org/ClinicalLatha#anatomicLocation> ;
                owl:someValuesFrom <http://mdacc.org/ClinicalLatha#KidneyAnatomicSite>
              ] ;
      label:creator foaf:JimLomax .

<http://mdacc.org/ClinicalLatha#KidneyTumor>
      rdf:type owl:Class ;
      rdfs:comment "Tumor anatomically located within the kidney"^^xsd:string ;
      rdfs:subClassOf <http://mdacc.org/ClinicalLatha#TumorType> ;
      rdfs:subClassOf
              [ rdf:type owl:Restriction ;
                owl:onProperty <http://mdacc.org/ClinicalLatha#anatomicLocation> ;
                owl:someValuesFrom <http://mdacc.org/ClinicalLatha#KidneyAnatomicSite>
              ] ;
      label:designNote "This concept is extensible."^^xsd:string , "This concept may have instances of it's own or may be a superclass for concept refinements."^^xsd:string ;
      dc:creator foaf:JimLomax .

<http://mdacc.org/ClinicalLatha#Kidney_KidneyAnatomicSite>
      rdf:type <http://mdacc.org/ClinicalLatha#KidneyAnatomicSite> ;
      label:creator foaf:JimLomax ;
      skos-xl:prefLabel label:Head_AnatomicSiteLabel .

<http://mdacc.org/ClinicalLatha#Kidney_KidneyCancer>
      rdf:type <http://mdacc.org/ClinicalLatha#KidneyCancer> ;
      <http://mdacc.org/ClinicalLatha#anatomicLocation>
              <http://mdacc.org/ClinicalLatha#Kidney_KidneyAnatomicSite> ;
      label:creator foaf:JimLomax ;
      skos-xl:prefLabel label:KidneyCancer_KidneyDiseaseLabel .

<http://mdacc.org/ClinicalLatha#LabProcedure>
      rdf:type owl:Class ;
      rdfs:comment "Any procedure that involves testing or manipulating a sample of blood, urine, or other body substance in a laboratory setting."^^xsd:string ;
      rdfs:subClassOf skos:Concept , <http://mdacc.org/ClinicalLatha#ClinicalPackage> ;
      rdfs:subClassOf
              [ rdf:type owl:Restriction ;
                owl:onProperty skos-xl:prefLabel ;
                owl:someValuesFrom label:LabProcedureLabel
              ] ;
      label:correspondsTo label:LabProcedure_NCIURI ;
      label:designNote "This concept is extensible."^^xsd:string , "This concept is directly related to the LabProcedure concept in NCI Thesaurus."^^xsd:string , "This concept may have instances of it's own or may be a superclass for concept refinements."^^xsd:string ;
      dc:creator foaf:JimLomax .

<http://mdacc.org/ClinicalLatha#LabProcedureExecution>
      rdf:type owl:Class ;
      rdfs:comment "The execution of a lab  procedure. An instance of a lab procedure only describes the  procedure itself, not the execution of the procedure."^^xsd:string ;
      rdfs:subClassOf skos:Concept , <http://mdacc.org/ClinicalLatha#ClinicalPackage> ;
      rdfs:subClassOf
              [ rdf:type owl:Restriction ;
                owl:onProperty <http://mdacc.org/ClinicalLatha#labProcedure> ;
                owl:someValuesFrom <http://mdacc.org/ClinicalLatha#LabProcedure>
              ] ;
      rdfs:subClassOf
              [ rdf:type owl:Restriction ;
                owl:onProperty skos-xl:prefLabel ;
                owl:someValuesFrom label:LabProcedureLabel
              ] ;
      label:designNote "There is no corresponding concept in BioPortal"^^xsd:string ;
      dc:creator foaf:JimLomax .

<http://mdacc.org/ClinicalLatha#LeftCerebralHemisphere_BrainAnatomicSite>
      rdf:type <http://mdacc.org/ClinicalLatha#BrainAnatomicSite> ;
      label:correspondsTo label:LeftCerebralHemisphere_NCIURI ;
      label:creator foaf:JimLomax ;
      skos-xl:prefLabel label:LeftCerebralHemisphere_AnatomicSiteLabel .

<http://mdacc.org/ClinicalLatha#LeftLung_LungAnatomicSite>
      rdf:type <http://mdacc.org/ClinicalLatha#LungAnatomicSite> ;
      <http://mdacc.org/ClinicalLatha#side>
              <http://mdacc.org/ClinicalLatha#Left_Side> ;
      label:correspondsTo label:LeftLung_NCIURI ;
      label:creator foaf:JimLomax ;
      skos-xl:prefLabel label:LeftLung_AnatomicSiteLabel .

<http://mdacc.org/ClinicalLatha#LeftOvary_OvaryAnatomicSite>
      rdf:type <http://mdacc.org/ClinicalLatha#OvaryAnatomicSite> ;
      <http://mdacc.org/ClinicalLatha#side>
              <http://mdacc.org/ClinicalLatha#Left_Side> ;
      label:creator foaf:JimLomax ;
      skos-xl:prefLabel label:LeftOvary_OvaryLabel .

<http://mdacc.org/ClinicalLatha#Left_Side>
      rdf:type <http://mdacc.org/ClinicalLatha#Side> ;
      label:creator foaf:JimLomax ;
      skos-xl:prefLabel label:Left_SideLabel .

<http://mdacc.org/ClinicalLatha#LengthUnits>
      rdf:type owl:Class ;
      rdfs:subClassOf <http://mdacc.org/ClinicalLatha#Units> ;
      label:creator foaf:JimLomax .

<http://mdacc.org/ClinicalLatha#Leptomeninges>
      rdf:type owl:Class ;
      rdfs:comment "The two innermost layers of tissue that cover the brain and spinal cord, the arachnoid mater and the pia mater."^^xsd:string ;
      rdfs:subClassOf <http://mdacc.org/ClinicalLatha#BrainMembrane> ;
      label:correspondsTo label:Leptomeninges_NCIURI ;
      label:designNote "We cannot find reason to further refine this concept, only add instances."^^xsd:string , "This concept is directly related to the Leptomeninges concept in NCI Thesaurus."^^xsd:string ;
      dc:creator foaf:JimLomax .

<http://mdacc.org/ClinicalLatha#LeptomeningialInvolvedTumor>
      rdf:type owl:Class ;
      rdfs:comment "Tumor growth on the thin sheet or layer of pliable tissue, serving as a covering or envelope of a part, as the lining of a cavity, as a partition or septum, or to connect two structures."^^xsd:string ;
      rdfs:subClassOf <http://mdacc.org/ClinicalLatha#TumorType> ;
      rdfs:subClassOf
              [ rdf:type owl:Restriction ;
                owl:onProperty <http://mdacc.org/ClinicalLatha#anatomicLocation> ;
                owl:someValuesFrom <http://mdacc.org/ClinicalLatha#Leptomeninges>
              ] ;
      label:designNote "This concept has no known corresponding concept in BioPortal"^^xsd:string ;
      dc:creator foaf:JimLomax .

<http://mdacc.org/ClinicalLatha#Leukemia>
      rdf:type owl:Class ;
      rdfs:comment "A malignant (clonal) hematologic disorder, involving hematopoietic stem cells and characterized by the presence of primitive or atypical myeloid or lymphoid cells in the bone marrow and the blood. Leukemias are classified as acute or chronic based on the degree of cellular differentiation and the predominant cell type present. Leukemia is usually associated with anemia, fever, hemorrhagic episodes, and splenomegaly. Common leukemias include acute myeloid leukemia, chronic myelogenous leukemia, acute lymphoblastic or precursor lymphoblastic leukemia, and chronic lymphocytic leukemia. Treatment is vital to patient survival; untreated, the natural course of acute leukemias is normally measured in weeks or months, while that of chronic leukemias is more often measured in months or years."^^xsd:string ;
      rdfs:subClassOf <http://mdacc.org/ClinicalLatha#Cancer> ;
      label:correspondsTo label:Leukemia_NCIURI ;
      label:creator foaf:JimLomax .

<http://mdacc.org/ClinicalLatha#Leukocyte>
      rdf:type owl:Class ;
      rdfs:comment "White blood cells. These include granular leukocytes (basophils; eosinophils; and neutrophils) as well as non-granular leukocytes (lymphocytes and monocytes)."^^xsd:string ;
      rdfs:subClassOf <http://mdacc.org/ClinicalLatha#Cell> ;
      label:correspondsTo label:Leukocyte_MESHURI ;
      label:designNote "This concept is extensible."^^xsd:string , "This concept is directly related to the Leukocyte concept in MESH"^^xsd:string , "This concept may have instances of it's own or may be a superclass for concept refinements."^^xsd:string ;
      dc:creator foaf:JimLomax .

<http://mdacc.org/ClinicalLatha#Liposarcoma>
      rdf:type owl:Class ;
      rdfs:subClassOf <http://mdacc.org/ClinicalLatha#TumorType> ;
      label:correspondsTo label:Liposarcoma_NCIURI ;
      label:creator foaf:JimLomax .

<http://mdacc.org/ClinicalLatha#Liposarcoma_Liposarcoma>
      rdf:type <http://mdacc.org/ClinicalLatha#Liposarcoma> ;
      rdfs:comment "A usually painless malignant tumor that arises from adipose tissue. Microscopically, it may contain a spectrum of neoplastic adipocytes ranging from lipoblasts to pleomorphic malignant adipocytes. Representative morphologic variants include: well differentiated, dedifferentiated, pleomorphic, and myxoid/round cell liposarcoma. The metastatic potential is higher in less differentiated tumors."^^xsd:string ;
      label:correspondsTo label:Liposarcoma_NCIURI ;
      label:creator foaf:JimLomax ;
      skos-xl:prefLabel label:Liposarcoma_LiposarcomaTumorLabel .

<http://mdacc.org/ClinicalLatha#LiverAnatomicSite>
      rdf:type owl:Class ;
      rdfs:subClassOf <http://mdacc.org/ClinicalLatha#AnatomicSite> ;
      label:correspondsTo label:Liver_NCIURI ;
      label:designNote "This concept is extensible; more specific anatomic location within the liver."^^xsd:string , "This concept is directly related to the Liver concept in NCI Thesaurus."^^xsd:string ;
      dc:creator foaf:JimLomax .

<http://mdacc.org/ClinicalLatha#LiverCancer>
      rdf:type owl:Class ;
      rdfs:subClassOf <http://mdacc.org/ClinicalLatha#Cancer> ;
      rdfs:subClassOf
              [ rdf:type owl:Restriction ;
                owl:onProperty <http://mdacc.org/ClinicalLatha#anatomicLocation> ;
                owl:someValuesFrom <http://mdacc.org/ClinicalLatha#LiverAnatomicSite>
              ] ;
      label:creator foaf:JimLomax .

<http://mdacc.org/ClinicalLatha#LiverCancer_LiverCancer>
      rdf:type <http://mdacc.org/ClinicalLatha#LiverCancer> ;
      <http://mdacc.org/ClinicalLatha#anatomicLocation>
              <http://mdacc.org/ClinicalLatha#Liver_LiverAnatomicSite> ;
      label:creator foaf:JimLomax ;
      skos-xl:prefLabel label:LiverCancer_LiverDiseaseLabel .

<http://mdacc.org/ClinicalLatha#LiverTumor>
      rdf:type owl:Class ;
      rdfs:comment "Tumor anatomically located within the Liver"^^xsd:string ;
      rdfs:subClassOf <http://mdacc.org/ClinicalLatha#TumorType> ;
      rdfs:subClassOf
              [ rdf:type owl:Restriction ;
                owl:onProperty <http://mdacc.org/ClinicalLatha#anatomicLocation> ;
                owl:someValuesFrom <http://mdacc.org/ClinicalLatha#LiverAnatomicSite>
              ] ;
      label:designNote "This concept is extensible."^^xsd:string , "This concept may have instances of it's own or may be a superclass for concept refinements."^^xsd:string ;
      dc:creator foaf:JimLomax .

<http://mdacc.org/ClinicalLatha#Liver_LiverAnatomicSite>
      rdf:type <http://mdacc.org/ClinicalLatha#LiverAnatomicSite> ;
      label:creator foaf:JimLomax ;
      skos-xl:prefLabel label:Liver_AnatomicSiteLabel .

<http://mdacc.org/ClinicalLatha#Living_VitalStatus>
      rdf:type <http://mdacc.org/ClinicalLatha#VitalStatus> ;
      label:correspondsTo label:Life_NCIURI ;
      label:creator foaf:JimLomax ;
      label:designNote "This concept directly corresponds to the Life concept in NCI Thesuarus"^^xsd:string .

<http://mdacc.org/ClinicalLatha#LungAdenocarcinoma_LungTumor>
      rdf:type <http://mdacc.org/ClinicalLatha#LungTumor> ;
      <http://mdacc.org/ClinicalLatha#anatomicLocation>
              <http://mdacc.org/ClinicalLatha#Lung_LungAnatomicSite> ;
      <http://mdacc.org/ClinicalLatha#manifestedBy>
              <http://mdacc.org/ClinicalLatha#LungCancer_LungCancer> ;
      label:correspondsTo label:LungAdenocarcinoma_NCIURI ;
      label:creator foaf:JimLomax ;
      skos-xl:prefLabel label:LungAdenocarcinoma_LungTumorLabel .

<http://mdacc.org/ClinicalLatha#LungAnatomicSite>
      rdf:type owl:Class ;
      rdfs:comment "One of a pair of viscera occupying the pulmonary cavities of the thorax, the organs of respiration in which aeration of the blood takes place. As a rule, the right lung is slightly larger than the left and is divided into three lobes (an upper, a middle, and a lower or basal), while the left has two lobes (an upper and a lower or basal). Each lung is irregularly conical in shape, presenting a blunt upper extremity (the apex), a concave base following the curve of the diaphragm, an outer convex surface (costal surface), an inner or mediastinal surface (mediastinal surface), a thin and sharp anterior border, and a thick and rounded posterior border."^^xsd:string ;
      rdfs:subClassOf <http://mdacc.org/ClinicalLatha#AnatomicSite> ;
      label:correspondsTo label:Lung_NCIURI ;
      label:designNote "This concept may have specific instances; (left lung, right lung) as an example."^^xsd:string , "This concept is extensible; more specific anatomic location within the lung."^^xsd:string , "This concept is directly related to the Lung concept in NCI Thesaurus."^^xsd:string ;
      dc:creator foaf:JimLomax .

<http://mdacc.org/ClinicalLatha#LungCancer>
      rdf:type owl:Class ;
      rdfs:subClassOf <http://mdacc.org/ClinicalLatha#Cancer> ;
      rdfs:subClassOf
              [ rdf:type owl:Restriction ;
                owl:onProperty <http://mdacc.org/ClinicalLatha#anatomicLocation> ;
                owl:someValuesFrom <http://mdacc.org/ClinicalLatha#LungAnatomicSite>
              ] ;
      label:creator foaf:JimLomax .

<http://mdacc.org/ClinicalLatha#LungCancer_LungCancer>
      rdf:type <http://mdacc.org/ClinicalLatha#LungCancer> ;
      <http://mdacc.org/ClinicalLatha#anatomicLocation>
              <http://mdacc.org/ClinicalLatha#Lung_LungAnatomicSite> ;
      label:correspondsTo label:LungCarcinoma_NCIURI ;
      label:creator foaf:JimLomax ;
      skos-xl:prefLabel label:LungCancer_LungDiseaseLabel .

<http://mdacc.org/ClinicalLatha#LungSlide>
      rdf:type owl:Class ;
      rdfs:subClassOf <http://mdacc.org/ClinicalLatha#Slide> ;
      rdfs:subClassOf
              [ rdf:type owl:Restriction ;
                owl:onProperty <http://mdacc.org/ClinicalLatha#tumorOrigin> ;
                owl:someValuesFrom <http://mdacc.org/ClinicalLatha#LungTumor>
              ] ;
      label:architect foaf:MoSanyang ;
      label:creator foaf:JimLomax ;
      label:developer foaf:PradheepRaju , foaf:DawitGebremichael .

<http://mdacc.org/ClinicalLatha#LungSmallCellCarcinoma_LungTumor>
      rdf:type <http://mdacc.org/ClinicalLatha#LungTumor> ;
      <http://mdacc.org/ClinicalLatha#anatomicLocation>
              <http://mdacc.org/ClinicalLatha#Lung_LungAnatomicSite> ;
      <http://mdacc.org/ClinicalLatha#manifestedBy>
              <http://mdacc.org/ClinicalLatha#LungCancer_LungCancer> ;
      label:correspondsTo label:LungSmallCellCarcinoma_NCIURI ;
      label:creator foaf:JimLomax ;
      skos-xl:prefLabel label:LungSmallCellCarcinoma_LungTumorLabel .

<http://mdacc.org/ClinicalLatha#LungTumor>
      rdf:type owl:Class ;
      rdfs:comment "Tumor anatomically located within the Lung"^^xsd:string ;
      rdfs:subClassOf <http://mdacc.org/ClinicalLatha#TumorType> ;
      rdfs:subClassOf
              [ rdf:type owl:Restriction ;
                owl:onProperty <http://mdacc.org/ClinicalLatha#anatomicLocation> ;
                owl:someValuesFrom <http://mdacc.org/ClinicalLatha#LungAnatomicSite>
              ] ;
      label:designNote "This concept is extensible."^^xsd:string , "This concept may have instances of it's own or may be a superclass for concept refinements."^^xsd:string ;
      dc:creator foaf:JimLomax .

<http://mdacc.org/ClinicalLatha#LungTumor_LungTumor>
      rdf:type <http://mdacc.org/ClinicalLatha#LungTumor> ;
      rdfs:comment "Generalization instance of lung tumor"^^xsd:string ;
      <http://mdacc.org/ClinicalLatha#anatomicLocation>
              <http://mdacc.org/ClinicalLatha#Lung_LungAnatomicSite> ;
      <http://mdacc.org/ClinicalLatha#manifestedBy>
              <http://mdacc.org/ClinicalLatha#LungCancer_LungCancer> ;
      label:creator foaf:JimLomax .

<http://mdacc.org/ClinicalLatha#Lung_LungAnatomicSite>
      rdf:type <http://mdacc.org/ClinicalLatha#LungAnatomicSite> ;
      label:correspondsTo label:Lung_NCIURI ;
      label:creator foaf:JimLomax ;
      skos-xl:prefLabel label:Lung_AnatomicSiteLabel .

<http://mdacc.org/ClinicalLatha#Lymphocyte>
      rdf:type owl:Class ;
      rdfs:comment "White blood cells formed in the body's lymphoid tissue. The nucleus is round or ovoid with coarse, irregularly clumped chromatin while the cytoplasm is typically pale blue with azurophilic (if any) granules. Most lymphocytes can be classified as either T or B (with subpopulations of each), or natural killer cells."^^xsd:string ;
      rdfs:subClassOf <http://mdacc.org/ClinicalLatha#Leukocyte> ;
      label:correspondsTo label:Lymphocyte_MESHURI ;
      label:designNote "This concept may have instances of it's own or may be a superclass for concept refinements  (B-Cell, T-Cell)."^^xsd:string , "This concept is extensible."^^xsd:string , "This concept is directly related to the Lymphocyte concept in MESH"^^xsd:string ;
      dc:creator foaf:JimLomax .

<http://mdacc.org/ClinicalLatha#LymphocyticNeoplasm_LymphoidCancer>
      rdf:type <http://mdacc.org/ClinicalLatha#LymphoidCancer> ;
      label:correspondsTo label:LymphocyticNeoplasm_NCIURI ;
      label:creator foaf:JimLomax ;
      skos-xl:prefLabel label:LymphocyticNeoplasm_LymphocyticCancerDiseaseLabel .

<http://mdacc.org/ClinicalLatha#LymphoidCancer>
      rdf:type owl:Class ;
      rdfs:subClassOf <http://mdacc.org/ClinicalLatha#Cancer> ;
      label:correspondsTo label:LymphoidCancer_NCIURI ;
      label:creator foaf:JimLomax .

<http://mdacc.org/ClinicalLatha#MDA_OV_Stage0_PathologicDistantMetastasisTNMFinding>
      rdf:type <http://mdacc.org/ClinicalLatha#Stage0_PathologicDistantMetastasisTNMFinding> ;
      rdfs:comment """ No distant metastases are found (this excludes peritoneal metastasis).
"""^^xsd:string ;
      <http://mdacc.org/ClinicalLatha#code>
              "M0"^^xsd:string ;
      <http://mdacc.org/ClinicalLatha#tnmScheme>
              <http://mdacc.org/ClinicalLatha#MDA_TNMOvarianNeoplasmStagingSystem> ;
      dc:creator foaf:JimLomax .

<http://mdacc.org/ClinicalLatha#MDA_OV_Stage0_PathologicPrimaryTumorTNMFinding>
      rdf:type <http://mdacc.org/ClinicalLatha#Stage0_PathologicPrimaryTumorTNMFinding> ;
      rdfs:comment "No primary tumor identified"^^xsd:string ;
      <http://mdacc.org/ClinicalLatha#code>
              "T0"^^xsd:string ;
      <http://mdacc.org/ClinicalLatha#tnmScheme>
              <http://mdacc.org/ClinicalLatha#MDA_TNMOvarianNeoplasmStagingSystem> ;
      dc:creator foaf:JimLomax .

<http://mdacc.org/ClinicalLatha#MDA_OV_Stage0_PathologicRegionalLymphNodesTNMFinding>
      rdf:type <http://mdacc.org/ClinicalLatha#Stage0_PathologicRegionalLymphNodesTNMFinding> ;
      rdfs:comment "Regional lymph nodes contain no metastases."^^xsd:string ;
      <http://mdacc.org/ClinicalLatha#code>
              "N0"^^xsd:string ;
      <http://mdacc.org/ClinicalLatha#tnmScheme>
              <http://mdacc.org/ClinicalLatha#MDA_TNMOvarianNeoplasmStagingSystem> ;
      dc:creator foaf:JimLomax .

<http://mdacc.org/ClinicalLatha#MDA_OV_Stage1_PathologicDistantMetastasisTNMFinding>
      rdf:type <http://mdacc.org/ClinicalLatha#Stage1_PathologicDistantMetastasisTNMFinding> ;
      rdfs:comment "Distant metastases are present."^^xsd:string ;
      <http://mdacc.org/ClinicalLatha#code>
              "M1"^^xsd:string ;
      <http://mdacc.org/ClinicalLatha#tnmScheme>
              <http://mdacc.org/ClinicalLatha#MDA_TNMOvarianNeoplasmStagingSystem> ;
      dc:creator foaf:JimLomax .

<http://mdacc.org/ClinicalLatha#MDA_OV_Stage1_PathologicPrimaryTumorTNMFinding>
      rdf:type <http://mdacc.org/ClinicalLatha#Stage1_PathologicPrimaryTumorTNMFinding> ;
      rdfs:comment "Tumor is limited to one or both ovaries."^^xsd:string ;
      <http://mdacc.org/ClinicalLatha#code>
              "T1"^^xsd:string ;
      <http://mdacc.org/ClinicalLatha#tnmScheme>
              <http://mdacc.org/ClinicalLatha#MDA_TNMOvarianNeoplasmStagingSystem> ;
      dc:creator foaf:JimLomax .

<http://mdacc.org/ClinicalLatha#MDA_OV_Stage1_PathologicRegionalLymphNodesTNMFinding>
      rdf:type <http://mdacc.org/ClinicalLatha#Stage1_PathologicRegionalLymphNodesTNMFinding> ;
      rdfs:comment "Evidence of lymph node metastasis. "^^xsd:string ;
      <http://mdacc.org/ClinicalLatha#code>
              "N1"^^xsd:string ;
      <http://mdacc.org/ClinicalLatha#tnmScheme>
              <http://mdacc.org/ClinicalLatha#MDA_TNMOvarianNeoplasmStagingSystem> ;
      dc:creator foaf:JimLomax .

<http://mdacc.org/ClinicalLatha#MDA_OV_Stage1a_PathologicPrimaryTumorTNMFinding>
      rdf:type <http://mdacc.org/ClinicalLatha#Stage1a_PathologicPrimaryTumorTNMFinding> ;
      rdfs:comment "Tumor is limited to one ovary. The capsule, or outer wall of the tumor, is intact, there is no tumor on the ovarian surface, and there are no cancer cells in ascites (abdominal fluid build-up) or peritoneal lavage (\"washings\" from the abdominal cavity). "^^xsd:string ;
      <http://mdacc.org/ClinicalLatha#code>
              "T1a"^^xsd:string ;
      <http://mdacc.org/ClinicalLatha#tnmScheme>
              <http://mdacc.org/ClinicalLatha#MDA_TNMOvarianNeoplasmStagingSystem> ;
      dc:creator foaf:JimLomax .

<http://mdacc.org/ClinicalLatha#MDA_OV_Stage1b_PathologicPrimaryTumorTNMFinding>
      rdf:type <http://mdacc.org/ClinicalLatha#Stage1b_PathologicPrimaryTumorTNMFinding> ;
      rdfs:comment "Tumor is limited to both ovaries. The capsule is intact, there is no tumor on the ovarian surface, and there are no cancer cells in ascites or peritoneal lavage. "^^xsd:string ;
      <http://mdacc.org/ClinicalLatha#code>
              "T1b"^^xsd:string ;
      <http://mdacc.org/ClinicalLatha#tnmScheme>
              <http://mdacc.org/ClinicalLatha#MDA_TNMOvarianNeoplasmStagingSystem> ;
      dc:creator foaf:JimLomax .

<http://mdacc.org/ClinicalLatha#MDA_OV_Stage1c_PathologicPrimaryTumorTNMFinding>
      rdf:type <http://mdacc.org/ClinicalLatha#Stage1c_PathologicPrimaryTumorTNMFinding> ;
      rdfs:comment "Tumor is limited to one or both ovaries with any of the following: ruptured capsule (burst outer wall of the tumor), tumor on ovarian surface, or cancer cells in the ascites or peritoneal lavage. "^^xsd:string ;
      <http://mdacc.org/ClinicalLatha#code>
              "T1c"^^xsd:string ;
      <http://mdacc.org/ClinicalLatha#tnmScheme>
              <http://mdacc.org/ClinicalLatha#MDA_TNMOvarianNeoplasmStagingSystem> ;
      dc:creator foaf:JimLomax .

<http://mdacc.org/ClinicalLatha#MDA_OV_Stage2_PathologicPrimaryTumorTNMFinding>
      rdf:type <http://mdacc.org/ClinicalLatha#Stage2_PathologicPrimaryTumorTNMFinding> ;
      rdfs:comment "Tumor involves one or both ovaries with spread into the pelvis. "^^xsd:string ;
      <http://mdacc.org/ClinicalLatha#code>
              "T2"^^xsd:string ;
      <http://mdacc.org/ClinicalLatha#tnmScheme>
              <http://mdacc.org/ClinicalLatha#MDA_TNMOvarianNeoplasmStagingSystem> ;
      dc:creator foaf:JimLomax .

<http://mdacc.org/ClinicalLatha#MDA_OV_Stage2a_PathologicPrimaryTumorTNMFinding>
      rdf:type <http://mdacc.org/ClinicalLatha#Stage2a_PathologicPrimaryTumorTNMFinding> ;
      rdfs:comment "Tumor has spread and/or attaches to the uterus and/or fallopian tubes. There are no cancer cells in ascites or peritoneal lavage. "^^xsd:string ;
      <http://mdacc.org/ClinicalLatha#code>
              "T2a"^^xsd:string ;
      <http://mdacc.org/ClinicalLatha#tnmScheme>
              <http://mdacc.org/ClinicalLatha#MDA_TNMOvarianNeoplasmStagingSystem> ;
      dc:creator foaf:JimLomax .

<http://mdacc.org/ClinicalLatha#MDA_OV_Stage2b_PathologicPrimaryTumorTNMFinding>
      rdf:type <http://mdacc.org/ClinicalLatha#Stage2b_PathologicPrimaryTumorTNMFinding> ;
      rdfs:comment "Tumor has spread to other pelvic tissues. There are no cancer cells in ascites or peritoneal lavage. "^^xsd:string ;
      <http://mdacc.org/ClinicalLatha#code>
              "T2b"^^xsd:string ;
      <http://mdacc.org/ClinicalLatha#tnmScheme>
              <http://mdacc.org/ClinicalLatha#MDA_TNMOvarianNeoplasmStagingSystem> ;
      dc:creator foaf:JimLomax .

<http://mdacc.org/ClinicalLatha#MDA_OV_Stage2c_PathologicPrimaryTumorTNMFinding>
      rdf:type <http://mdacc.org/ClinicalLatha#Stage2c_PathologicPrimaryTumorTNMFinding> ;
      rdfs:comment "Tumor has spread to pelvic tissues, with cancer cells in ascites or peritoneal lavage. "^^xsd:string ;
      <http://mdacc.org/ClinicalLatha#code>
              "T2c"^^xsd:string ;
      <http://mdacc.org/ClinicalLatha#tnmScheme>
              <http://mdacc.org/ClinicalLatha#MDA_TNMOvarianNeoplasmStagingSystem> ;
      dc:creator foaf:JimLomax .

<http://mdacc.org/ClinicalLatha#MDA_OV_Stage3_PathologicPrimaryTumorTNMFinding>
      rdf:type <http://mdacc.org/ClinicalLatha#Stage3_PathologicPrimaryTumorTNMFinding> ;
      rdfs:comment "Tumor involves one or both ovaries, with microscopically confirmed peritoneal metastasis outside the pelvis and/or metastasis to regional (nearby) lymph node(s). "^^xsd:string ;
      <http://mdacc.org/ClinicalLatha#code>
              "T3"^^xsd:string ;
      <http://mdacc.org/ClinicalLatha#tnmScheme>
              <http://mdacc.org/ClinicalLatha#MDA_TNMOvarianNeoplasmStagingSystem> ;
      dc:creator foaf:JimLomax .

<http://mdacc.org/ClinicalLatha#MDA_OV_Stage3a_PathologicPrimaryTumorTNMFinding>
      rdf:type <http://mdacc.org/ClinicalLatha#Stage3a_PathologicPrimaryTumorTNMFinding> ;
      rdfs:comment "Microscopic peritoneal metastasis beyond the pelvis. "^^xsd:string ;
      <http://mdacc.org/ClinicalLatha#code>
              "T3a"^^xsd:string ;
      <http://mdacc.org/ClinicalLatha#tnmScheme>
              <http://mdacc.org/ClinicalLatha#MDA_TNMOvarianNeoplasmStagingSystem> ;
      dc:creator foaf:JimLomax .

<http://mdacc.org/ClinicalLatha#MDA_OV_Stage3b_PathologicPrimaryTumorTNMFinding>
      rdf:type <http://mdacc.org/ClinicalLatha#Stage3b_PathologicPrimaryTumorTNMFinding> ;
      rdfs:comment "Macroscopic (visible to the naked eye) peritoneal metastasis beyond the pelvis, 2 cm or less in greatest dimension. "^^xsd:string ;
      <http://mdacc.org/ClinicalLatha#code>
              "T3b"^^xsd:string ;
      <http://mdacc.org/ClinicalLatha#tnmScheme>
              <http://mdacc.org/ClinicalLatha#MDA_TNMOvarianNeoplasmStagingSystem> ;
      dc:creator foaf:JimLomax .

<http://mdacc.org/ClinicalLatha#MDA_OV_Stage3c_PathologicPrimaryTumorTNMFinding>
      rdf:type <http://mdacc.org/ClinicalLatha#Stage3c_PathologicPrimaryTumorTNMFinding> ;
      rdfs:comment "Peritoneal metastasis beyond the pelvis, more than 2 cm in greatest dimension. "^^xsd:string ;
      <http://mdacc.org/ClinicalLatha#code>
              "T3c"^^xsd:string ;
      <http://mdacc.org/ClinicalLatha#tnmScheme>
              <http://mdacc.org/ClinicalLatha#MDA_TNMOvarianNeoplasmStagingSystem> ;
      dc:creator foaf:JimLomax .

<http://mdacc.org/ClinicalLatha#MDA_Stage0TMNOVTumorStage>
      rdf:type <http://mdacc.org/ClinicalLatha#Stage0TMNOVTumorStage> ;
      <http://mdacc.org/ClinicalLatha#cancer>
              <http://mdacc.org/ClinicalLatha#OvarianCancer_OvarianCancer> ;
      <http://mdacc.org/ClinicalLatha#diseaseStagingSystem>
              <http://mdacc.org/ClinicalLatha#MDA_TNMOvarianNeoplasmStagingSystem> ;
      <http://mdacc.org/ClinicalLatha#finding>
              <http://mdacc.org/ClinicalLatha#MDA_OV_Stage0_PathologicPrimaryTumorTNMFinding> , <http://mdacc.org/ClinicalLatha#MDA_OV_Stage0_PathologicRegionalLymphNodesTNMFinding> , <http://mdacc.org/ClinicalLatha#MDA_OV_Stage0_PathologicDistantMetastasisTNMFinding> ;
      dc:identifier "0"^^xsd:string .

<http://mdacc.org/ClinicalLatha#MDA_Stage0_PathologicPrimaryTumorTNMFinding>
      rdf:type <http://mdacc.org/ClinicalLatha#Stage0_PathologicPrimaryTumorTNMFinding> ;
      <http://mdacc.org/ClinicalLatha#code>
              "pT0"^^xsd:string ;
      <http://mdacc.org/ClinicalLatha#tnmScheme>
              <http://mdacc.org/ClinicalLatha#MDA_TNMDiseaseStagingSystem> .

<http://mdacc.org/ClinicalLatha#MDA_Stage1_PathologicPrimaryTumorTNMFinding>
      rdf:type <http://mdacc.org/ClinicalLatha#Stage1_PathologicPrimaryTumorTNMFinding> ;
      <http://mdacc.org/ClinicalLatha#code>
              "pT1"^^xsd:string ;
      <http://mdacc.org/ClinicalLatha#tnmScheme>
              <http://mdacc.org/ClinicalLatha#MDA_TNMDiseaseStagingSystem> .

<http://mdacc.org/ClinicalLatha#MDA_Stage1a_PathologicPrimaryTumorTNMFinding>
      rdf:type <http://mdacc.org/ClinicalLatha#Stage1a_PathologicPrimaryTumorTNMFinding> ;
      <http://mdacc.org/ClinicalLatha#code>
              "pT1a"^^xsd:string ;
      <http://mdacc.org/ClinicalLatha#tnmScheme>
              <http://mdacc.org/ClinicalLatha#MDA_TNMDiseaseStagingSystem> .

<http://mdacc.org/ClinicalLatha#MDA_Stage1b_PathologicPrimaryTumorTNMFinding>
      rdf:type <http://mdacc.org/ClinicalLatha#Stage1b_PathologicPrimaryTumorTNMFinding> ;
      <http://mdacc.org/ClinicalLatha#code>
              "pT1b"^^xsd:string ;
      <http://mdacc.org/ClinicalLatha#tnmScheme>
              <http://mdacc.org/ClinicalLatha#MDA_TNMDiseaseStagingSystem> .

<http://mdacc.org/ClinicalLatha#MDA_Stage1c_PathologicPrimaryTumorTNMFinding>
      rdf:type <http://mdacc.org/ClinicalLatha#Stage1c_PathologicPrimaryTumorTNMFinding> ;
      <http://mdacc.org/ClinicalLatha#code>
              "pT1c"^^xsd:string ;
      <http://mdacc.org/ClinicalLatha#tnmScheme>
              <http://mdacc.org/ClinicalLatha#MDA_TNMDiseaseStagingSystem> .

<http://mdacc.org/ClinicalLatha#MDA_Stage2_PathologicPrimaryTumorTNMFinding>
      rdf:type <http://mdacc.org/ClinicalLatha#Stage2_PathologicPrimaryTumorTNMFinding> ;
      <http://mdacc.org/ClinicalLatha#code>
              "pT2"^^xsd:string ;
      <http://mdacc.org/ClinicalLatha#tnmScheme>
              <http://mdacc.org/ClinicalLatha#MDA_TNMDiseaseStagingSystem> .

<http://mdacc.org/ClinicalLatha#MDA_Stage2a_PathologicPrimaryTumorTNMFinding>
      rdf:type <http://mdacc.org/ClinicalLatha#Stage2a_PathologicPrimaryTumorTNMFinding> ;
      <http://mdacc.org/ClinicalLatha#code>
              "pT2a"^^xsd:string ;
      <http://mdacc.org/ClinicalLatha#tnmScheme>
              <http://mdacc.org/ClinicalLatha#MDA_TNMDiseaseStagingSystem> .

<http://mdacc.org/ClinicalLatha#MDA_Stage2b_PathologicPrimaryTumorTNMFinding>
      rdf:type <http://mdacc.org/ClinicalLatha#Stage2b_PathologicPrimaryTumorTNMFinding> ;
      <http://mdacc.org/ClinicalLatha#code>
              "pT2b"^^xsd:string ;
      <http://mdacc.org/ClinicalLatha#tnmScheme>
              <http://mdacc.org/ClinicalLatha#MDA_TNMDiseaseStagingSystem> .

<http://mdacc.org/ClinicalLatha#MDA_Stage2c_PathologicPrimaryTumorTNMFinding>
      rdf:type <http://mdacc.org/ClinicalLatha#Stage2c_PathologicPrimaryTumorTNMFinding> ;
      <http://mdacc.org/ClinicalLatha#code>
              "pT2c"^^xsd:string ;
      <http://mdacc.org/ClinicalLatha#tnmScheme>
              <http://mdacc.org/ClinicalLatha#MDA_TNMDiseaseStagingSystem> .

<http://mdacc.org/ClinicalLatha#MDA_Stage3_PathologicPrimaryTumorTNMFinding>
      rdf:type <http://mdacc.org/ClinicalLatha#Stage3_PathologicPrimaryTumorTNMFinding> ;
      <http://mdacc.org/ClinicalLatha#code>
              "pT3"^^xsd:string ;
      <http://mdacc.org/ClinicalLatha#tnmScheme>
              <http://mdacc.org/ClinicalLatha#MDA_TNMDiseaseStagingSystem> .

<http://mdacc.org/ClinicalLatha#MDA_Stage3a_PathologicPrimaryTumorTNMFinding>
      rdf:type <http://mdacc.org/ClinicalLatha#Stage3a_PathologicPrimaryTumorTNMFinding> ;
      <http://mdacc.org/ClinicalLatha#code>
              "pT3a"^^xsd:string ;
      <http://mdacc.org/ClinicalLatha#tnmScheme>
              <http://mdacc.org/ClinicalLatha#MDA_TNMDiseaseStagingSystem> .

<http://mdacc.org/ClinicalLatha#MDA_Stage3b_PathologicPrimaryTumorTNMFinding>
      rdf:type <http://mdacc.org/ClinicalLatha#Stage3b_PathologicPrimaryTumorTNMFinding> ;
      <http://mdacc.org/ClinicalLatha#code>
              "pT3b"^^xsd:string ;
      <http://mdacc.org/ClinicalLatha#tnmScheme>
              <http://mdacc.org/ClinicalLatha#MDA_TNMDiseaseStagingSystem> .

<http://mdacc.org/ClinicalLatha#MDA_Stage3c_PathologicPrimaryTumorTNMFinding>
      rdf:type <http://mdacc.org/ClinicalLatha#Stage3c_PathologicPrimaryTumorTNMFinding> ;
      <http://mdacc.org/ClinicalLatha#code>
              "pT3c"^^xsd:string ;
      <http://mdacc.org/ClinicalLatha#tnmScheme>
              <http://mdacc.org/ClinicalLatha#MDA_TNMDiseaseStagingSystem> .

<http://mdacc.org/ClinicalLatha#MDA_Stage4_PathologicPrimaryTumorTNMFinding>
      rdf:type <http://mdacc.org/ClinicalLatha#Stage4_PathologicPrimaryTumorTNMFinding> ;
      <http://mdacc.org/ClinicalLatha#code>
              "pT4"^^xsd:string ;
      <http://mdacc.org/ClinicalLatha#tnmScheme>
              <http://mdacc.org/ClinicalLatha#MDA_TNMDiseaseStagingSystem> .

<http://mdacc.org/ClinicalLatha#MDA_Stage4a_PathologicPrimaryTumorTNMFinding>
      rdf:type <http://mdacc.org/ClinicalLatha#Stage4a_PathologicPrimaryTumorTNMFinding> ;
      <http://mdacc.org/ClinicalLatha#code>
              "pT4a"^^xsd:string ;
      <http://mdacc.org/ClinicalLatha#tnmScheme>
              <http://mdacc.org/ClinicalLatha#MDA_TNMDiseaseStagingSystem> .

<http://mdacc.org/ClinicalLatha#MDA_Stage4b_PathologicPrimaryTumorTNMFinding>
      rdf:type <http://mdacc.org/ClinicalLatha#Stage4b_PathologicPrimaryTumorTNMFinding> ;
      <http://mdacc.org/ClinicalLatha#code>
              "pT4b"^^xsd:string ;
      <http://mdacc.org/ClinicalLatha#tnmScheme>
              <http://mdacc.org/ClinicalLatha#MDA_TNMDiseaseStagingSystem> .

<http://mdacc.org/ClinicalLatha#MDA_Stage4c_PathologicPrimaryTumorTNMFinding>
      rdf:type <http://mdacc.org/ClinicalLatha#Stage4c_PathologicPrimaryTumorTNMFinding> ;
      <http://mdacc.org/ClinicalLatha#code>
              "pT4c"^^xsd:string ;
      <http://mdacc.org/ClinicalLatha#tnmScheme>
              <http://mdacc.org/ClinicalLatha#MDA_TNMDiseaseStagingSystem> .

<http://mdacc.org/ClinicalLatha#MDA_Stage4d_PathologicPrimaryTumorTNMFinding>
      rdf:type <http://mdacc.org/ClinicalLatha#Stage4d_PathologicPrimaryTumorTNMFinding> ;
      <http://mdacc.org/ClinicalLatha#code>
              "pT4d"^^xsd:string ;
      <http://mdacc.org/ClinicalLatha#tnmScheme>
              <http://mdacc.org/ClinicalLatha#MDA_TNMDiseaseStagingSystem> .

<http://mdacc.org/ClinicalLatha#MDA_TNMDiseaseStagingSystem>
      rdf:type <http://mdacc.org/ClinicalLatha#TNMDiseaseStagingSystem> .

<http://mdacc.org/ClinicalLatha#MDA_TNMOvarianNeoplasmStagingSystem>
      rdf:type <http://mdacc.org/ClinicalLatha#TNMOvarianNeoplasmStagingSystem> ;
      dc:creator foaf:JimLomax .

<http://mdacc.org/ClinicalLatha#MDAndersonBrainBankOwner>
      rdf:type mage:Person .

<http://mdacc.org/ClinicalLatha#MDAndersonBrainBankRepository>
      rdf:type mage:BioSourceProvider .

<http://mdacc.org/ClinicalLatha#Macrophage>
      rdf:type owl:Class ;
      rdfs:comment "The relatively long-lived phagocytic cell of mammalian tissues that are derived from blood monocytes. Main types are peritoneal macrophages; alveolar macrophages; histiocytes; kupffer cells of the liver; and osteoclasts. They may further differentiate within chronic inflammatory lesions to epitheliod cells or may fuse to form foreign body giant cells or langhans giant cells."^^xsd:string ;
      rdfs:subClassOf <http://mdacc.org/ClinicalLatha#ConnectiveTissueCell> ;
      label:correspondsTo label:Macrophage_MESHURI ;
      label:designNote "This concept is extensible."^^xsd:string , "This concept may have instances of it's own  or may be a superclass for concept refinements."^^xsd:string , "This concept is directly related to the Macrophage concept in MESH."^^xsd:string ;
      dc:creator foaf:JimLomax .

<http://mdacc.org/ClinicalLatha#Male_Gender>
      rdf:type <http://mdacc.org/ClinicalLatha#Gender> ;
      label:correspondsTo label:Male_NCIURI ;
      label:creator foaf:JimLomax ;
      label:designNote "This concept directly corresponds to the concept of Male in NCI Thesaurus."^^xsd:string .

<http://mdacc.org/ClinicalLatha#MalignantTumor>
      rdf:type owl:Class ;
      rdfs:comment "A tumor composed of atypical neoplastic, often pleomorphic cells that invade other tissues. Malignant neoplasms often metastasize to distant anatomic sites and may recur after excision. The most common malignant neoplasms are carcinomas (adenocarcinomas or squamous cell carcinomas), Hodgkin and non-Hodgkin lymphomas, leukemias, melanomas, and sarcomas."^^xsd:string ;
      rdfs:subClassOf <http://mdacc.org/ClinicalLatha#TumorType> ;
      label:correspondsTo label:MalignantTumor_NCIURI ;
      label:creator foaf:JimLomax ;
      label:designNote "This concept is extensible."^^xsd:string , "This concept is directly related to the Malignant Neoplasm concept in NCI Thesaurus."^^xsd:string , "This concept may have instances of it's own or may be a superclass for concept refinements."^^xsd:string .

<http://mdacc.org/ClinicalLatha#Malignant_MetastaticIndication>
      rdf:type <http://mdacc.org/ClinicalLatha#MetastaticIndication> ;
      skos-xl:prefLabel label:Malignant_MetastaticIndicationLabel .

<http://mdacc.org/ClinicalLatha#MastCell>
      rdf:type owl:Class ;
      rdfs:comment "Granulated cells that are found in almost all tissues, most abundantly in the skin and the gastrointestinal tract. Like the basophils, mast cells contain large amounts of histamine and heparin. Unlike basophils, mast cells normally remain in the tissues and do not circulate in the blood. Mast cells, derived from the bone marrow stem cells, are regulated by the stem cell factor."^^xsd:string ;
      rdfs:subClassOf <http://mdacc.org/ClinicalLatha#ConnectiveTissueCell> ;
      label:correspondsTo label:MastCell_MESHURI ;
      label:designNote "This concept is extensible."^^xsd:string , "This concept is directly related to the Mast Cell concept in MESH."^^xsd:string , "This concept may have instances of it's own  or may be a superclass for concept refinements."^^xsd:string ;
      dc:creator foaf:JimLomax .

<http://mdacc.org/ClinicalLatha#Membrane>
      rdf:type owl:Class ;
      rdfs:comment "A thin sheet or layer of pliable tissue, serving as a covering or envelope of a part, as the lining of a cavity, as a partition or septum, or to connect two structures."^^xsd:string ;
      rdfs:subClassOf <http://mdacc.org/ClinicalLatha#Tissue> ;
      label:correspondsTo label:Membrane_NCIURI ;
      label:designNote "This concept is directly related to the Membrane concept in NCI Thesaurus."^^xsd:string , "This concept is extensible; there are different types of membranes, each of which will have different properties."^^xsd:string , "This concept may have instances of it's own or may be a superclass for concept refinements."^^xsd:string ;
      dc:creator foaf:JimLomax .

<http://mdacc.org/ClinicalLatha#Meninges>
      rdf:type owl:Class ;
      rdfs:comment "A membrane that cover and protect the brain and spinal cord."^^xsd:string ;
      rdfs:subClassOf <http://mdacc.org/ClinicalLatha#BrainMembrane> ;
      label:correspondsTo label:Meninges_NCIURI ;
      label:designNote "We cannot find reason to further refine this concept, only add instances."^^xsd:string , "This concept is directly related to the Meninges concept in NCI Thesaurus."^^xsd:string ;
      dc:creator foaf:JimLomax .

<http://mdacc.org/ClinicalLatha#MetastaticIndication>
      rdf:type owl:Class ;
      rdfs:comment "An abnormal tissue growth resulted from uncontrolled cell proliferation"^^xsd:string ;
      rdfs:subClassOf skos:Concept , <http://mdacc.org/ClinicalLatha#ClinicalPackage> ;
      rdfs:subClassOf
              [ rdf:type owl:Restriction ;
                owl:onProperty skos-xl:prefLabel ;
                owl:someValuesFrom label:MetastaticIndicationLabel
              ] ;
      label:architect foaf:MoSanyang ;
      label:correspondsTo label:Neoplasm_NCIURI ;
      label:creator foaf:JimLomax ;
      label:designNote "Currently this is a TCGA specific concept"^^xsd:string ;
      label:developer foaf:PradheepRaju , foaf:JimLomax , foaf:DawitGebremichael .

<http://mdacc.org/ClinicalLatha#Metastatic_MetastaticIndication>
      rdf:type <http://mdacc.org/ClinicalLatha#MetastaticIndication> ;
      skos-xl:prefLabel label:Metatstatic_MetastaticIndicationLabel .

<http://mdacc.org/ClinicalLatha#MgM2_175_Dosage>
      rdf:type <http://mdacc.org/ClinicalLatha#DrugDosage> ;
      <http://mdacc.org/ClinicalLatha#units>
              <http://mdacc.org/ClinicalLatha#MgM2_DosageUnits> ;
      <http://mdacc.org/ClinicalLatha#value>
              "175"^^xsd:string .

<http://mdacc.org/ClinicalLatha#MgM2_DosageUnits>
      rdf:type <http://mdacc.org/ClinicalLatha#DrugDosageUnits> ;
      rdfs:comment "Also known as body surface area units. (milligrams per meters squared)"^^xsd:string ;
      skos-xl:prefLabel label:MgM2_UnitsLabel .

<http://mdacc.org/ClinicalLatha#Mg_DosageUnits>
      rdf:type <http://mdacc.org/ClinicalLatha#DrugDosageUnits> ;
      skos-xl:prefLabel label:Miligram_Abbr_UnitsLabel .

<http://mdacc.org/ClinicalLatha#Microplate>
      rdf:type owl:Class ;
      rdfs:comment "A Microplate is a piece of equipment containing physical subdivisions that are arrayed in a standard size, number and arrangement, each holds a small amount of substance."^^xsd:string ;
      rdfs:subClassOf <http://mdacc.org/ClinicalLatha#ScientificEquipment> , skos:Concept ;
      rdfs:subClassOf
              [ rdf:type owl:Restriction ;
                owl:onProperty skos-xl:prefLabel ;
                owl:someValuesFrom label:MicroplateLabel
              ] ;
      label:correspondsTo label:Microplate_NCIURI ;
      label:designNote "This concept is directly related to the Microplate  concept in NCI Thesaurus."^^xsd:string , "This concept may have instances of it's own or may be a superclass for concept refinements."^^xsd:string ;
      dc:creator foaf:JimLomax .

<http://mdacc.org/ClinicalLatha#Milliliter_VolumeUnits>
      rdf:type <http://mdacc.org/ClinicalLatha#VolumeUnits> ;
      skos-xl:prefLabel label:Millilter_UnitsLabel .

<http://mdacc.org/ClinicalLatha#MindBomb1Protein_Indicator>
      rdf:type <http://mdacc.org/ClinicalLatha#CancerProgressionIndicator> , <http://mdacc.org/ClinicalLatha#Protein> , <http://mdacc.org/ClinicalLatha#TumorMarker> ;
      label:correspondsTo label:MIB1_MESHURI ;
      label:creator foaf:JimLomax ;
      label:designNote "This concept is directly related to the MIB1 concept in NCI Thesaurus."^^xsd:string ;
      skos-xl:prefLabel label:MB1_IndicatorLabel .

<http://mdacc.org/ClinicalLatha#Molarity_ConcentrationUnits>
      rdf:type <http://mdacc.org/ClinicalLatha#ConcentrationUnits> .

<http://mdacc.org/ClinicalLatha#MouthAnatomicSite>
      rdf:type owl:Class ;
      rdfs:comment "LR:   This is part of Head and Neck cancer.  So do we have to link the 'Mouth' to 'Head' anatomic site"^^xsd:string , "Slitlike space in the oral cavity , bounded externally by the lips and cheek, and internally by the gingiva and teeth."^^xsd:string ;
      rdfs:subClassOf <http://mdacc.org/ClinicalLatha#AnatomicSite> ;
      label:correspondsTo label:Mouth_MESHURI ;
      label:designNote "This concept is extensible; more specific anatomic location within the mouth."^^xsd:string , "This concept may have specific instances."^^xsd:string , "This concept is directly related to the Mouth concept in MESH."^^xsd:string ;
      dc:creator foaf:JimLomax .

<http://mdacc.org/ClinicalLatha#Mucosa>
      rdf:type owl:Class ;
      rdfs:comment "The moist tissue that lines some organs and body cavities (such as the nose, mouth, lungs) and makes mucus (a thick, slippery fluid)."^^xsd:string ;
      rdfs:subClassOf <http://mdacc.org/ClinicalLatha#Membrane> ;
      label:correspondsTo label:Mucosa_NCIURI ;
      label:designNote "This concept is directly related to the Mucosa  concept in NCI Thesaurus."^^xsd:string , "This concept is extensible; there are different types of brain membranes each of which will have different properties."^^xsd:string , "This concept may have instances of it's own or may be a superclass for concept refinements."^^xsd:string ;
      dc:creator foaf:JimLomax .

<http://mdacc.org/ClinicalLatha#MuscleCell>
      rdf:type owl:Class ;
      rdfs:comment "Mature contractile cells, commonly known as myocytes, that form one of three kinds of muscle. The three types of muscle cells are skeletal (muscle fibers, skeletal), cardiac (myocytes, cardiac), and smooth (myocytes, smooth muscle). They are derived from embryonic (precursor) muscle cells called myoblasts."^^xsd:string ;
      rdfs:subClassOf <http://mdacc.org/ClinicalLatha#Cell> ;
      label:correspondsTo label:MuscleCell_MESHURI ;
      label:designNote "This concept is extensible."^^xsd:string , "This concept is directly related to the Muscle Cell concept in MESH"^^xsd:string , "This concept may have instances of it's own or may be a superclass for concept refinements."^^xsd:string ;
      dc:creator foaf:JimLomax .

<http://mdacc.org/ClinicalLatha#MuscleTissue>
      rdf:type owl:Class ;
      rdfs:comment "Contractile tissue that produces movement in animals."^^xsd:string ;
      rdfs:subClassOf <http://mdacc.org/ClinicalLatha#Tissue> ;
      rdfs:subClassOf
              [ rdf:type owl:Restriction ;
                owl:onProperty <http://mdacc.org/ClinicalLatha#composedOf> ;
                owl:someValuesFrom <http://mdacc.org/ClinicalLatha#MuscleCell>
              ] ;
      label:correspondsTo label:MuscleTissue_MESHURI ;
      label:designNote "This concept may have instances of it's own or may be a superclass for concept refinements."^^xsd:string , "This concept is directly related to the Muscle Tissue concept in MESH."^^xsd:string ;
      dc:creator foaf:JimLomax .

<http://mdacc.org/ClinicalLatha#Myeloma>
      rdf:type owl:Class ;
      rdfs:comment "Cancer that arises in plasma cells (white blood cells that produce antibodies)."^^xsd:string ;
      rdfs:subClassOf <http://mdacc.org/ClinicalLatha#TumorType> ;
      rdfs:subClassOf
              [ rdf:type owl:Restriction ;
                owl:onProperty <http://mdacc.org/ClinicalLatha#cellularDifferentiation> ;
                owl:someValuesFrom <http://mdacc.org/ClinicalLatha#PlasmaCell>
              ] ;
      label:correspondsTo label:PlasmaCellMyeloma_NCIURI ;
      label:designNote "This concept is extensible."^^xsd:string , "This concept is directly related to the Plasma Cell Myeloma concept in NCI Thesaurus."^^xsd:string , "This concept may have instances of it's own or may be a superclass for concept refinements."^^xsd:string ;
      dc:creator foaf:JimLomax .

<http://mdacc.org/ClinicalLatha#NativeHawaiianPacificIslander_Race>
      rdf:type <http://mdacc.org/ClinicalLatha#Race> ;
      label:correspondsTo label:NativeHawaiianPacificIslander_NCIURI ;
      label:designNote "This concept is directly related to the Native Hawaiian Pacific Isalnder Race concept in NCI Thesaurus."^^xsd:string ;
      dc:creator foaf:JimLomax .

<http://mdacc.org/ClinicalLatha#NeckAnatomicSite>
      rdf:type owl:Class ;
      rdfs:subClassOf <http://mdacc.org/ClinicalLatha#AnatomicSite> ;
      label:designNote "This concept may have specific instances"^^xsd:string , "This concept is extensible; more specific anatomic location within the head."^^xsd:string ;
      dc:creator foaf:JimLomax .

<http://mdacc.org/ClinicalLatha#Neck_NeckAnatomicSite>
      rdf:type <http://mdacc.org/ClinicalLatha#NeckAnatomicSite> ;
      label:creator foaf:JimLomax ;
      skos-xl:prefLabel label:Neck_AnatomicSiteLabel .

<http://mdacc.org/ClinicalLatha#Neoplasm>
      rdf:type owl:Class ;
      rdfs:comment "An abnormal tissue growth resulted from uncontrolled cell proliferation"^^xsd:string ;
      rdfs:subClassOf <http://mdacc.org/ClinicalLatha#ClinicalPackage> ;
      dc:creator foaf:JimLomax ;
      owl:equivalentClass <http://mdacc.org/ClinicalLatha#TumorType> .

<http://mdacc.org/ClinicalLatha#NeoplasticGrowthFinding>
      rdf:type owl:Class ;
      rdfs:comment "An abnormal tissue growth resulted from uncontrolled cell proliferation"^^xsd:string ;
      rdfs:subClassOf <http://mdacc.org/ClinicalLatha#Finding> ;
      label:correspondsTo label:NeoplasticGrowth_NCIURI ;
      label:designNote "This concept directly corresponds to the Neoplastic Growth Or Spread concept in NCI Thesaurus."^^xsd:string ;
      dc:creator foaf:JimLomax .

<http://mdacc.org/ClinicalLatha#NerveTissue>
      rdf:type owl:Class ;
      rdfs:subClassOf <http://mdacc.org/ClinicalLatha#Tissue> ;
      rdfs:subClassOf
              [ rdf:type owl:Restriction ;
                owl:onProperty <http://mdacc.org/ClinicalLatha#composedOf> ;
                owl:someValuesFrom
                        [ rdf:type owl:Class ;
                          owl:unionOf (<http://mdacc.org/ClinicalLatha#GlialCell> <http://mdacc.org/ClinicalLatha#Neuron>)
                        ]
              ] ;
      label:correspondsTo label:NerveTissue_MESHURI ;
      label:designNote "This concept is directly related to the Nerve Tissue concept in MESH."^^xsd:string , "This concept may have instances of it's own or may be a superclass for concept refinements."^^xsd:string ;
      dc:creator foaf:JimLomax .

<http://mdacc.org/ClinicalLatha#Neuron>
      rdf:type owl:Class ;
      rdfs:comment "The basic cellular units of nervous tissue. Each neuron consists of a body, an axon, and dendrites. Their purpose is to receive, conduct, and transmit impulses in the nervous system."^^xsd:string ;
      rdfs:subClassOf <http://mdacc.org/ClinicalLatha#Cell> ;
      label:correspondsTo label:Neuron_MESHURI ;
      label:designNote "This concept is extensible."^^xsd:string , "This concept is directly related to the Neuron concept in MESH"^^xsd:string , "This concept may have instances of it's own or may be a superclass for concept refinements."^^xsd:string ;
      dc:creator foaf:JimLomax .

<http://mdacc.org/ClinicalLatha#NonHodgkinsLymphoma_LymphoidCancer>
      rdf:type <http://mdacc.org/ClinicalLatha#LymphoidCancer> ;
      label:correspondsTo label:NonHodgkinsLymphoma_NCIURI ;
      label:creator foaf:JimLomax ;
      skos-xl:prefLabel label:NonHodgkinsLymphoma_LymphocyticCancerDiseaseLabel .

<http://mdacc.org/ClinicalLatha#NonMalignant_MetastaticIndication>
      rdf:type <http://mdacc.org/ClinicalLatha#MetastaticIndication> ;
      skos-xl:prefLabel label:NonMalignant_MetastaticIndicationLabel .

<http://mdacc.org/ClinicalLatha#NormalTumorGenotypeMatch>
      rdf:type owl:Class ;
      rdfs:comment "Indicates that there is a normal tissue sample and a tumor tissue sample from the same anatomical location for the same Patient"^^xsd:string ;
      rdfs:subClassOf <http://mdacc.org/ClinicalLatha#ClinicalPackage> ;
      label:designNote "This is a derived concept"^^xsd:string , "There is no corresponding concept in BioPortal"^^xsd:string .

<http://mdacc.org/ClinicalLatha#NotHispanicOrLatino_Ethnicity>
      rdf:type <http://mdacc.org/ClinicalLatha#Ethnicity> ;
      label:creator foaf:JimLomax ;
      label:designNote "This concept is specific to TCGA"^^xsd:string ;
      skos-xl:prefLabel label:NotHispanicLatino_EthnicityLabel .

<http://mdacc.org/ClinicalLatha#NuclearGrade>
      rdf:type owl:Class ;
      rdfs:comment "An evaluation of the size and shape of the nucleus in tumor cells and the percentage of tumor cells that are in the process of dividing or growing. Cancers with low nuclear grade grow and spread less quickly than cancers with high nuclear grade."^^xsd:string ;
      rdfs:subClassOf <http://mdacc.org/ClinicalLatha#DiseaseScoringSystem> , skos:Concept ;
      rdfs:subClassOf
              [ rdf:type owl:Restriction ;
                owl:onProperty skos-xl:prefLabel ;
                owl:someValuesFrom label:NuclearGradeLabel
              ] ;
      label:correspondsTo label:NuclearGrade_NCIURI ;
      label:designNote "This concept is extensible."^^xsd:string , "This concept is directly related to the concept of Nuclear Grade in NCI Thesaurus"^^xsd:string , "This concept may have instances of it's own or may be a superclass for concept refinements."^^xsd:string ;
      dc:creator foaf:JimLomax .

<http://mdacc.org/ClinicalLatha#Nucleus>
      rdf:type mage:CellularComponent .

<http://mdacc.org/ClinicalLatha#OVTumorStage>
      rdf:type owl:Class ;
      rdfs:subClassOf <http://mdacc.org/ClinicalLatha#TumorStage> ;
      rdfs:subClassOf
              [ rdf:type owl:Restriction ;
                owl:onProperty <http://mdacc.org/ClinicalLatha#cancer> ;
                owl:someValuesFrom <http://mdacc.org/ClinicalLatha#OvarianCancer>
              ] ;
      dc:creator foaf:JimLomax .

<http://mdacc.org/ClinicalLatha#Oligodendrocyte>
      rdf:type owl:Class ;
      rdfs:comment "A class of neuroglial (macroglial) cells in the central nervous system. Oligodendroglia may be called interfascicular, perivascular, or perineuronal satellite cells according to their location. The most important recognized function of these cells is the formation of the insulating myelin sheaths of axons in the central nervous system"^^xsd:string ;
      rdfs:subClassOf <http://mdacc.org/ClinicalLatha#GlialCell> ;
      label:correspondsTo label:Oligodendrocyte_NCIURI ;
      label:designNote "This concept is extensible."^^xsd:string , "This concept is directly related to the Oligodendrocyte concept in NCI Thesaurus"^^xsd:string , "This concept may have instances of it's own or may be a superclass for concept refinements."^^xsd:string ;
      dc:creator foaf:JimLomax .

<http://mdacc.org/ClinicalLatha#Oligodendroglioma>
      rdf:type owl:Class ;
      rdfs:comment "A well-differentiated (WHO grade II), diffusely infiltrating neuroglial tumor, typically located in the cerebral hemispheres. It is composed predominantly of cells which morphologically resemble oligodendroglia. The neoplastic cells have rounded homogeneous nuclei and, on paraffin sections, a swollen, clear cytoplasm "^^xsd:string ;
      rdfs:subClassOf <http://mdacc.org/ClinicalLatha#Glioma> ;
      rdfs:subClassOf
              [ rdf:type owl:Restriction ;
                owl:onProperty <http://mdacc.org/ClinicalLatha#cellularDifferentiation> ;
                owl:someValuesFrom <http://mdacc.org/ClinicalLatha#Oligodendrocyte>
              ] ;
      label:correspondsTo label:Oligodendroglioma_NCIURI ;
      label:designNote "This concept is extensible."^^xsd:string , "This concept is directly related to the Oligodendroglioma concept in SNOMED."^^xsd:string , "This concept may have instances of it's own or may be a superclass for concept refinements."^^xsd:string ;
      dc:creator foaf:JimLomax .

<http://mdacc.org/ClinicalLatha#OmentumAnatomicSite>
      rdf:type owl:Class ;
      rdfs:comment "A fold of peritoneum originating at the stomach and supporting the viscera."^^xsd:string ;
      rdfs:subClassOf <http://mdacc.org/ClinicalLatha#AnatomicSite> ;
      label:correspondsTo label:Omentum_NCIURI ;
      label:designNote "This concept is extensible; more specific anatomic location within the omentum."^^xsd:string , "This concept may have specific instances."^^xsd:string , "This concept is directly related to the Omentum concept in NCI Thesaurus."^^xsd:string ;
      dc:creator foaf:JimLomax .

<http://mdacc.org/ClinicalLatha#OneM_Concentration>
      rdf:type <http://mdacc.org/ClinicalLatha#Quantity> ;
      <http://mdacc.org/ClinicalLatha#units>
              <http://mdacc.org/ClinicalLatha#Molarity_ConcentrationUnits> ;
      <http://mdacc.org/ClinicalLatha#value>
              "1"^^xsd:string .

<http://mdacc.org/ClinicalLatha#OnePointFiveM_Concentration>
      rdf:type <http://mdacc.org/ClinicalLatha#Concentration> ;
      <http://mdacc.org/ClinicalLatha#units>
              <http://mdacc.org/ClinicalLatha#Molarity_ConcentrationUnits> ;
      <http://mdacc.org/ClinicalLatha#value>
              "1.5"^^xsd:string .

<http://mdacc.org/ClinicalLatha#Ontology_1>
      rdf:type owl:Ontology .

<http://mdacc.org/ClinicalLatha#OralCavityAnatomicSite>
      rdf:type owl:Class ;
      rdfs:comment "The cavity located at the upper end of the alimentary canal, behind the teeth and gums that is bounded on the outside by the lips, above by the hard and soft palates and below by the tongue"^^xsd:string ;
      rdfs:subClassOf <http://mdacc.org/ClinicalLatha#MouthAnatomicSite> ;
      label:correspondsTo label:OralCavity_NCIURI ;
      label:designNote "This concept is directly related to the Oral Cavity concept in NCI Thesaurus."^^xsd:string , "This concept may have specific instances."^^xsd:string , "This concept is extensible; more specific anatomic location within the oral cavity."^^xsd:string ;
      dc:creator foaf:JimLomax .

<http://mdacc.org/ClinicalLatha#Oral_TherapeuticAgentDelivery>
      rdf:type <http://mdacc.org/ClinicalLatha#TherapeuticAgentDelivery> ;
      skos-xl:prefLabel label:Oral_TherapeuticAgentDeliveryLabel .

<http://mdacc.org/ClinicalLatha#Other_DiagnosticProcedure>
      rdf:type <http://mdacc.org/ClinicalLatha#DiagnosticProcedure> ;
      label:creator foaf:JimLomax ;
      label:designNote "This instance needs to go away since \"other\" is not a valid option. This will require some NLP in the notes."^^xsd:string ;
      skos-xl:prefLabel label:Other_DiagnosticProcedureLabel .

<http://mdacc.org/ClinicalLatha#Outcome>
      rdf:type owl:Class ;
      rdfs:comment "The result of an action on a system; either internal or external action. This definition is necessarily generic to support the more specific uses of the concept. "^^xsd:string ;
      rdfs:subClassOf skos:Concept , <http://mdacc.org/ClinicalLatha#ClinicalPackage> ;
      rdfs:subClassOf
              [ rdf:type owl:Restriction ;
                owl:onProperty skos-xl:prefLabel ;
                owl:someValuesFrom label:OutcomeLabel
              ] ;
      label:correspondsTo label:Outcome_NCIURI ;
      label:designNote "This concept is extensible."^^xsd:string , "This concept is directly related to the Outcome concept in NCI Thesaurus."^^xsd:string , "This concept may have instances of it's own or may be a superclass for concept refinements."^^xsd:string ;
      dc:creator foaf:JimLomax .

<http://mdacc.org/ClinicalLatha#OvarianCancer>
      rdf:type owl:Class ;
      rdfs:subClassOf <http://mdacc.org/ClinicalLatha#Cancer> ;
      rdfs:subClassOf
              [ rdf:type owl:Restriction ;
                owl:onProperty <http://mdacc.org/ClinicalLatha#anatomicLocation> ;
                owl:someValuesFrom <http://mdacc.org/ClinicalLatha#OvaryAnatomicSite>
              ] ;
      label:correspondsTo label:OvarianCancer_MESHURI ;
      label:designNote "It is unclear if there are further refinements to the concept, currently we only see a need for instances of Ovarian Cancer"^^xsd:string , "This concept is directly related to the Ovarian Cancer concept in MESH."^^xsd:string ;
      dc:creator foaf:JimLomax .

<http://mdacc.org/ClinicalLatha#OvarianCancer_OvarianCancer>
      rdf:type <http://mdacc.org/ClinicalLatha#OvarianCancer> ;
      <http://mdacc.org/ClinicalLatha#anatomicLocation>
              <http://mdacc.org/ClinicalLatha#Ovary_OvaryAnatomicSite> ;
      label:correspondsTo label:OvarianCancer_MESHURI ;
      skos-xl:prefLabel label:OvarianCancer_OvarianCancerDiseaseLabel .

<http://mdacc.org/ClinicalLatha#OvarianEpithelialCancer_OvarianCancer>
      rdf:type <http://mdacc.org/ClinicalLatha#OvarianCancer> ;
      rdfs:comment "LR: cancer that begins in the cells on the surface of the ovary -NCI thesaurus"^^xsd:string ;
      rdfs:label "OvarianEpithelialCancer"^^xsd:string ;
      <http://mdacc.org/ClinicalLatha#anatomicLocation>
              <http://mdacc.org/ClinicalLatha#Ovary_OvaryAnatomicSite> ;
      label:creator foaf:LathaRamdas .

<http://mdacc.org/ClinicalLatha#OvarianPeritoneum_OvaryAnatomicSite>
      rdf:type <http://mdacc.org/ClinicalLatha#OvaryAnatomicSite> ;
      rdfs:comment "LR:  Skos-xl label is incorrect"^^xsd:string ;
      label:creator foaf:JimLomax ;
      skos-xl:prefLabel label:LeftOvary_OvaryLabel .

<http://mdacc.org/ClinicalLatha#OvarianSerousCarcinoma>
      rdf:type owl:Class ;
      rdfs:comment "Ovarian Serous Carcinoma is a type of Ovarian Cancer."^^xsd:string ;
      rdfs:subClassOf <http://mdacc.org/ClinicalLatha#SerousCarcinoma> ;
      rdfs:subClassOf
              [ rdf:type owl:Restriction ;
                owl:onProperty <http://mdacc.org/ClinicalLatha#anatomicLocation> ;
                owl:someValuesFrom <http://mdacc.org/ClinicalLatha#OvaryAnatomicSite>
              ] ;
      label:correspondsTo label:OvarianSerousCarcinoma_NCIURI ;
      label:designNote "This concept is extensible."^^xsd:string , "This concept may have instances of it's own or may be a superclass for concept refinements."^^xsd:string , "This concept is directly related to the OvarianSerousCarcinoma concept in NCI Thesaurus."^^xsd:string ;
      dc:creator foaf:JimLomax .

<http://mdacc.org/ClinicalLatha#OvarianSerousCystadenocarcinoma_OvarianTumor>
      rdf:type <http://mdacc.org/ClinicalLatha#OvarianTumor> ;
      <http://mdacc.org/ClinicalLatha#anatomicLocation>
              <http://mdacc.org/ClinicalLatha#Ovary_OvaryAnatomicSite> ;
      <http://mdacc.org/ClinicalLatha#manifestedBy>
              <http://mdacc.org/ClinicalLatha#OvarianCancer_OvarianCancer> ;
      label:correspondsTo label:OvarianSerousCarcinoma_NCIURI ;
      label:creator foaf:JimLomax ;
      skos-xl:prefLabel label:OvarianSerousCystadenocarcinoma_OvarianTumorLabel .

<http://mdacc.org/ClinicalLatha#OvarianSlide>
      rdf:type owl:Class ;
      rdfs:subClassOf <http://mdacc.org/ClinicalLatha#Slide> ;
      rdfs:subClassOf
              [ rdf:type owl:Restriction ;
                owl:onProperty <http://mdacc.org/ClinicalLatha#tumorOrigin> ;
                owl:someValuesFrom <http://mdacc.org/ClinicalLatha#OvarianTumor>
              ] ;
      label:architect foaf:MoSanyang ;
      label:creator foaf:JimLomax ;
      label:developer foaf:PradheepRaju , foaf:DawitGebremichael .

<http://mdacc.org/ClinicalLatha#OvarianTumor>
      rdf:type owl:Class ;
      rdfs:comment "Tumor anatomically located within the Ovary"^^xsd:string ;
      rdfs:subClassOf <http://mdacc.org/ClinicalLatha#TumorType> ;
      rdfs:subClassOf
              [ rdf:type owl:Restriction ;
                owl:onProperty <http://mdacc.org/ClinicalLatha#anatomicLocation> ;
                owl:someValuesFrom <http://mdacc.org/ClinicalLatha#OvaryAnatomicSite>
              ] ;
      label:designNote "This concept is extensible."^^xsd:string , "This concept may have instances of it's own or may be a superclass for concept refinements."^^xsd:string ;
      dc:creator foaf:JimLomax .

<http://mdacc.org/ClinicalLatha#OvarianTumor_OvarianTumor>
      rdf:type <http://mdacc.org/ClinicalLatha#OvarianTumor> ;
      <http://mdacc.org/ClinicalLatha#anatomicLocation>
              <http://mdacc.org/ClinicalLatha#Ovary_OvaryAnatomicSite> ;
      <http://mdacc.org/ClinicalLatha#manifestedBy>
              <http://mdacc.org/ClinicalLatha#OvarianCancer_OvarianCancer> ;
      label:creator foaf:JimLomax .

<http://mdacc.org/ClinicalLatha#OvaryAnatomicSite>
      rdf:type owl:Class ;
      rdfs:comment "The pair of female reproductive glands in which the ova, or eggs, are formed. The ovaries are located in the pelvis, one on each side of the uterus"^^xsd:string ;
      rdfs:subClassOf <http://mdacc.org/ClinicalLatha#AnatomicSite> ;
      label:correspondsTo label:Ovary_NCIURI ;
      label:designNote "This concept is directly related to the Ovary concept in NCI Thesaurus."^^xsd:string , "This concept may have specific instances."^^xsd:string , "This concept is extensible; more specific anatomic location within the ovary."^^xsd:string ;
      dc:creator foaf:JimLomax .

<http://mdacc.org/ClinicalLatha#Ovary_OvaryAnatomicSite>
      rdf:type <http://mdacc.org/ClinicalLatha#OvaryAnatomicSite> ;
      rdfs:comment "LR:  Clinical property refers to Left_side.  This needs to be corrected."^^xsd:string ;
      <http://mdacc.org/ClinicalLatha#side>
              <http://mdacc.org/ClinicalLatha#Left_Side> ;
      label:creator foaf:JimLomax ;
      skos-xl:prefLabel label:Ovary_OvaryLabel .

<http://mdacc.org/ClinicalLatha#PNG>
      rdf:type <http://mdacc.org/ClinicalLatha#ImageFormat> .

<http://mdacc.org/ClinicalLatha#PalliativeRegimen>
      rdf:type owl:Class ;
      rdfs:subClassOf <http://mdacc.org/ClinicalLatha#Regimen> ;
      label:architect foaf:MoSanyang ;
      label:creator foaf:JimLomax ;
      label:developer foaf:PradheepRaju , foaf:DawitGebremichael .

<http://mdacc.org/ClinicalLatha#PancreasAnatomicSite>
      rdf:type owl:Class ;
      rdfs:comment "LR:  This need to be changed to the correct comment"^^xsd:string , "The pair of female reproductive glands in which the ova, or eggs, are formed. The ovaries are located in the pelvis, one on each side of the uterus"^^xsd:string ;
      rdfs:subClassOf <http://mdacc.org/ClinicalLatha#AnatomicSite> ;
      label:correspondsTo label:Pancreas_NCIURI ;
      label:designNote "This concept is directly related to the Ovary concept in NCI Thesaurus."^^xsd:string , "This concept may have specific instances."^^xsd:string , "This concept is extensible; more specific anatomic location within the ovary."^^xsd:string ;
      dc:creator foaf:JimLomax .

<http://mdacc.org/ClinicalLatha#Pancreas_PancreasAnatomicSite>
      rdf:type <http://mdacc.org/ClinicalLatha#PancreasAnatomicSite> ;
      label:correspondsTo label:Pancreas_NCIURI ;
      label:creator foaf:JimLomax ;
      skos-xl:prefLabel label:Pancreas_AnatomicSiteLabel .

<http://mdacc.org/ClinicalLatha#PancreaticAdenocarcinoma_PancreaticTumor>
      rdf:type <http://mdacc.org/ClinicalLatha#PancreaticTumor> ;
      <http://mdacc.org/ClinicalLatha#anatomicLocation>
              <http://mdacc.org/ClinicalLatha#Pancreas_PancreasAnatomicSite> ;
      <http://mdacc.org/ClinicalLatha#manifestedBy>
              <http://mdacc.org/ClinicalLatha#PancreaticCancer_PancreaticCancer> ;
      label:correspondsTo label:PancreaticAdenocarcinoma_NCIURI ;
      skos-xl:prefLabel label:PancreaticAdenocarcinoma_PancreaticTumorLabel .

<http://mdacc.org/ClinicalLatha#PancreaticCancer>
      rdf:type owl:Class ;
      rdfs:subClassOf <http://mdacc.org/ClinicalLatha#Cancer> ;
      rdfs:subClassOf
              [ rdf:type owl:Restriction ;
                owl:onProperty <http://mdacc.org/ClinicalLatha#anatomicLocation> ;
                owl:someValuesFrom <http://mdacc.org/ClinicalLatha#PancreasAnatomicSite>
              ] ;
      label:correspondsTo label:PancreaticCancer_MEDRAURI ;
      dc:creator foaf:JimLomax .

<http://mdacc.org/ClinicalLatha#PancreaticCancer_PancreaticCancer>
      rdf:type <http://mdacc.org/ClinicalLatha#PancreaticCancer> ;
      <http://mdacc.org/ClinicalLatha#anatomicLocation>
              <http://mdacc.org/ClinicalLatha#Pancreas_PancreasAnatomicSite> ;
      label:correspondsTo label:PancreaticCancer_MEDRAURI ;
      skos-xl:prefLabel label:PancreaticCancer_PancreaticCancerDiseaseLabel .

<http://mdacc.org/ClinicalLatha#PancreaticTumor>
      rdf:type owl:Class ;
      rdfs:comment "Tumor anatomically located within the Pancreas"^^xsd:string ;
      rdfs:subClassOf <http://mdacc.org/ClinicalLatha#TumorType> ;
      rdfs:subClassOf
              [ rdf:type owl:Restriction ;
                owl:onProperty <http://mdacc.org/ClinicalLatha#anatomicLocation> ;
                owl:someValuesFrom <http://mdacc.org/ClinicalLatha#PancreasAnatomicSite>
              ] ;
      label:designNote "This concept is extensible."^^xsd:string , "This concept may have instances of it's own or may be a superclass for concept refinements."^^xsd:string ;
      dc:creator foaf:JimLomax .

<http://mdacc.org/ClinicalLatha#PapillaryRenaCelllCarcinoma_KidneyCancer>
      rdf:type <http://mdacc.org/ClinicalLatha#KidneyTumor> ;
      rdfs:comment "LR:  Change PapillaryRenaCelllCarcinoma to PapillaryRenalCellCarcinoma"^^xsd:string ;
      <http://mdacc.org/ClinicalLatha#anatomicLocation>
              <http://mdacc.org/ClinicalLatha#Kidney_KidneyAnatomicSite> ;
      <http://mdacc.org/ClinicalLatha#manifestedBy>
              <http://mdacc.org/ClinicalLatha#Kidney_KidneyCancer> ;
      label:correspondsTo label:PapillaryRenalCellCarcinoma_NCIURI ;
      label:creator foaf:JimLomax ;
      skos-xl:prefLabel label:PapillaryRenalCellCarcinoma_KidneyTumorLabel .

<http://mdacc.org/ClinicalLatha#PartialResponse_PrimaryTherapyOutcome>
      rdf:type <http://mdacc.org/ClinicalLatha#PrimaryTherapyOutcome> ;
      label:creator foaf:JimLomax ;
      skos-xl:prefLabel label:PartialResponse_OutcomeLabel .

<http://mdacc.org/ClinicalLatha#PathologicDistantMetastasisTNMFinding>
      rdf:type owl:Class ;
      rdfs:comment "The extent of  metastasis to other parts of the body. "^^xsd:string ;
      rdfs:subClassOf <http://mdacc.org/ClinicalLatha#PathologicTNMFinding> ;
      label:correspondsTo label:PathologicDistantMetastasisTNMFinding_NCIURI ;
      dc:creator foaf:JimLomax .

<http://mdacc.org/ClinicalLatha#PathologicPrimaryTumorTNMFinding>
      rdf:type owl:Class ;
      rdfs:comment "The extent of the primary tumor as pathology reveals. The extent of the primary tumor increases as the classification number increases. pT0 means that the pathologic results indicate no primary tumor. pT1 - pT4 are diesgnations for increasing pathlogic primary tumor extent, however there are no quantitative measurements, direct or relative,  with the designations."^^xsd:string ;
      rdfs:subClassOf <http://mdacc.org/ClinicalLatha#PathologicTNMFinding> ;
      label:correspondsTo label:PathologicPrimaryTumorTNMFinding_NCIURI ;
      dc:creator foaf:JimLomax .

<http://mdacc.org/ClinicalLatha#PathologicRegionalLymphNodesTNMFinding>
      rdf:type owl:Class ;
      rdfs:comment "The extent of regional  lymph node metastasis as pathology reveals. The extent of regional lymph node metatstasis increases as the classification number increases. pN0 means that the pathologic results indicate no regional lymph node metastasis. pN1 - pN3 are designations for increasing metastasis of regional lymph nodes, however there are no quantitative measurements, direct or relative,  with the designations."^^xsd:string ;
      rdfs:subClassOf <http://mdacc.org/ClinicalLatha#PathologicTNMFinding> ;
      label:correspondsTo label:PathologicRegionalLymphNodesTNMFinding_NCIURI ;
      dc:creator foaf:JimLomax .

<http://mdacc.org/ClinicalLatha#PathologicTNMFinding>
      rdf:type owl:Class ;
      rdfs:comment "TNM staging performed as part of pathologic specimen. Pathological TMN staging findings, while there is a generic classification scheme, are not always reported according to that scheme. The classification scheme can vary by cancer type, pathologist, institution, lab or any number of other factors. Also, while the coding scheme for TMN staging is standarized for some cancer types, again, this does not mean that it will be used."^^xsd:string ;
      rdfs:subClassOf <http://mdacc.org/ClinicalLatha#Finding> ;
      rdfs:subClassOf
              [ rdf:type owl:Restriction ;
                owl:onProperty <http://mdacc.org/ClinicalLatha#code> ;
                owl:someValuesFrom rdfs:Literal
              ] ;
      rdfs:subClassOf
              [ rdf:type owl:Restriction ;
                owl:onProperty <http://mdacc.org/ClinicalLatha#tnmScheme> ;
                owl:someValuesFrom <http://mdacc.org/ClinicalLatha#TNMDiseaseStagingSystem>
              ] ;
      label:correspondsTo label:TNMFinding_NCIURI ;
      label:designNote "This concept is extensible."^^xsd:string , "This concept is directly related to the TNM Finding  concept in NCI Thesaurus."^^xsd:string , "This concept may have instances of it's own or may be a superclass for concept refinements."^^xsd:string ;
      dc:creator foaf:JimLomax .

<http://mdacc.org/ClinicalLatha#PathologicalDiagnosisMethod>
      rdf:type owl:Class ;
      rdfs:comment "Methods, procedures, and tests performed to diagnose disease, disordered function, or disability."^^xsd:string ;
      rdfs:subClassOf <http://mdacc.org/ClinicalLatha#ClinicalPackage> ;
      label:domainQuestion
              "Is this the same as diagnostic procedure ?"^^xsd:string ;
      dc:creator foaf:JimLomax .

<http://mdacc.org/ClinicalLatha#PathologicalDiagnosisPatientEvent>
      rdf:type owl:Class ;
      rdfs:subClassOf <http://mdacc.org/ClinicalLatha#DiagnosisPatientEvent> ;
      dc:creator foaf:JimLomax .

<http://mdacc.org/ClinicalLatha#Pathology>
      rdf:type owl:Class ;
      rdfs:subClassOf <http://mdacc.org/ClinicalLatha#ClinicalPackage> ;
      rdfs:subClassOf
              [ rdf:type owl:Restriction ;
                owl:onProperty <http://mdacc.org/ClinicalLatha#observationOf> ;
                owl:someValuesFrom <http://mdacc.org/ClinicalLatha#TumorType>
              ] ;
      label:architect foaf:MoSanyang ;
      label:creator foaf:JimLomax ;
      label:developer foaf:PradheepRaju , foaf:JimLomax , foaf:DawitGebremichael .

<http://mdacc.org/ClinicalLatha#Patient>
      rdf:type owl:Class ;
      rdfs:subClassOf foaf:Person , skos:Concept , <http://mdacc.org/ClinicalLatha#ClinicalPackage> ;
      rdfs:subClassOf
              [ rdf:type owl:Restriction ;
                owl:onProperty <http://mdacc.org/ClinicalLatha#patientId> ;
                owl:someValuesFrom <http://mdacc.org/ClinicalLatha#PatientId>
              ] ;
      label:correspondsTo label:Patient_NCIURI ;
      label:creator foaf:JimLomax ;
      label:designNote "This concept is extensible."^^xsd:string , "A patient must have a Patient Id"^^xsd:string , "This concept may have instances of it's own or may be a superclass for concept refinements."^^xsd:string , "This concept is directly related to the Patient concept in NCI Thesaurus."^^xsd:string .

<http://mdacc.org/ClinicalLatha#Patient1Birth_Instant>
      rdf:type time-entry:Instant ;
      time-entry:inCalendarClockDataType
              "1999-10-12T10:38:32"^^xsd:dateTime .

<http://mdacc.org/ClinicalLatha#Patient1Death_Instant>
      rdf:type time-entry:Instant ;
      time-entry:inCalendarClockDataType
              "2010-11-01T17:38:09.188"^^xsd:dateTime .

<http://mdacc.org/ClinicalLatha#PatientId>
      rdf:type owl:Class ;
      rdfs:comment "Patient Id is a concept for uniquely identifying a Patient.   "^^xsd:string ;
      rdfs:subClassOf skos:Concept , <http://mdacc.org/ClinicalLatha#ClinicalPackage> ;
      rdfs:subClassOf
              [ rdf:type owl:Restriction ;
                owl:onProperty dc:identifier ;
                owl:someValuesFrom xsd:string
              ] ;
      label:designNote "To allow for variations in  consumable labels for the concept, the  SKOS-XL framework is used; SKOS-XL in particular for its extensions that allow relationships  to exist between labels."^^xsd:string , "The consumable label for a Patient Id may vary across  domain interpretations. This is the case with The Cancer Genome Atlas, where patients are identified in a clinical context by a \"BCRPatientBarcode\"."^^xsd:string , "To aid in data integration a Patient Id will be defined  by a union of known concepts that logically map to the concept of Patient Id."^^xsd:string ;
      owl:equivalentClass
              [ rdf:type owl:Restriction ;
                owl:onProperty sample:patientIdOf ;
                owl:someValuesFrom owl:Thing
              ] .

<http://mdacc.org/ClinicalLatha#Peritoneum>
      rdf:type owl:Class ;
      rdfs:comment "The tissue that lines the wall of the abdominal cavity, intestine, and mesentery. It consists of the parietal peritoneum that covers the inside of the abdominal wall and the visceral peritoneum that covers the surface of the intestine and mesentery."^^xsd:string ;
      rdfs:subClassOf <http://mdacc.org/ClinicalLatha#Membrane> ;
      label:correspondsTo label:Peritoneum_NCIURI ;
      label:designNote "This concept may have instances of it's own or may be a superclass for concept refinements."^^xsd:string , "This concept is directly related to the Peritoneum  concept in NCI Thesaurus."^^xsd:string ;
      dc:creator foaf:JimLomax .

<http://mdacc.org/ClinicalLatha#PersonNeoplasmCancerStatus>
      rdf:type owl:Class ;
      rdfs:comment "This seems to be existential; yes or no, does the patient have cancer. This is derived from a conceptual relationship between patient and tumor."^^xsd:string ;
      rdfs:subClassOf <http://mdacc.org/ClinicalLatha#ClinicalPackage> ;
      label:designNote "This is a TCGA specific entity"^^xsd:string , "There is no corresponding concept in BioPortal"^^xsd:string , "This is actually a property, \"hasCancer\", yes or no. Actually this is derived from a patient having at least one diagnosis of cancer that has not gone into remission."^^xsd:string ;
      dc:creator foaf:JimLomax .

<http://mdacc.org/ClinicalLatha#Phagocyte>
      rdf:type owl:Class ;
      rdfs:comment "Cells that can carry out the process of phagocytosis."^^xsd:string ;
      rdfs:subClassOf <http://mdacc.org/ClinicalLatha#ConnectiveTissueCell> ;
      label:correspondsTo label:Phagocyte_MESHURI ;
      label:designNote "This concept is extensible."^^xsd:string , "This concept is directly related to the Phagocyte concept in MESH."^^xsd:string , "This concept may have instances of it's own  or may be a superclass for concept refinements."^^xsd:string ;
      dc:creator foaf:JimLomax .

<http://mdacc.org/ClinicalLatha#Pill_DosageUnits>
      rdf:type <http://mdacc.org/ClinicalLatha#DrugDosageUnits> ;
      <http://mdacc.org/ClinicalLatha#value>
              "Pill"^^xsd:string .

<http://mdacc.org/ClinicalLatha#PlasmaCell>
      rdf:type owl:Class ;
      rdfs:comment "Specialized forms of antibody-producing B-lymphocytes. They synthesize and secrete immunoglobulin. They are found only in lymphoid organs and at sites of immune responses and normally do not circulate in the blood or lymph."^^xsd:string ;
      rdfs:subClassOf <http://mdacc.org/ClinicalLatha#BCell> ;
      label:correspondsTo label:PlasmaCell_NCIURI ;
      label:designNote "This concept is extensible."^^xsd:string , "This concept is directly related to the Plasma Cell concept in NCI Thesaurus"^^xsd:string , "This concept may have instances of it's own or may be a superclass for concept refinements."^^xsd:string ;
      dc:creator foaf:JimLomax .

<http://mdacc.org/ClinicalLatha#PopulationCharacteristic>
      rdf:type owl:Class ;
      rdfs:comment "A common factor (e.g., geographic location, ethnicity, disease, age, gender) that unites groups of individuals."^^xsd:string ;
      rdfs:subClassOf skos:Concept , <http://mdacc.org/ClinicalLatha#ClinicalPackage> ;
      rdfs:subClassOf
              [ rdf:type owl:Restriction ;
                owl:onProperty skos-xl:prefLabel ;
                owl:someValuesFrom label:PopulationCharacteristicLabel
              ] ;
      label:correspondsTo label:PopulationGroup_NCIURI ;
      label:creator foaf:JimLomax ;
      label:designNote "This concept is extensible."^^xsd:string , "This concept is similar to the concept of Population Group in NCI Thesaurus, however there are some inconsistencies in the definition of the class and the definition of subclasses."^^xsd:string , "This concept may have instances of it's own or may be a superclass for concept refinements."^^xsd:string .

<http://mdacc.org/ClinicalLatha#PortionExample_Volume>
      rdf:type <http://mdacc.org/ClinicalLatha#Volume> ;
      <http://mdacc.org/ClinicalLatha#units>
              <http://mdacc.org/ClinicalLatha#Milliliter_VolumeUnits> ;
      <http://mdacc.org/ClinicalLatha#value>
              "1.0"^^xsd:string .

<http://mdacc.org/ClinicalLatha#Pounds_WeightUnits>
      rdf:type <http://mdacc.org/ClinicalLatha#WeightUnits> ;
      <http://mdacc.org/ClinicalLatha#value>
              "Pounds"^^xsd:string .

<http://mdacc.org/ClinicalLatha#PreTreatmentHistoryExistentialEvent>
      rdf:type owl:Class ;
      rdfs:comment "In a TCGA context this represents if a Patient has any pre treatment history; a boolean value, it is not the history itself."^^xsd:string ;
      rdfs:subClassOf <http://mdacc.org/ClinicalLatha#ExistentialEvent> ;
      label:designNote "This concept may be demoted to an instance"^^xsd:string , "There is no corresponding concept in BioPortal"^^xsd:string ;
      dc:creator foaf:JimLomax .

<http://mdacc.org/ClinicalLatha#PrimaryTherapyOutcome>
      rdf:type owl:Class ;
      rdfs:comment "The outcome of the primary therapy session."^^xsd:string ;
      rdfs:subClassOf <http://mdacc.org/ClinicalLatha#TherapeuticProcedureOutcome> ;
      label:creator foaf:JimLomax ;
      label:designNote "This concept is extensible."^^xsd:string , "There is no corresponding concept in BioPortal"^^xsd:string , "This concept is specific to TCGA (so far)"^^xsd:string , "This concept may have instances of it's own or may be a superclass for concept refinements."^^xsd:string .

<http://mdacc.org/ClinicalLatha#Primary_MetastaticIndication>
      rdf:type <http://mdacc.org/ClinicalLatha#MetastaticIndication> ;
      skos-xl:prefLabel label:Primary_MetastaticIndicationLabel .

<http://mdacc.org/ClinicalLatha#PriorCancerOccurence>
      rdf:type owl:Class ;
      rdfs:comment "Indicates if a Patient had cancer prior to the current occurence."^^xsd:string ;
      rdfs:subClassOf <http://mdacc.org/ClinicalLatha#ClinicalPackage> ;
      label:designNote "There is no corresponding concept in BioPortal"^^xsd:string , "This is actually a property, \"hadCancer\", yes or no. Actually this is derived from a patient having at least one diagnosis of cancer that has  gone into remission."^^xsd:string ;
      dc:creator foaf:JimLomax .

<http://mdacc.org/ClinicalLatha#ProgressionRegimen>
      rdf:type owl:Class ;
      rdfs:subClassOf <http://mdacc.org/ClinicalLatha#Regimen> ;
      label:architect foaf:MoSanyang ;
      label:creator foaf:JimLomax ;
      label:developer foaf:PradheepRaju , foaf:DawitGebremichael .

<http://mdacc.org/ClinicalLatha#ProgressiveDisease_PrimaryTherapyOutcome>
      rdf:type <http://mdacc.org/ClinicalLatha#PrimaryTherapyOutcome> ;
      label:creator foaf:JimLomax ;
      skos-xl:prefLabel label:ProgressiveDisease_OutcomeLabel .

<http://mdacc.org/ClinicalLatha#ProstateAdenocarcinoma_ProstateTumor>
      rdf:type <http://mdacc.org/ClinicalLatha#ProstateTumor> ;
      <http://mdacc.org/ClinicalLatha#anatomicLocation>
              <http://mdacc.org/ClinicalLatha#Prostate_ProstateAnatomicSite> ;
      <http://mdacc.org/ClinicalLatha#manifestedBy>
              <http://mdacc.org/ClinicalLatha#ProstateCancer_ProstateCancer> ;
      label:correspondsTo label:ProstateAdenocarcinoma_NCIURI ;
      label:creator foaf:JimLomax ;
      skos-xl:prefLabel label:ProstateAdenocarcinoma_ProstateTumorLabel .

<http://mdacc.org/ClinicalLatha#ProstateAnatomicSite>
      rdf:type owl:Class ;
      rdfs:comment "The pair of female reproductive glands in which the ova, or eggs, are formed. The ovaries are located in the pelvis, one on each side of the uterus"^^xsd:string ;
      rdfs:subClassOf <http://mdacc.org/ClinicalLatha#AnatomicSite> ;
      label:correspondsTo label:Pancreas_NCIURI ;
      label:designNote "This concept is directly related to the Ovary concept in NCI Thesaurus."^^xsd:string , "This concept may have specific instances."^^xsd:string , "This concept is extensible; more specific anatomic location within the ovary."^^xsd:string ;
      dc:creator foaf:JimLomax .

<http://mdacc.org/ClinicalLatha#ProstateCancer>
      rdf:type owl:Class ;
      rdfs:subClassOf <http://mdacc.org/ClinicalLatha#Cancer> ;
      rdfs:subClassOf
              [ rdf:type owl:Restriction ;
                owl:onProperty <http://mdacc.org/ClinicalLatha#anatomicLocation> ;
                owl:someValuesFrom <http://mdacc.org/ClinicalLatha#ProstateAnatomicSite>
              ] ;
      label:correspondsTo label:ProstateCancer_MEDRAURI ;
      dc:creator foaf:JimLomax .

<http://mdacc.org/ClinicalLatha#ProstateCancer_ProstateCancer>
      rdf:type <http://mdacc.org/ClinicalLatha#ProstateCancer> ;
      <http://mdacc.org/ClinicalLatha#anatomicLocation>
              <http://mdacc.org/ClinicalLatha#Prostate_ProstateAnatomicSite> ;
      label:correspondsTo label:ProstateCancer_MEDRAURI ;
      label:creator foaf:JimLomax ;
      skos-xl:prefLabel label:ProstateCancer_ProstateCancerDiseaseLabel .

<http://mdacc.org/ClinicalLatha#ProstateTumor>
      rdf:type owl:Class ;
      rdfs:comment "Tumor anatomically located within the Prostate"^^xsd:string ;
      rdfs:subClassOf <http://mdacc.org/ClinicalLatha#TumorType> ;
      rdfs:subClassOf
              [ rdf:type owl:Restriction ;
                owl:onProperty <http://mdacc.org/ClinicalLatha#anatomicLocation> ;
                owl:someValuesFrom <http://mdacc.org/ClinicalLatha#ProstateAnatomicSite>
              ] ;
      label:designNote "This concept is extensible."^^xsd:string , "This concept may have instances of it's own or may be a superclass for concept refinements."^^xsd:string ;
      dc:creator foaf:JimLomax .

<http://mdacc.org/ClinicalLatha#Prostate_ProstateAnatomicSite>
      rdf:type <http://mdacc.org/ClinicalLatha#ProstateAnatomicSite> ;
      label:correspondsTo label:Prostate_NCIURI ;
      label:creator foaf:JimLomax ;
      skos-xl:prefLabel label:Prostate_AnatomicSiteLabel .

<http://mdacc.org/ClinicalLatha#Proteasome>
      rdf:type mage:CellularComponent .

<http://mdacc.org/ClinicalLatha#Protein>
      rdf:type owl:Class ;
      rdfs:comment "A group of complex organic macromolecules composed of one or more chains (linear polymers) of alpha-L-amino acids linked by peptide bonds and ranging in size from a few thousand to over 1 million Daltons"^^xsd:string ;
      rdfs:subClassOf <http://mdacc.org/ClinicalLatha#BioMaterial> ;
      label:correspondsTo label:Protein_NCIURI ;
      label:designNote "This concept is extensible; there are different types of Proteins (antibodies, enzymes) each of which will have different properties."^^xsd:string , "This concept is directly related to the Protein concept in NCI Thesaurus."^^xsd:string , "This concept may have instances of it's own or may be a superclass for concept refinements."^^xsd:string ;
      dc:creator foaf:JimLomax .

<http://mdacc.org/ClinicalLatha#ProteinDimer>
      rdf:type mage:CellularComponent .

<http://mdacc.org/ClinicalLatha#ProteinTrimer>
      rdf:type mage:CellularComponent .

<http://mdacc.org/ClinicalLatha#Protocol>
      rdf:type owl:Class ;
      rdfs:comment "This concept is extensible."^^xsd:string , "A rule which guides how an activity should be performed."^^xsd:string ;
      rdfs:subClassOf skos:Concept , <http://mdacc.org/ClinicalLatha#ClinicalPackage> ;
      rdfs:subClassOf
              [ rdf:type owl:Restriction ;
                owl:onProperty skos-xl:prefLabel ;
                owl:someValuesFrom label:ProtocolLabel
              ] ;
      rdfs:subClassOf
              [ rdf:type owl:Restriction ;
                owl:onProperty dc:identifier ;
                owl:someValuesFrom rdfs:Literal
              ] ;
      label:correspondsTo label:Protocol_NCIURI ;
      label:designNote "This concept is extensible."^^xsd:string , "This concept is directly related to the Protocol concept in NCI Thesaurus."^^xsd:string , "This concept may have instances of it's own or may be a superclass for concept refinements."^^xsd:string ;
      dc:creator foaf:JimLomax .

<http://mdacc.org/ClinicalLatha#ProtocolType>
      rdf:type owl:Class ;
      rdfs:comment "This concept is extensible."^^xsd:string , "Classification mechanism for Protocols"^^xsd:string ;
      rdfs:subClassOf skos:Concept , <http://mdacc.org/ClinicalLatha#ClinicalPackage> ;
      rdfs:subClassOf
              [ rdf:type owl:Restriction ;
                owl:onProperty skos-xl:prefLabel ;
                owl:someValuesFrom label:ProtocolLabel
              ] ;
      rdfs:subClassOf
              [ rdf:type owl:Restriction ;
                owl:onProperty dc:identifier ;
                owl:someValuesFrom rdfs:Literal
              ] ;
      label:designNote "This concept is extensible."^^xsd:string , "This concept may have instances of it's own or may be a superclass for concept refinements."^^xsd:string ;
      dc:creator foaf:JimLomax .

<http://mdacc.org/ClinicalLatha#PurityMeasurment>
      rdf:type owl:Class ;
      rdfs:comment "Measures the purity of a substance."^^xsd:string ;
      rdfs:subClassOf <http://mdacc.org/ClinicalLatha#Quantity> ;
      label:designNote "This concept does not corresponds toany concept in BioPortal"^^xsd:string ;
      dc:creator foaf:JimLomax .

<http://mdacc.org/ClinicalLatha#Quantity>
      rdf:type owl:Class ;
      rdfs:comment "How much of something there is to measure.A quantity is more than a numeric value; it is a numeric value with units of measurement"^^xsd:string ;
      rdfs:subClassOf skos:Concept , <http://mdacc.org/ClinicalLatha#ClinicalPackage> ;
      rdfs:subClassOf
              [ rdf:type owl:Restriction ;
                owl:onProperty <http://mdacc.org/ClinicalLatha#value> ;
                owl:someValuesFrom rdfs:Literal
              ] ;
      rdfs:subClassOf
              [ rdf:type owl:Restriction ;
                owl:onProperty <http://mdacc.org/ClinicalLatha#units> ;
                owl:someValuesFrom <http://mdacc.org/ClinicalLatha#Units>
              ] ;
      rdfs:subClassOf
              [ rdf:type owl:Restriction ;
                owl:onProperty skos-xl:prefLabel ;
                owl:someValuesFrom label:QuantityLabel
              ] ;
      label:correspondsTo label:Quantity_NCIURI ;
      label:designNote "This concept is extensible."^^xsd:string , "This concept is directly related to the Quantity concept in NCI Thesaurus."^^xsd:string , "This concept hierarchy really belongs in its own ontology: Measurement"^^xsd:string , "This concept may have instances of it's own or may be a superclass for concept refinements."^^xsd:string ;
      dc:creator foaf:JimLomax .

<http://mdacc.org/ClinicalLatha#RNA>
      rdf:type owl:Class ;
      rdfs:comment "Single-stranded long chain of nucleotides containing ribose. It is the end product of DNA transcription by the enzyme RNA polymerase. It is essential in protein synthesis."^^xsd:string ;
      rdfs:subClassOf <http://mdacc.org/ClinicalLatha#BioMaterial> ;
      label:correspondsTo label:RNA_NCIURI ;
      label:creator foaf:JimLomax ;
      label:designNote "This concept is directly related to the RNA concept in NCI Thesaurus."^^xsd:string , "This concept is extensible; there are different types of RNA (tRNA, mRNA, rRNA) each of which will have different properties."^^xsd:string , "This concept may have instances of it's own or may be a superclass for concept refinements."^^xsd:string .

<http://mdacc.org/ClinicalLatha#Race>
      rdf:type owl:Class ;
      rdfs:comment "The US Census Bureau makes use of both race and ethnicity in surveys, however there are no race or ethnicity vocabularies or taxonomies used."^^xsd:string , "http://en.wikipedia.org/wiki/Race_and_ethnicity_in_the_United_States_Census"^^xsd:string ;
      rdfs:subClassOf <http://mdacc.org/ClinicalLatha#PopulationCharacteristic> ;
      rdfs:subClassOf
              [ rdf:type owl:Restriction ;
                owl:onProperty skos-xl:prefLabel ;
                owl:someValuesFrom label:RaceLabel
              ] ;
      label:correspondsTo label:Race_NCIURI ;
      label:designNote "This concept is extensible."^^xsd:string , "This concept is directly related to the Race concept in NCI Thesaurus."^^xsd:string , "This concept may have instances of it's own or may be a superclass for concept refinements."^^xsd:string ;
      dc:creator foaf:JimLomax .

<http://mdacc.org/ClinicalLatha#RadiationDosage>
      rdf:type owl:Class ;
      rdfs:comment "The amount of radiation energy that is deposited in a unit mass of material, such as tissues of plants or animal. In radiotherapy, radiation dosage is expressed in gray units (Gy). In radiologic health, the dosage is expressed by the product of absorbed dose (Gy) and quality factor (a function of linear energy transfer), and is called radiation dose equivalent in sievert units (Sv)."^^xsd:string ;
      rdfs:subClassOf <http://mdacc.org/ClinicalLatha#Dosage> ;
      rdfs:subClassOf
              [ rdf:type owl:Restriction ;
                owl:onProperty skos-xl:prefLabel ;
                owl:someValuesFrom label:DosageLabel
              ] ;
      label:correspondsTo label:RadiationDosage_MESHURI ;
      label:designNote "This concept directly corresponds to the Radiation Dosage concept in MESH."^^xsd:string ;
      dc:creator foaf:JimLomax .

<http://mdacc.org/ClinicalLatha#RadiationDosageUnits>
      rdf:type owl:Class ;
      rdfs:subClassOf <http://mdacc.org/ClinicalLatha#DosageUnits> ;
      dc:creator foaf:JimLomax .

<http://mdacc.org/ClinicalLatha#RadiationTherapy>
      rdf:type owl:Class ;
      rdfs:comment "The use of high-energy radiation from x-rays, gamma rays, neutrons, and other sources to kill cancer cells and shrink tumors. Radiation may come from a machine outside the body (external-beam radiation therapy) or from materials called radioisotopes. Radioisotopes produce radiation and can be placed in or near the tumor or in the area near cancer cells. This type of radiation treatment is called internal radiation therapy, implant radiation, interstitial radiation, or brachytherapy. Systemic radiation therapy uses a radioactive substance, such as a radiolabeled monoclonal antibody, that circulates throughout the body."^^xsd:string ;
      rdfs:subClassOf <http://mdacc.org/ClinicalLatha#TherapeuticProcedure> ;
      label:correspondsTo label:RadiationTherapy_NCIURI ;
      label:designNote "This concept is extensible."^^xsd:string , "This concept is directly related to the Radiation Therapy concept in NCI Thesaurus."^^xsd:string , "This concept may have instances of it's own or may be a superclass for concept refinements."^^xsd:string ;
      dc:creator foaf:JimLomax .

<http://mdacc.org/ClinicalLatha#RadiationTherapyExistentialEvent>
      rdf:type owl:Class ;
      rdfs:comment "This concept represents the existential nature of a radiation therapy; the concept is not concerned with spatio-temporal aspects of the event, only that it occurred."^^xsd:string ;
      rdfs:subClassOf <http://mdacc.org/ClinicalLatha#TherapeuticProcedureExistentialEvent> ;
      label:designNote "This existential concept is a product of TCGA's need to capture just the existence of a radiation therapy."^^xsd:string , "This concept is related to the Radiation Therapy under Therapeutic Procedure"^^xsd:string , "This concept may be domeoted to an instance"^^xsd:string ;
      dc:creator foaf:JimLomax .

<http://mdacc.org/ClinicalLatha#RadioIsotopeRadiationTherapy>
      rdf:type owl:Class ;
      rdfs:comment "Radiation therapy that uses a machine to aim high-energy rays at the cancer."^^xsd:string ;
      rdfs:subClassOf <http://mdacc.org/ClinicalLatha#RadiationTherapy> ;
      label:correspondsTo label:RadioIsotopeTherapy_NCIURI ;
      label:designNote "This concept is extensible."^^xsd:string , "This concept is directly related to the Radio Isotope Radiation Therapy concept in NCI Thesaurus."^^xsd:string , "This concept may have instances of it's own or may be a superclass for concept refinements."^^xsd:string ;
      dc:creator foaf:JimLomax .

<http://mdacc.org/ClinicalLatha#RadioisotopeRadiation>
      rdf:type owl:Class ;
      rdfs:subClassOf <http://mdacc.org/Drug#Radiation> .

<http://mdacc.org/ClinicalLatha#RectalAdenocarcinoma_RectalTumor>
      rdf:type <http://mdacc.org/ClinicalLatha#RectalTumor> ;
      <http://mdacc.org/ClinicalLatha#anatomicLocation>
              <http://mdacc.org/ClinicalLatha#Prostate_ProstateAnatomicSite> ;
      <http://mdacc.org/ClinicalLatha#manifestedBy>
              <http://mdacc.org/ClinicalLatha#ProstateCancer_ProstateCancer> ;
      label:correspondsTo label:RectalAdenocarcinoma_NCIURI ;
      skos-xl:prefLabel label:RectalAdenocarcinoma_RectalTumorLabel .

<http://mdacc.org/ClinicalLatha#RectalCancer>
      rdf:type owl:Class ;
      rdfs:subClassOf <http://mdacc.org/ClinicalLatha#Cancer> ;
      rdfs:subClassOf
              [ rdf:type owl:Restriction ;
                owl:onProperty <http://mdacc.org/ClinicalLatha#anatomicLocation> ;
                owl:someValuesFrom <http://mdacc.org/ClinicalLatha#RectumAnatomicSite>
              ] ;
      label:correspondsTo label:RectalCancer_MEDRAURI ;
      dc:creator foaf:JimLomax .

<http://mdacc.org/ClinicalLatha#RectalCancer_RectalCancer>
      rdf:type <http://mdacc.org/ClinicalLatha#RectalCancer> ;
      <http://mdacc.org/ClinicalLatha#anatomicLocation>
              <http://mdacc.org/ClinicalLatha#Rectum_RectumAnatomicSite> ;
      label:correspondsTo label:RectalCancer_MEDRAURI ;
      skos-xl:prefLabel label:RectalCancer_RectalCancerDiseaseLabel .

<http://mdacc.org/ClinicalLatha#RectalTumor>
      rdf:type owl:Class ;
      rdfs:comment "Tumor anatomically located within the Rectum"^^xsd:string ;
      rdfs:subClassOf <http://mdacc.org/ClinicalLatha#TumorType> ;
      rdfs:subClassOf
              [ rdf:type owl:Restriction ;
                owl:onProperty <http://mdacc.org/ClinicalLatha#anatomicLocation> ;
                owl:someValuesFrom <http://mdacc.org/ClinicalLatha#RectumAnatomicSite>
              ] ;
      label:designNote "This concept is extensible."^^xsd:string , "This concept may have instances of it's own or may be a superclass for concept refinements."^^xsd:string ;
      dc:creator foaf:JimLomax .

<http://mdacc.org/ClinicalLatha#RectumAnatomicSite>
      rdf:type owl:Class ;
      rdfs:comment "The terminal portion of the gastrointestinal tract, extending from the rectosigmoid junction to the anal canal"^^xsd:string ;
      rdfs:subClassOf <http://mdacc.org/ClinicalLatha#AnatomicSite> ;
      label:correspondsTo label:Rectum_NCIURI ;
      label:designNote "This concept is directly related to the Rectum concept in NCI Thesaurus."^^xsd:string , "This concept is extensible; more specific anatomic location within the rectum."^^xsd:string , "This concept may have specific instances"^^xsd:string ;
      dc:creator foaf:JimLomax .

<http://mdacc.org/ClinicalLatha#Rectum_RectumAnatomicSite>
      rdf:type <http://mdacc.org/ClinicalLatha#RectumAnatomicSite> ;
      label:correspondsTo label:Rectum_NCIURI ;
      label:creator foaf:JimLomax ;
      skos-xl:prefLabel label:Rectum_RectumLabel .

<http://mdacc.org/ClinicalLatha#RecurrenceRegimen>
      rdf:type owl:Class ;
      rdfs:subClassOf <http://mdacc.org/ClinicalLatha#Regimen> ;
      label:architect foaf:MoSanyang ;
      label:creator foaf:JimLomax ;
      label:developer foaf:PradheepRaju , foaf:DawitGebremichael .

<http://mdacc.org/ClinicalLatha#Regimen>
      rdf:type owl:Class ;
      rdfs:comment "A plan that specifies the dosage, schedule, and  duration of a collection of  therapeutic procedures."^^xsd:string , "A regimen may be developed abstractly for a group (cohort) or may developed for a specific patient."^^xsd:string ;
      rdfs:subClassOf skos:Concept , <http://mdacc.org/ClinicalLatha#ClinicalPackage> ;
      rdfs:subClassOf
              [ rdf:type owl:Class ;
                owl:unionOf ([ rdf:type owl:Restriction ;
                            owl:onProperty <http://mdacc.org/ClinicalLatha#therapeuticProcedures> ;
                            owl:someValuesFrom collections:List
                          ] [ rdf:type owl:Restriction ;
                            owl:onProperty <http://mdacc.org/ClinicalLatha#therapeuticProcedure> ;
                            owl:someValuesFrom <http://mdacc.org/ClinicalLatha#TherapeuticProcedure>
                          ])
              ] ;
      rdfs:subClassOf
              [ rdf:type owl:Restriction ;
                owl:onProperty skos-xl:prefLabel ;
                owl:someValuesFrom label:RegimenLabel
              ] ;
      label:correspondsTo label:Regimen_NCIURI ;
      label:designNote "This concept is extensible."^^xsd:string , "This concept is directly related to the Regimen concept in NCI Thesaurus."^^xsd:string , "This concept may have instances of it's own or may be a superclass for concept refinements."^^xsd:string ;
      dc:creator foaf:JimLomax .

<http://mdacc.org/ClinicalLatha#RegimenModel>
      rdf:type owl:Class ;
      rdfs:comment "A Regimen Model is a Regimen that is not designed specifically for a Patient, it is designed to be a guide for treatments of a particular condition."^^xsd:string ;
      rdfs:subClassOf skos:Concept , <http://mdacc.org/ClinicalLatha#ClinicalPackage> ;
      rdfs:subClassOf
              [ rdf:type owl:Restriction ;
                owl:onProperty <http://mdacc.org/ClinicalLatha#therapeuticProcedures> ;
                owl:someValuesFrom collections:List
              ] ;
      rdfs:subClassOf
              [ rdf:type owl:Restriction ;
                owl:onProperty skos-xl:prefLabel ;
                owl:someValuesFrom label:RegimenLabel
              ] ;
      label:designNote "There is no corresponding concept in BioPortal"^^xsd:string ;
      dc:creator foaf:JimLomax .

<http://mdacc.org/ClinicalLatha#RegimenModel1_RegimenModel>
      rdf:type <http://mdacc.org/ClinicalLatha#RegimenModel> ;
      <http://mdacc.org/ClinicalLatha#therapeuticProcedures>
              <http://mdacc.org/ClinicalLatha#TherpaeuticProcedures1_Collection> .

<http://mdacc.org/ClinicalLatha#Remission_DiseaseOutcome>
      rdf:type <http://mdacc.org/ClinicalLatha#DiseaseOutcome> ;
      <http://mdacc.org/ClinicalLatha#outcomeOf>
              <http://mdacc.org/ClinicalLatha#BladderCancer_BladderCancer> ;
      label:correspondsTo label:Remission_NCIURI ;
      label:creator foaf:JimLomax ;
      label:designNote "This concept directly corresponds to the concept of Remission in NCI Thesaurus"^^xsd:string .

<http://mdacc.org/ClinicalLatha#RenaCelllCarcinoma_KidneyTumor>
      rdf:type <http://mdacc.org/ClinicalLatha#KidneyTumor> ;
      rdfs:comment "LR: In the references, correct RenaCelllCarcinoma to RenalCellCarcinoma"^^xsd:string ;
      <http://mdacc.org/ClinicalLatha#anatomicLocation>
              <http://mdacc.org/ClinicalLatha#Kidney_KidneyAnatomicSite> ;
      <http://mdacc.org/ClinicalLatha#manifestedBy>
              <http://mdacc.org/ClinicalLatha#Kidney_KidneyCancer> ;
      label:correspondsTo label:RenalCellCarcinoma_NCIURI ;
      label:creator foaf:JimLomax ;
      skos-xl:prefLabel label:RenalCellCarcinoma_KidneyTumorLabel .

<http://mdacc.org/ClinicalLatha#RenaCelllClearCellCarcinoma_KidneyTumor>
      rdf:type <http://mdacc.org/ClinicalLatha#KidneyTumor> ;
      <http://mdacc.org/ClinicalLatha#anatomicLocation>
              <http://mdacc.org/ClinicalLatha#Kidney_KidneyAnatomicSite> ;
      <http://mdacc.org/ClinicalLatha#manifestedBy>
              <http://mdacc.org/ClinicalLatha#Kidney_KidneyCancer> ;
      label:correspondsTo label:RenalCellClearCellCarcinoma_NCIURI ;
      label:creator foaf:JimLomax ;
      skos-xl:prefLabel label:RenalClearCellCarcinoma_KidneyTumorLabel .

<http://mdacc.org/ClinicalLatha#RenalCarcinoma_KidneyTumor>
      rdf:type <http://mdacc.org/ClinicalLatha#KidneyTumor> ;
      <http://mdacc.org/ClinicalLatha#anatomicLocation>
              <http://mdacc.org/ClinicalLatha#Kidney_KidneyAnatomicSite> ;
      <http://mdacc.org/ClinicalLatha#manifestedBy>
              <http://mdacc.org/ClinicalLatha#Kidney_KidneyCancer> ;
      label:correspondsTo label:RenalCarcinoma_NCIURI ;
      label:creator foaf:JimLomax ;
      skos-xl:prefLabel label:RenalCarcinoma_KidneyTumorLabel .

<http://mdacc.org/ClinicalLatha#ResidualTumorFinding>
      rdf:type owl:Class ;
      rdfs:comment "Residual tumor finding post surgical procedure"^^xsd:string ;
      rdfs:subClassOf <http://mdacc.org/ClinicalLatha#Finding> ;
      rdfs:subClassOf
              [ rdf:type owl:Restriction ;
                owl:onProperty dc:identifier ;
                owl:someValuesFrom xsd:string
              ] ;
      label:correspondsTo label:ResidualTumor_MESHURI ;
      label:designNote "The TCGA specific interpretation of this concept is only a size of residual tumor, which is categorized by size range. A specific size is not captured."^^xsd:string , "This concept directly corresponds to the Residual Neoplasm concept in MESH."^^xsd:string ;
      dc:creator foaf:JimLomax .

<http://mdacc.org/ClinicalLatha#Resource_2>
      rdf:type rdfs:Resource .

<http://mdacc.org/ClinicalLatha#RightCerebralHemisphere_BrainAnatomicSite>
      rdf:type <http://mdacc.org/ClinicalLatha#BrainAnatomicSite> ;
      label:correspondsTo label:RightCerebralHemisphere_NCIURI ;
      label:creator foaf:JimLomax ;
      skos-xl:prefLabel label:RightCerebralHemisphere_AnatomicSiteLabel .

<http://mdacc.org/ClinicalLatha#RightLung_LungAnatomicSite>
      rdf:type <http://mdacc.org/ClinicalLatha#LungAnatomicSite> ;
      <http://mdacc.org/ClinicalLatha#side>
              <http://mdacc.org/ClinicalLatha#Right_Side> ;
      label:correspondsTo label:RightLung_NCIURI ;
      label:creator foaf:JimLomax ;
      skos-xl:prefLabel label:RightLung_AnatomicSiteLabel .

<http://mdacc.org/ClinicalLatha#RightOvary_OvaryAnatomicSite>
      rdf:type <http://mdacc.org/ClinicalLatha#OvaryAnatomicSite> ;
      rdfs:comment "LR:  Property clinical:Side refers to left for this Right ovary instance.  Please correct"^^xsd:string ;
      <http://mdacc.org/ClinicalLatha#side>
              <http://mdacc.org/ClinicalLatha#Right_Side> ;
      label:creator foaf:JimLomax ;
      skos-xl:prefLabel label:LeftOvary_OvaryLabel .

<http://mdacc.org/ClinicalLatha#Right_Side>
      rdf:type <http://mdacc.org/ClinicalLatha#Side> ;
      label:creator foaf:JimLomax ;
      skos-xl:prefLabel label:Left_SideLabel .

<http://mdacc.org/ClinicalLatha#RoughEndoplasmicReticulum>
      rdf:type mage:CellularComponent .

<http://mdacc.org/ClinicalLatha#ScientificEquipment>
      rdf:type owl:Class ;
      rdfs:comment "An object used in scientific research that is not consumed."^^xsd:string ;
      rdfs:subClassOf <http://mdacc.org/ClinicalLatha#Equipment> ;
      label:correspondsTo label:ScientificEquipment_NCIURI ;
      label:designNote "This concept is extensible."^^xsd:string , "This concept is directly related to the Scientific Equipment concept in NCI Thesaurus."^^xsd:string , "This concept may have instances of it's own or may be a superclass for concept refinements."^^xsd:string ;
      dc:creator foaf:JimLomax .

<http://mdacc.org/ClinicalLatha#Secondary_MetastaticIndication>
      rdf:type <http://mdacc.org/ClinicalLatha#MetastaticIndication> ;
      skos-xl:prefLabel label:Secondary_MetastaticIndicationLabel .

<http://mdacc.org/ClinicalLatha#SelectBioMaterials>
      rdf:type rdfs:Class ;
      rdfs:subClassOf sp:Select .

<http://mdacc.org/ClinicalLatha#Sephardic_JewishOrigin>
      rdf:type <http://mdacc.org/ClinicalLatha#JewishOrigin> ;
      label:creator foaf:JimLomax ;
      label:designNote "There is no concept of Sephardic Jew in the BioPortal"^^xsd:string ;
      skos-xl:prefLabel label:Sephardic_JewishOriginLabel .

<http://mdacc.org/ClinicalLatha#SerousCarcinoma>
      rdf:type owl:Class ;
      rdfs:comment "Serous carcinoma is an epithelial malignancy (carcinoma) that arises from the lining of a cavity that produces a serum-like fluid (a serous cavity)."^^xsd:string ;
      rdfs:subClassOf <http://mdacc.org/ClinicalLatha#Carcinoma> ;
      label:designNote "This concept is extensible."^^xsd:string , "This concept is not respresented in BioPortal (more specific serous carcinomas are represented)."^^xsd:string , "This concept may have instances of it's own or may be a superclass for concept refinements."^^xsd:string ;
      dc:creator foaf:JimLomax .

<http://mdacc.org/ClinicalLatha#SerousCavityAnatomicSite>
      rdf:type owl:Class ;
      rdfs:comment "General anatomical term that refers to a cavity that is enclosed by a serous membrane and contains serous fluid. Examples: pleural cavity, peritoneal cavity, subdeltoid bursa, synovial cavity of hip joint."^^xsd:string ;
      rdfs:subClassOf <http://mdacc.org/ClinicalLatha#AnatomicSite> ;
      label:correspondsTo label:SerousCavity_FMAURI , label:SerousCavity_SNOMEDURI ;
      label:designNote "This concept is directly related to the Serous Cavity concept in SNOMED and Foundation of Anatomy vocabularies"^^xsd:string , "This concept is extensible; more specific serous cavities."^^xsd:string , "This concept may have specific instances."^^xsd:string ;
      dc:creator foaf:JimLomax .

<http://mdacc.org/ClinicalLatha#Side>
      rdf:type owl:Class ;
      rdfs:comment "The concept of sidedness or position; left, right."^^xsd:string ;
      rdfs:subClassOf skos:Concept , <http://mdacc.org/ClinicalLatha#ClinicalPackage> ;
      rdfs:subClassOf
              [ rdf:type owl:Restriction ;
                owl:onProperty skos-xl:prefLabel ;
                owl:someValuesFrom label:SideLabel
              ] ;
      label:correspondsTo label:Side_NCIURI ;
      label:designNote "This concept directly corresponds to the concept of Side in NCI Thesaurus"^^xsd:string ;
      dc:creator foaf:JimLomax .

<http://mdacc.org/ClinicalLatha#SideLabel>
      rdf:type skos-xl:Label .

<http://mdacc.org/ClinicalLatha#SiteOfTumorFirstRecurrence>
      rdf:type owl:Class ;
      rdfs:subClassOf <http://mdacc.org/ClinicalLatha#ClinicalPackage> ;
      dc:creator foaf:JimLomax .

<http://mdacc.org/ClinicalLatha#SkinAnatomicSite>
      rdf:type owl:Class ;
      rdfs:subClassOf <http://mdacc.org/ClinicalLatha#AnatomicSite> ;
      label:correspondsTo label:Skin_NCIURI ;
      label:designNote "This concept is extensible; more specific anatomic location within the rectum."^^xsd:string , "This concept may have specific instances"^^xsd:string , "This concept is directly related to the Skin concept in NCI Thesaurus."^^xsd:string ;
      dc:creator foaf:JimLomax .

<http://mdacc.org/ClinicalLatha#SkinCancer>
      rdf:type owl:Class ;
      rdfs:subClassOf <http://mdacc.org/ClinicalLatha#Cancer> ;
      rdfs:subClassOf
              [ rdf:type owl:Restriction ;
                owl:onProperty <http://mdacc.org/ClinicalLatha#anatomicLocation> ;
                owl:someValuesFrom <http://mdacc.org/ClinicalLatha#SkinAnatomicSite>
              ] ;
      label:correspondsTo label:SkinCancer_MEDRAURI ;
      dc:creator foaf:JimLomax .

<http://mdacc.org/ClinicalLatha#SkinCancer_SkinCancer>
      rdf:type <http://mdacc.org/ClinicalLatha#SkinCancer> ;
      <http://mdacc.org/ClinicalLatha#anatomicLocation>
              <http://mdacc.org/ClinicalLatha#Skin_SkinAnatomicSite> ;
      label:correspondsTo label:SkinCancer_MEDRAURI ;
      label:creator foaf:JimLomax ;
      skos-xl:prefLabel label:SkinCancer_SkinCancerDiseaseLabel .

<http://mdacc.org/ClinicalLatha#SkinCutaneousMelanoma_SkinTumor>
      rdf:type <http://mdacc.org/ClinicalLatha#SkinTumor> ;
      <http://mdacc.org/ClinicalLatha#anatomicLocation>
              <http://mdacc.org/ClinicalLatha#Skin_SkinAnatomicSite> ;
      <http://mdacc.org/ClinicalLatha#manifestedBy>
              <http://mdacc.org/ClinicalLatha#SkinCancer_SkinCancer> ;
      skos-xl:prefLabel label:SkinCutaneousMelanoma_SkinTumorLabel .

<http://mdacc.org/ClinicalLatha#SkinTumor>
      rdf:type owl:Class ;
      rdfs:comment "Tumor anatomically located within Skin"^^xsd:string ;
      rdfs:subClassOf <http://mdacc.org/ClinicalLatha#TumorType> ;
      rdfs:subClassOf
              [ rdf:type owl:Restriction ;
                owl:onProperty <http://mdacc.org/ClinicalLatha#anatomicLocation> ;
                owl:someValuesFrom <http://mdacc.org/ClinicalLatha#SkinAnatomicSite>
              ] ;
      label:designNote "This concept is extensible."^^xsd:string , "This concept may have instances of it's own or may be a superclass for concept refinements."^^xsd:string ;
      dc:creator foaf:JimLomax .

<http://mdacc.org/ClinicalLatha#Skin_SkinAnatomicSite>
      rdf:type <http://mdacc.org/ClinicalLatha#SkinAnatomicSite> ;
      label:correspondsTo label:Skin_NCIURI ;
      label:creator foaf:JimLomax ;
      skos-xl:prefLabel label:Skin_AnatomicSiteLabel .

<http://mdacc.org/ClinicalLatha#Slide>
      rdf:type owl:Class ;
      rdfs:comment "A flat rectangular piece of glass on which specimens can be mounted for microscopic study."^^xsd:string , "We need a term for the slide analysis results, this concept will hold the quantitative values associated with each slide interpretation. For now I will leave this concept alone and add the slide result properties"^^xsd:string ;
      rdfs:subClassOf skos:Concept , <http://mdacc.org/ClinicalLatha#ClinicalPackage> ;
      label:correspondsTo label:Slide_NCIURI ;
      label:designNote "This concept is extensible."^^xsd:string , "This concept is directly related to the Slide concept in NCI Thesaurus."^^xsd:string , "This concept may have instances of it's own or may be a superclass for concept refinements."^^xsd:string ;
      dc:creator foaf:JimLomax .

<http://mdacc.org/ClinicalLatha#SquamousCellBladderCancer_BladderCancer>
      rdf:type <http://mdacc.org/ClinicalLatha#BladderCancer> ;
      rdfs:label "SquamousCellBladderCancer"^^xsd:string ;
      label:creator foaf:LathaRamdas .

<http://mdacc.org/ClinicalLatha#StableDisease_PrimaryTherapyOutcome>
      rdf:type <http://mdacc.org/ClinicalLatha#PrimaryTherapyOutcome> ;
      label:creator foaf:JimLomax ;
      skos-xl:prefLabel label:StableDisease_OutcomeLabel .

<http://mdacc.org/ClinicalLatha#Stage0TMNOVTumorStage>
      rdf:type owl:Class ;
      rdfs:subClassOf <http://mdacc.org/ClinicalLatha#TMNOVTumorStage> ;
      owl:equivalentClass
              [ rdf:type owl:Class ;
                owl:intersectionOf (<http://mdacc.org/ClinicalLatha#TumorStage> [ rdf:type owl:Restriction ;
                            owl:onProperty <http://mdacc.org/ClinicalLatha#cancer> ;
                            owl:someValuesFrom <http://mdacc.org/ClinicalLatha#OvarianCancer>
                          ] [ rdf:type owl:Restriction ;
                            owl:onProperty <http://mdacc.org/ClinicalLatha#diseaseStagingSystem> ;
                            owl:someValuesFrom <http://mdacc.org/ClinicalLatha#TNMDiseaseStagingSystem>
                          ] [ rdf:type owl:Restriction ;
                            owl:onProperty <http://mdacc.org/ClinicalLatha#finding> ;
                            owl:someValuesFrom <http://mdacc.org/ClinicalLatha#Stage0_PathologicPrimaryTumorTNMFinding>
                          ] [ rdf:type owl:Restriction ;
                            owl:onProperty <http://mdacc.org/ClinicalLatha#finding> ;
                            owl:someValuesFrom <http://mdacc.org/ClinicalLatha#Stage0_PathologicRegionalLymphNodesTNMFinding>
                          ] [ rdf:type owl:Restriction ;
                            owl:onProperty <http://mdacc.org/ClinicalLatha#finding> ;
                            owl:someValuesFrom <http://mdacc.org/ClinicalLatha#Stage0_PathologicDistantMetastasisTNMFinding>
                          ])
              ] .

<http://mdacc.org/ClinicalLatha#Stage0_PathologicDistantMetastasisTNMFinding>
      rdf:type owl:Class ;
      rdfs:comment "No morphologic evidence of distant metastasis, in accordance with TNM classification system guidelines."^^xsd:string ;
      rdfs:subClassOf <http://mdacc.org/ClinicalLatha#PathologicDistantMetastasisTNMFinding> ;
      label:correspondsTo label:pm0StagePathologicDistantMetastasisTNMFinding_NCIURI ;
      dc:creator foaf:JimLomax .

<http://mdacc.org/ClinicalLatha#Stage0_PathologicPrimaryTumorTNMFinding>
      rdf:type owl:Class ;
      rdfs:comment "No morphologic evidence of primary tumor, in accordance with TNM classification system guidelines."^^xsd:string ;
      rdfs:subClassOf <http://mdacc.org/ClinicalLatha#PathologicPrimaryTumorTNMFinding> ;
      label:correspondsTo label:pt0StagePathologicPrimaryTumorTNMFinding_NCIURI ;
      dc:creator foaf:JimLomax .

<http://mdacc.org/ClinicalLatha#Stage0_PathologicRegionalLymphNodesTNMFinding>
      rdf:type owl:Class ;
      rdfs:comment "No evidence of regional lymph node metastasis, in accordance with TNM classification system guidelines."^^xsd:string ;
      rdfs:subClassOf <http://mdacc.org/ClinicalLatha#PathologicRegionalLymphNodesTNMFinding> ;
      label:correspondsTo label:pn0StagePathologicRegionalLymphNodesTNMFinding_NCIURI ;
      dc:creator foaf:JimLomax .

<http://mdacc.org/ClinicalLatha#Stage1_PathologicDistantMetastasisTNMFinding>
      rdf:type owl:Class ;
      rdfs:comment "TNM stagingof the primary tumor"^^xsd:string ;
      rdfs:subClassOf <http://mdacc.org/ClinicalLatha#PathologicDistantMetastasisTNMFinding> ;
      label:correspondsTo label:pm1StagePathologicDistantMetastasisTNMFinding_NCIURI ;
      dc:creator foaf:JimLomax .

<http://mdacc.org/ClinicalLatha#Stage1_PathologicPrimaryTumorTNMFinding>
      rdf:type owl:Class ;
      rdfs:comment "TNM stagingof the primary tumor"^^xsd:string ;
      rdfs:subClassOf <http://mdacc.org/ClinicalLatha#PathologicPrimaryTumorTNMFinding> ;
      label:correspondsTo label:pt1StagePathologicPrimaryTumorTNMFinding_NCIURI ;
      dc:creator foaf:JimLomax .

<http://mdacc.org/ClinicalLatha#Stage1_PathologicRegionalLymphNodesTNMFinding>
      rdf:type owl:Class ;
      rdfs:comment "Comment placeholder"^^xsd:string ;
      rdfs:subClassOf <http://mdacc.org/ClinicalLatha#PathologicRegionalLymphNodesTNMFinding> ;
      label:correspondsTo label:pn1StagePathologicRegionalLymphNodesTNMFinding_NCIURI ;
      dc:creator foaf:JimLomax .

<http://mdacc.org/ClinicalLatha#Stage1aTMNOVTumorStage>
      rdf:type owl:Class ;
      rdfs:subClassOf <http://mdacc.org/ClinicalLatha#TMNOVTumorStage> ;
      owl:equivalentClass
              [ rdf:type owl:Class ;
                owl:intersectionOf (<http://mdacc.org/ClinicalLatha#TumorStage> [ rdf:type owl:Restriction ;
                            owl:onProperty <http://mdacc.org/ClinicalLatha#cancer> ;
                            owl:someValuesFrom <http://mdacc.org/ClinicalLatha#OvarianCancer>
                          ] [ rdf:type owl:Restriction ;
                            owl:onProperty <http://mdacc.org/ClinicalLatha#diseaseStagingSystem> ;
                            owl:someValuesFrom <http://mdacc.org/ClinicalLatha#TNMDiseaseStagingSystem>
                          ] [ rdf:type owl:Restriction ;
                            owl:onProperty <http://mdacc.org/ClinicalLatha#finding> ;
                            owl:someValuesFrom <http://mdacc.org/ClinicalLatha#Stage1a_PathologicPrimaryTumorTNMFinding>
                          ] [ rdf:type owl:Restriction ;
                            owl:onProperty <http://mdacc.org/ClinicalLatha#finding> ;
                            owl:someValuesFrom <http://mdacc.org/ClinicalLatha#Stage0_PathologicRegionalLymphNodesTNMFinding>
                          ] [ rdf:type owl:Restriction ;
                            owl:onProperty <http://mdacc.org/ClinicalLatha#finding> ;
                            owl:someValuesFrom <http://mdacc.org/ClinicalLatha#Stage0_PathologicDistantMetastasisTNMFinding>
                          ])
              ] .

<http://mdacc.org/ClinicalLatha#Stage1a_PathologicDistantMetastasisTNMFinding>
      rdf:type owl:Class ;
      rdfs:comment "TNM stagingof the primary tumor"^^xsd:string ;
      rdfs:subClassOf <http://mdacc.org/ClinicalLatha#Stage1_PathologicDistantMetastasisTNMFinding> ;
      label:correspondsTo label:pm1aStagePathologicDistantMetastasisTNMFinding_NCIURI ;
      dc:creator foaf:JimLomax .

<http://mdacc.org/ClinicalLatha#Stage1a_PathologicPrimaryTumorTNMFinding>
      rdf:type owl:Class ;
      rdfs:comment "TNM stagingof the primary tumor"^^xsd:string ;
      rdfs:subClassOf <http://mdacc.org/ClinicalLatha#Stage1_PathologicPrimaryTumorTNMFinding> ;
      label:correspondsTo label:pt1aStagePathologicPrimaryTumorTNMFinding_NCIURI ;
      dc:creator foaf:JimLomax .

<http://mdacc.org/ClinicalLatha#Stage1a_PathologicRegionalLymphNodesTNMFinding>
      rdf:type owl:Class ;
      rdfs:comment "Comment placeholder"^^xsd:string ;
      rdfs:subClassOf <http://mdacc.org/ClinicalLatha#Stage1_PathologicRegionalLymphNodesTNMFinding> ;
      label:correspondsTo label:pn1aStagePathologicRegionalLymphNodesTNMFinding_NCIURI ;
      dc:creator foaf:JimLomax .

<http://mdacc.org/ClinicalLatha#Stage1bTMNOVTumorStage>
      rdf:type owl:Class ;
      rdfs:subClassOf <http://mdacc.org/ClinicalLatha#TMNOVTumorStage> ;
      owl:equivalentClass
              [ rdf:type owl:Class ;
                owl:intersectionOf (<http://mdacc.org/ClinicalLatha#TumorStage> [ rdf:type owl:Restriction ;
                            owl:onProperty <http://mdacc.org/ClinicalLatha#cancer> ;
                            owl:someValuesFrom <http://mdacc.org/ClinicalLatha#OvarianCancer>
                          ] [ rdf:type owl:Restriction ;
                            owl:onProperty <http://mdacc.org/ClinicalLatha#diseaseStagingSystem> ;
                            owl:someValuesFrom <http://mdacc.org/ClinicalLatha#TNMDiseaseStagingSystem>
                          ] [ rdf:type owl:Restriction ;
                            owl:onProperty <http://mdacc.org/ClinicalLatha#finding> ;
                            owl:someValuesFrom <http://mdacc.org/ClinicalLatha#Stage1b_PathologicPrimaryTumorTNMFinding>
                          ] [ rdf:type owl:Restriction ;
                            owl:onProperty <http://mdacc.org/ClinicalLatha#finding> ;
                            owl:someValuesFrom <http://mdacc.org/ClinicalLatha#Stage0_PathologicRegionalLymphNodesTNMFinding>
                          ] [ rdf:type owl:Restriction ;
                            owl:onProperty <http://mdacc.org/ClinicalLatha#finding> ;
                            owl:someValuesFrom <http://mdacc.org/ClinicalLatha#Stage0_PathologicDistantMetastasisTNMFinding>
                          ])
              ] .

<http://mdacc.org/ClinicalLatha#Stage1b_PathologicDistantMetastasisTNMFinding>
      rdf:type owl:Class ;
      rdfs:comment "TNM stagingof the primary tumor"^^xsd:string ;
      rdfs:subClassOf <http://mdacc.org/ClinicalLatha#Stage1_PathologicDistantMetastasisTNMFinding> ;
      label:correspondsTo label:pm1bStagePathologicDistantMetastasisTNMFinding_NCIURI ;
      dc:creator foaf:JimLomax .

<http://mdacc.org/ClinicalLatha#Stage1b_PathologicPrimaryTumorTNMFinding>
      rdf:type owl:Class ;
      rdfs:comment "TNM stagingof the primary tumor"^^xsd:string ;
      rdfs:subClassOf <http://mdacc.org/ClinicalLatha#Stage1_PathologicPrimaryTumorTNMFinding> ;
      dc:creator foaf:JimLomax .

<http://mdacc.org/ClinicalLatha#Stage1b_PathologicRegionalLymphNodesTNMFinding>
      rdf:type owl:Class ;
      rdfs:comment "Comment placeholder"^^xsd:string ;
      rdfs:subClassOf <http://mdacc.org/ClinicalLatha#Stage1_PathologicRegionalLymphNodesTNMFinding> ;
      label:correspondsTo label:pn1bStagePathologicRegionalLymphNodesTNMFinding_NCIURI ;
      dc:creator foaf:JimLomax .

<http://mdacc.org/ClinicalLatha#Stage1cTMNOVTumorStage>
      rdf:type owl:Class ;
      rdfs:subClassOf <http://mdacc.org/ClinicalLatha#TMNOVTumorStage> ;
      owl:equivalentClass
              [ rdf:type owl:Class ;
                owl:intersectionOf (<http://mdacc.org/ClinicalLatha#TumorStage> [ rdf:type owl:Restriction ;
                            owl:onProperty <http://mdacc.org/ClinicalLatha#cancer> ;
                            owl:someValuesFrom <http://mdacc.org/ClinicalLatha#OvarianCancer>
                          ] [ rdf:type owl:Restriction ;
                            owl:onProperty <http://mdacc.org/ClinicalLatha#diseaseStagingSystem> ;
                            owl:someValuesFrom <http://mdacc.org/ClinicalLatha#TNMDiseaseStagingSystem>
                          ] [ rdf:type owl:Restriction ;
                            owl:onProperty <http://mdacc.org/ClinicalLatha#finding> ;
                            owl:someValuesFrom <http://mdacc.org/ClinicalLatha#Stage1c_PathologicPrimaryTumorTNMFinding>
                          ] [ rdf:type owl:Restriction ;
                            owl:onProperty <http://mdacc.org/ClinicalLatha#finding> ;
                            owl:someValuesFrom <http://mdacc.org/ClinicalLatha#Stage0_PathologicRegionalLymphNodesTNMFinding>
                          ] [ rdf:type owl:Restriction ;
                            owl:onProperty <http://mdacc.org/ClinicalLatha#finding> ;
                            owl:someValuesFrom <http://mdacc.org/ClinicalLatha#Stage0_PathologicDistantMetastasisTNMFinding>
                          ])
              ] .

<http://mdacc.org/ClinicalLatha#Stage1c_PathologicDistantMetastasisTNMFinding>
      rdf:type owl:Class ;
      rdfs:comment "TNM stagingof the primary tumor"^^xsd:string ;
      rdfs:subClassOf <http://mdacc.org/ClinicalLatha#Stage1_PathologicDistantMetastasisTNMFinding> ;
      label:correspondsTo label:pm1cStagePathologicDistantMetastasisTNMFinding_NCIURI ;
      dc:creator foaf:JimLomax .

<http://mdacc.org/ClinicalLatha#Stage1c_PathologicPrimaryTumorTNMFinding>
      rdf:type owl:Class ;
      rdfs:comment "TNM staging of the primary tumor"^^xsd:string ;
      rdfs:subClassOf <http://mdacc.org/ClinicalLatha#Stage1_PathologicPrimaryTumorTNMFinding> ;
      label:correspondsTo label:pt1cStagePathologicPrimaryTumorTNMFinding_NCIURI ;
      dc:creator foaf:JimLomax .

<http://mdacc.org/ClinicalLatha#Stage1c_PathologicRegionalLymphNodesTNMFinding>
      rdf:type owl:Class ;
      rdfs:comment "Comment placeholder"^^xsd:string ;
      rdfs:subClassOf <http://mdacc.org/ClinicalLatha#Stage1_PathologicRegionalLymphNodesTNMFinding> ;
      label:correspondsTo label:pn1cStagePathologicRegionalLymphNodesTNMFinding_NCIURI ;
      dc:creator foaf:JimLomax .

<http://mdacc.org/ClinicalLatha#Stage2_PathologicPrimaryTumorTNMFinding>
      rdf:type owl:Class ;
      rdfs:comment "TNM stagingof the primary tumor"^^xsd:string ;
      rdfs:subClassOf <http://mdacc.org/ClinicalLatha#PathologicPrimaryTumorTNMFinding> ;
      label:correspondsTo label:pt2StagePathologicPrimaryTumorTNMFinding_NCIURI ;
      dc:creator foaf:JimLomax .

<http://mdacc.org/ClinicalLatha#Stage2_PathologicRegionalLymphNodesTNMFinding>
      rdf:type owl:Class ;
      rdfs:comment "Comment placeholder"^^xsd:string ;
      rdfs:subClassOf <http://mdacc.org/ClinicalLatha#PathologicRegionalLymphNodesTNMFinding> ;
      label:correspondsTo label:pn2StagePathologicRegionalLymphNodesTNMFinding_NCIURI ;
      dc:creator foaf:JimLomax .

<http://mdacc.org/ClinicalLatha#Stage2aTMNOVTumorStage>
      rdf:type owl:Class ;
      rdfs:subClassOf <http://mdacc.org/ClinicalLatha#TMNOVTumorStage> ;
      owl:equivalentClass
              [ rdf:type owl:Class ;
                owl:intersectionOf (<http://mdacc.org/ClinicalLatha#TumorStage> [ rdf:type owl:Restriction ;
                            owl:onProperty <http://mdacc.org/ClinicalLatha#cancer> ;
                            owl:someValuesFrom <http://mdacc.org/ClinicalLatha#OvarianCancer>
                          ] [ rdf:type owl:Restriction ;
                            owl:onProperty <http://mdacc.org/ClinicalLatha#diseaseStagingSystem> ;
                            owl:someValuesFrom <http://mdacc.org/ClinicalLatha#TNMDiseaseStagingSystem>
                          ] [ rdf:type owl:Restriction ;
                            owl:onProperty <http://mdacc.org/ClinicalLatha#finding> ;
                            owl:someValuesFrom <http://mdacc.org/ClinicalLatha#Stage2a_PathologicPrimaryTumorTNMFinding>
                          ] [ rdf:type owl:Restriction ;
                            owl:onProperty <http://mdacc.org/ClinicalLatha#finding> ;
                            owl:someValuesFrom <http://mdacc.org/ClinicalLatha#Stage0_PathologicRegionalLymphNodesTNMFinding>
                          ] [ rdf:type owl:Restriction ;
                            owl:onProperty <http://mdacc.org/ClinicalLatha#finding> ;
                            owl:someValuesFrom <http://mdacc.org/ClinicalLatha#Stage0_PathologicDistantMetastasisTNMFinding>
                          ])
              ] .

<http://mdacc.org/ClinicalLatha#Stage2a_PathologicPrimaryTumorTNMFinding>
      rdf:type owl:Class ;
      rdfs:comment "TNM stagingof the primary tumor"^^xsd:string ;
      rdfs:subClassOf <http://mdacc.org/ClinicalLatha#Stage2_PathologicPrimaryTumorTNMFinding> ;
      label:correspondsTo label:pt2aStagePathologicPrimaryTumorTNMFinding_NCIURI ;
      dc:creator foaf:JimLomax .

<http://mdacc.org/ClinicalLatha#Stage2a_PathologicRegionalLymphNodesTNMFinding>
      rdf:type owl:Class ;
      rdfs:comment "Comment placeholder"^^xsd:string ;
      rdfs:subClassOf <http://mdacc.org/ClinicalLatha#Stage2_PathologicRegionalLymphNodesTNMFinding> ;
      label:correspondsTo label:pn2aStagePathologicRegionalLymphNodesTNMFinding_NCIURI ;
      dc:creator foaf:JimLomax .

<http://mdacc.org/ClinicalLatha#Stage2bTMNOVTumorStage>
      rdf:type owl:Class ;
      rdfs:subClassOf <http://mdacc.org/ClinicalLatha#TMNOVTumorStage> ;
      owl:equivalentClass
              [ rdf:type owl:Class ;
                owl:intersectionOf (<http://mdacc.org/ClinicalLatha#TumorStage> [ rdf:type owl:Restriction ;
                            owl:onProperty <http://mdacc.org/ClinicalLatha#cancer> ;
                            owl:someValuesFrom <http://mdacc.org/ClinicalLatha#OvarianCancer>
                          ] [ rdf:type owl:Restriction ;
                            owl:onProperty <http://mdacc.org/ClinicalLatha#diseaseStagingSystem> ;
                            owl:someValuesFrom <http://mdacc.org/ClinicalLatha#TNMDiseaseStagingSystem>
                          ] [ rdf:type owl:Restriction ;
                            owl:onProperty <http://mdacc.org/ClinicalLatha#finding> ;
                            owl:someValuesFrom <http://mdacc.org/ClinicalLatha#Stage2b_PathologicPrimaryTumorTNMFinding>
                          ] [ rdf:type owl:Restriction ;
                            owl:onProperty <http://mdacc.org/ClinicalLatha#finding> ;
                            owl:someValuesFrom <http://mdacc.org/ClinicalLatha#Stage0_PathologicRegionalLymphNodesTNMFinding>
                          ] [ rdf:type owl:Restriction ;
                            owl:onProperty <http://mdacc.org/ClinicalLatha#finding> ;
                            owl:someValuesFrom <http://mdacc.org/ClinicalLatha#Stage0_PathologicDistantMetastasisTNMFinding>
                          ])
              ] .

<http://mdacc.org/ClinicalLatha#Stage2b_PathologicPrimaryTumorTNMFinding>
      rdf:type owl:Class ;
      rdfs:comment "TNM stagingof the primary tumor"^^xsd:string ;
      rdfs:subClassOf <http://mdacc.org/ClinicalLatha#Stage2_PathologicPrimaryTumorTNMFinding> ;
      label:correspondsTo label:pt2bStagePathologicPrimaryTumorTNMFinding_NCIURI ;
      dc:creator foaf:JimLomax .

<http://mdacc.org/ClinicalLatha#Stage2b_PathologicRegionalLymphNodesTNMFinding>
      rdf:type owl:Class ;
      rdfs:comment "Comment placeholder"^^xsd:string ;
      rdfs:subClassOf <http://mdacc.org/ClinicalLatha#Stage2_PathologicRegionalLymphNodesTNMFinding> ;
      label:correspondsTo label:pn2bStagePathologicRegionalLymphNodesTNMFinding_NCIURI ;
      dc:creator foaf:JimLomax .

<http://mdacc.org/ClinicalLatha#Stage2cTMNOVTumorStage>
      rdf:type owl:Class ;
      rdfs:subClassOf <http://mdacc.org/ClinicalLatha#TMNOVTumorStage> ;
      owl:equivalentClass
              [ rdf:type owl:Class ;
                owl:intersectionOf (<http://mdacc.org/ClinicalLatha#TumorStage> [ rdf:type owl:Restriction ;
                            owl:onProperty <http://mdacc.org/ClinicalLatha#cancer> ;
                            owl:someValuesFrom <http://mdacc.org/ClinicalLatha#OvarianCancer>
                          ] [ rdf:type owl:Restriction ;
                            owl:onProperty <http://mdacc.org/ClinicalLatha#diseaseStagingSystem> ;
                            owl:someValuesFrom <http://mdacc.org/ClinicalLatha#TNMDiseaseStagingSystem>
                          ] [ rdf:type owl:Restriction ;
                            owl:onProperty <http://mdacc.org/ClinicalLatha#finding> ;
                            owl:someValuesFrom <http://mdacc.org/ClinicalLatha#Stage2c_PathologicPrimaryTumorTNMFinding>
                          ] [ rdf:type owl:Restriction ;
                            owl:onProperty <http://mdacc.org/ClinicalLatha#finding> ;
                            owl:someValuesFrom <http://mdacc.org/ClinicalLatha#Stage0_PathologicRegionalLymphNodesTNMFinding>
                          ] [ rdf:type owl:Restriction ;
                            owl:onProperty <http://mdacc.org/ClinicalLatha#finding> ;
                            owl:someValuesFrom <http://mdacc.org/ClinicalLatha#Stage0_PathologicDistantMetastasisTNMFinding>
                          ])
              ] .

<http://mdacc.org/ClinicalLatha#Stage2c_PathologicPrimaryTumorTNMFinding>
      rdf:type owl:Class ;
      rdfs:comment "TNM stagingof the primary tumor"^^xsd:string ;
      rdfs:subClassOf <http://mdacc.org/ClinicalLatha#Stage2_PathologicPrimaryTumorTNMFinding> ;
      label:correspondsTo label:pt2cStagePathologicPrimaryTumorTNMFinding_NCIURI ;
      dc:creator foaf:JimLomax .

<http://mdacc.org/ClinicalLatha#Stage2c_PathologicRegionalLymphNodesTNMFinding>
      rdf:type owl:Class ;
      rdfs:comment "Comment placeholder"^^xsd:string ;
      rdfs:subClassOf <http://mdacc.org/ClinicalLatha#Stage2_PathologicRegionalLymphNodesTNMFinding> ;
      label:correspondsTo label:pn2cStagePathologicRegionalLymphNodesTNMFinding_NCIURI ;
      dc:creator foaf:JimLomax .

<http://mdacc.org/ClinicalLatha#Stage3_PathologicPrimaryTumorTNMFinding>
      rdf:type owl:Class ;
      rdfs:comment "TNM stagingof the primary tumor"^^xsd:string ;
      rdfs:subClassOf <http://mdacc.org/ClinicalLatha#PathologicPrimaryTumorTNMFinding> ;
      label:correspondsTo label:pt3StagePathologicPrimaryTumorTNMFinding_NCIURI ;
      dc:creator foaf:JimLomax .

<http://mdacc.org/ClinicalLatha#Stage3_PathologicRegionalLymphNodesTNMFinding>
      rdf:type owl:Class ;
      rdfs:comment "Comment placeholder"^^xsd:string ;
      rdfs:subClassOf <http://mdacc.org/ClinicalLatha#PathologicRegionalLymphNodesTNMFinding> ;
      label:correspondsTo label:pn3StagePathologicRegionalLymphNodesTNMFinding_NCIURI ;
      dc:creator foaf:JimLomax .

<http://mdacc.org/ClinicalLatha#Stage3aTMNOVTumorStage>
      rdf:type owl:Class ;
      rdfs:subClassOf <http://mdacc.org/ClinicalLatha#TMNOVTumorStage> ;
      owl:equivalentClass
              [ rdf:type owl:Class ;
                owl:intersectionOf (<http://mdacc.org/ClinicalLatha#TumorStage> [ rdf:type owl:Restriction ;
                            owl:onProperty <http://mdacc.org/ClinicalLatha#cancer> ;
                            owl:someValuesFrom <http://mdacc.org/ClinicalLatha#OvarianCancer>
                          ] [ rdf:type owl:Restriction ;
                            owl:onProperty <http://mdacc.org/ClinicalLatha#diseaseStagingSystem> ;
                            owl:someValuesFrom <http://mdacc.org/ClinicalLatha#TNMDiseaseStagingSystem>
                          ] [ rdf:type owl:Restriction ;
                            owl:onProperty <http://mdacc.org/ClinicalLatha#finding> ;
                            owl:someValuesFrom <http://mdacc.org/ClinicalLatha#Stage3a_PathologicPrimaryTumorTNMFinding>
                          ] [ rdf:type owl:Restriction ;
                            owl:onProperty <http://mdacc.org/ClinicalLatha#finding> ;
                            owl:someValuesFrom <http://mdacc.org/ClinicalLatha#Stage0_PathologicRegionalLymphNodesTNMFinding>
                          ] [ rdf:type owl:Restriction ;
                            owl:onProperty <http://mdacc.org/ClinicalLatha#finding> ;
                            owl:someValuesFrom <http://mdacc.org/ClinicalLatha#Stage0_PathologicDistantMetastasisTNMFinding>
                          ])
              ] .

<http://mdacc.org/ClinicalLatha#Stage3a_PathologicPrimaryTumorTNMFinding>
      rdf:type owl:Class ;
      rdfs:comment "TNM stagingof the primary tumor"^^xsd:string ;
      rdfs:subClassOf <http://mdacc.org/ClinicalLatha#Stage3_PathologicPrimaryTumorTNMFinding> ;
      label:correspondsTo label:pt3aStagePathologicPrimaryTumorTNMFinding_NCIURI ;
      dc:creator foaf:JimLomax .

<http://mdacc.org/ClinicalLatha#Stage3a_PathologicRegionalLymphNodesTNMFinding>
      rdf:type owl:Class ;
      rdfs:comment "Comment placeholder"^^xsd:string ;
      rdfs:subClassOf <http://mdacc.org/ClinicalLatha#Stage3_PathologicRegionalLymphNodesTNMFinding> ;
      label:correspondsTo label:pn3aStagePathologicRegionalLymphNodesTNMFinding_NCIURI ;
      dc:creator foaf:JimLomax .

<http://mdacc.org/ClinicalLatha#Stage3bTMNOVTumorStage>
      rdf:type owl:Class ;
      rdfs:subClassOf <http://mdacc.org/ClinicalLatha#TMNOVTumorStage> ;
      owl:equivalentClass
              [ rdf:type owl:Class ;
                owl:intersectionOf (<http://mdacc.org/ClinicalLatha#TumorStage> [ rdf:type owl:Restriction ;
                            owl:onProperty <http://mdacc.org/ClinicalLatha#cancer> ;
                            owl:someValuesFrom <http://mdacc.org/ClinicalLatha#OvarianCancer>
                          ] [ rdf:type owl:Restriction ;
                            owl:onProperty <http://mdacc.org/ClinicalLatha#diseaseStagingSystem> ;
                            owl:someValuesFrom <http://mdacc.org/ClinicalLatha#TNMDiseaseStagingSystem>
                          ] [ rdf:type owl:Restriction ;
                            owl:onProperty <http://mdacc.org/ClinicalLatha#finding> ;
                            owl:someValuesFrom <http://mdacc.org/ClinicalLatha#Stage3b_PathologicPrimaryTumorTNMFinding>
                          ] [ rdf:type owl:Restriction ;
                            owl:onProperty <http://mdacc.org/ClinicalLatha#finding> ;
                            owl:someValuesFrom <http://mdacc.org/ClinicalLatha#Stage0_PathologicRegionalLymphNodesTNMFinding>
                          ] [ rdf:type owl:Restriction ;
                            owl:onProperty <http://mdacc.org/ClinicalLatha#finding> ;
                            owl:someValuesFrom <http://mdacc.org/ClinicalLatha#Stage0_PathologicDistantMetastasisTNMFinding>
                          ])
              ] .

<http://mdacc.org/ClinicalLatha#Stage3b_PathologicPrimaryTumorTNMFinding>
      rdf:type owl:Class ;
      rdfs:comment "TNM stagingof the primary tumor"^^xsd:string ;
      rdfs:subClassOf <http://mdacc.org/ClinicalLatha#Stage3_PathologicPrimaryTumorTNMFinding> ;
      label:correspondsTo label:pt3bStagePathologicPrimaryTumorTNMFinding_NCIURI ;
      dc:creator foaf:JimLomax .

<http://mdacc.org/ClinicalLatha#Stage3b_PathologicRegionalLymphNodesTNMFinding>
      rdf:type owl:Class ;
      rdfs:comment "Comment placeholder"^^xsd:string ;
      rdfs:subClassOf <http://mdacc.org/ClinicalLatha#Stage3_PathologicRegionalLymphNodesTNMFinding> ;
      label:correspondsTo label:pn3bStagePathologicRegionalLymphNodesTNMFinding_NCIURI ;
      dc:creator foaf:JimLomax .

<http://mdacc.org/ClinicalLatha#Stage3cTMNOVTumorStage>
      rdf:type owl:Class ;
      rdfs:subClassOf <http://mdacc.org/ClinicalLatha#TMNOVTumorStage> ;
      owl:equivalentClass
              [ rdf:type owl:Class ;
                owl:intersectionOf (<http://mdacc.org/ClinicalLatha#TumorStage> [ rdf:type owl:Restriction ;
                            owl:onProperty <http://mdacc.org/ClinicalLatha#cancer> ;
                            owl:someValuesFrom <http://mdacc.org/ClinicalLatha#OvarianCancer>
                          ] [ rdf:type owl:Restriction ;
                            owl:onProperty <http://mdacc.org/ClinicalLatha#diseaseStagingSystem> ;
                            owl:someValuesFrom <http://mdacc.org/ClinicalLatha#TNMDiseaseStagingSystem>
                          ] [ rdf:type owl:Class ;
                            owl:unionOf ([ rdf:type owl:Class ;
                                        owl:intersectionOf ([ rdf:type owl:Restriction ;
                                                    owl:onProperty <http://mdacc.org/ClinicalLatha#finding> ;
                                                    owl:someValuesFrom <http://mdacc.org/ClinicalLatha#Stage3b_PathologicPrimaryTumorTNMFinding>
                                                  ] [ rdf:type owl:Restriction ;
                                                    owl:onProperty <http://mdacc.org/ClinicalLatha#finding> ;
                                                    owl:someValuesFrom <http://mdacc.org/ClinicalLatha#Stage0_PathologicRegionalLymphNodesTNMFinding>
                                                  ] [ rdf:type owl:Restriction ;
                                                    owl:onProperty <http://mdacc.org/ClinicalLatha#finding> ;
                                                    owl:someValuesFrom <http://mdacc.org/ClinicalLatha#Stage0_PathologicDistantMetastasisTNMFinding>
                                                  ])
                                      ] [ rdf:type owl:Class ;
                                        owl:intersectionOf ([ rdf:type owl:Restriction ;
                                                    owl:onProperty <http://mdacc.org/ClinicalLatha#finding> ;
                                                    owl:someValuesFrom <http://mdacc.org/ClinicalLatha#Stage1_PathologicRegionalLymphNodesTNMFinding>
                                                  ] [ rdf:type owl:Restriction ;
                                                    owl:onProperty <http://mdacc.org/ClinicalLatha#finding> ;
                                                    owl:someValuesFrom <http://mdacc.org/ClinicalLatha#Stage0_PathologicDistantMetastasisTNMFinding>
                                                  ])
                                      ])
                          ])
              ] .

<http://mdacc.org/ClinicalLatha#Stage3c_PathologicPrimaryTumorTNMFinding>
      rdf:type owl:Class ;
      rdfs:comment "TNM stagingof the primary tumor"^^xsd:string ;
      rdfs:subClassOf <http://mdacc.org/ClinicalLatha#Stage3_PathologicPrimaryTumorTNMFinding> ;
      label:correspondsTo label:pt3cStagePathologicPrimaryTumorTNMFinding_NCIURI ;
      dc:creator foaf:JimLomax .

<http://mdacc.org/ClinicalLatha#Stage3c_PathologicRegionalLymphNodesTNMFinding>
      rdf:type owl:Class ;
      rdfs:comment "Comment placeholder"^^xsd:string ;
      rdfs:subClassOf <http://mdacc.org/ClinicalLatha#Stage3_PathologicRegionalLymphNodesTNMFinding> ;
      label:correspondsTo label:pn3cStagePathologicRegionalLymphNodesTNMFinding_NCIURI ;
      dc:creator foaf:JimLomax .

<http://mdacc.org/ClinicalLatha#Stage4TMNOVTumorStage>
      rdf:type owl:Class ;
      rdfs:subClassOf <http://mdacc.org/ClinicalLatha#TMNOVTumorStage> ;
      owl:equivalentClass
              [ rdf:type owl:Class ;
                owl:intersectionOf (<http://mdacc.org/ClinicalLatha#TumorStage> [ rdf:type owl:Restriction ;
                            owl:onProperty <http://mdacc.org/ClinicalLatha#cancer> ;
                            owl:someValuesFrom <http://mdacc.org/ClinicalLatha#OvarianCancer>
                          ] [ rdf:type owl:Restriction ;
                            owl:onProperty <http://mdacc.org/ClinicalLatha#diseaseStagingSystem> ;
                            owl:someValuesFrom <http://mdacc.org/ClinicalLatha#TNMDiseaseStagingSystem>
                          ] [ rdf:type owl:Restriction ;
                            owl:onProperty <http://mdacc.org/ClinicalLatha#finding> ;
                            owl:someValuesFrom <http://mdacc.org/ClinicalLatha#Stage1_PathologicDistantMetastasisTNMFinding>
                          ])
              ] .

<http://mdacc.org/ClinicalLatha#Stage4_PathologicPrimaryTumorTNMFinding>
      rdf:type owl:Class ;
      rdfs:comment "TNM stagingof the primary tumor"^^xsd:string ;
      rdfs:subClassOf <http://mdacc.org/ClinicalLatha#PathologicPrimaryTumorTNMFinding> ;
      label:correspondsTo label:pt4StagePathologicPrimaryTumorTNMFinding_NCIURI ;
      dc:creator foaf:JimLomax .

<http://mdacc.org/ClinicalLatha#Stage4a_PathologicPrimaryTumorTNMFinding>
      rdf:type owl:Class ;
      rdfs:comment "TNM stagingof the primary tumor"^^xsd:string ;
      rdfs:subClassOf <http://mdacc.org/ClinicalLatha#Stage4_PathologicPrimaryTumorTNMFinding> ;
      label:correspondsTo label:pt4aStagePathologicPrimaryTumorTNMFinding_NCIURI ;
      dc:creator foaf:JimLomax .

<http://mdacc.org/ClinicalLatha#Stage4b_PathologicPrimaryTumorTNMFinding>
      rdf:type owl:Class ;
      rdfs:comment "TNM stagingof the primary tumor"^^xsd:string ;
      rdfs:subClassOf <http://mdacc.org/ClinicalLatha#Stage4_PathologicPrimaryTumorTNMFinding> ;
      label:correspondsTo label:pt4bStagePathologicPrimaryTumorTNMFinding_NCIURI ;
      dc:creator foaf:JimLomax .

<http://mdacc.org/ClinicalLatha#Stage4c_PathologicPrimaryTumorTNMFinding>
      rdf:type owl:Class ;
      rdfs:comment "TNM stagingof the primary tumor"^^xsd:string ;
      rdfs:subClassOf <http://mdacc.org/ClinicalLatha#Stage4_PathologicPrimaryTumorTNMFinding> ;
      label:correspondsTo label:pt4cStagePathologicPrimaryTumorTNMFinding_NCIURI ;
      dc:creator foaf:JimLomax .

<http://mdacc.org/ClinicalLatha#Stage4d_PathologicPrimaryTumorTNMFinding>
      rdf:type owl:Class ;
      rdfs:comment "TNM stagingof the primary tumor"^^xsd:string ;
      rdfs:subClassOf <http://mdacc.org/ClinicalLatha#Stage4_PathologicPrimaryTumorTNMFinding> ;
      label:correspondsTo label:pt4dStagePathologicPrimaryTumorTNMFinding_NCIURI ;
      dc:creator foaf:JimLomax .

<http://mdacc.org/ClinicalLatha#StomachAdenocarcinoma_StomachTumor>
      rdf:type <http://mdacc.org/ClinicalLatha#StomachTumor> ;
      <http://mdacc.org/ClinicalLatha#anatomicLocation>
              <http://mdacc.org/ClinicalLatha#Stomach_StomachAnatomicSite> ;
      <http://mdacc.org/ClinicalLatha#manifestedBy>
              <http://mdacc.org/ClinicalLatha#StomachCancer_StomachCancer> ;
      label:correspondsTo label:StomachAdenocarcinoma_NCIURI ;
      label:creator foaf:JimLomax ;
      skos-xl:prefLabel label:StomachAdenocarcinoma_StomachTumorLabel .

<http://mdacc.org/ClinicalLatha#StomachAnatomicSite>
      rdf:type owl:Class ;
      rdfs:subClassOf <http://mdacc.org/ClinicalLatha#AnatomicSite> ;
      label:correspondsTo label:Stomach_NCIURI ;
      label:designNote "This concept is extensible; more specific anatomic location within the stomach."^^xsd:string , "This concept may have specific instances"^^xsd:string , "This concept is directly related to the Stomach concept in NCI Thesaurus."^^xsd:string ;
      dc:creator foaf:JimLomax .

<http://mdacc.org/ClinicalLatha#StomachCancer>
      rdf:type owl:Class ;
      rdfs:subClassOf <http://mdacc.org/ClinicalLatha#Cancer> ;
      rdfs:subClassOf
              [ rdf:type owl:Restriction ;
                owl:onProperty <http://mdacc.org/ClinicalLatha#anatomicLocation> ;
                owl:someValuesFrom <http://mdacc.org/ClinicalLatha#StomachAnatomicSite>
              ] ;
      label:correspondsTo label:StomachCancer_MEDRAURI ;
      dc:creator foaf:JimLomax .

<http://mdacc.org/ClinicalLatha#StomachCancer_StomachCancer>
      rdf:type <http://mdacc.org/ClinicalLatha#StomachCancer> ;
      <http://mdacc.org/ClinicalLatha#anatomicLocation>
              <http://mdacc.org/ClinicalLatha#Stomach_StomachAnatomicSite> ;
      label:correspondsTo label:StomachCancer_MEDRAURI ;
      label:creator foaf:JimLomax ;
      skos-xl:prefLabel label:StomachCancer_StomachCancerDiseaseLabel .

<http://mdacc.org/ClinicalLatha#StomachTumor>
      rdf:type owl:Class ;
      rdfs:comment "Tumor anatomically located within Stomach"^^xsd:string ;
      rdfs:subClassOf <http://mdacc.org/ClinicalLatha#TumorType> ;
      rdfs:subClassOf
              [ rdf:type owl:Restriction ;
                owl:onProperty <http://mdacc.org/ClinicalLatha#anatomicLocation> ;
                owl:someValuesFrom <http://mdacc.org/ClinicalLatha#StomachAnatomicSite>
              ] ;
      label:designNote "This concept is extensible."^^xsd:string , "This concept may have instances of it's own or may be a superclass for concept refinements."^^xsd:string ;
      dc:creator foaf:JimLomax .

<http://mdacc.org/ClinicalLatha#Stomach_StomachAnatomicSite>
      rdf:type <http://mdacc.org/ClinicalLatha#StomachAnatomicSite> ;
      rdfs:comment "LR:  Please correct the skos-xl:preflabel"^^xsd:string ;
      label:correspondsTo label:Skin_NCIURI ;
      label:creator foaf:JimLomax ;
      skos-xl:prefLabel label:Skin_AnatomicSiteLabel .

<http://mdacc.org/ClinicalLatha#SurgicalProcedure>
      rdf:type owl:Class ;
      rdfs:comment "A procedure to remove or repair a part of the body or to find out whether disease is present. An operation."^^xsd:string ;
      rdfs:subClassOf skos:Concept , <http://mdacc.org/ClinicalLatha#ClinicalPackage> ;
      rdfs:subClassOf
              [ rdf:type owl:Restriction ;
                owl:onProperty skos-xl:prefLabel ;
                owl:someValuesFrom label:SurgicalProcedureLabel
              ] ;
      rdfs:subClassOf
              [ rdf:type owl:Restriction ;
                owl:onProperty dc:identifier ;
                owl:someValuesFrom xsd:string
              ] ;
      label:correspondsTo label:SurgicalProcedure_NCIURI ;
      label:designNote "This concept is extensible."^^xsd:string , "This concept is directly related to the Surgical Procedure concept in NCI Thesaurus."^^xsd:string , "This concept may have instances of it's own or may be a superclass for concept refinements."^^xsd:string ;
      dc:creator foaf:JimLomax .

<http://mdacc.org/ClinicalLatha#SurgicalProcedure1_SurgicalProcedure>
      rdf:type <http://mdacc.org/ClinicalLatha#SurgicalProcedure> ;
      dc:identifier "Generic Surgery"^^xsd:string .

<http://mdacc.org/ClinicalLatha#TCell>
      rdf:type owl:Class ;
      rdfs:comment "A lymphocyte derived from a pre T-lymphocyte in the thymus and stored in secondary lymphoid organs, bone marrow, and lymph nodes. It circulates in the bloodstream and the lymphatic system, where it searches for and attacks particular foreign or abnormal cells. A mature T lymphocyte has T cell receptors and other surface proteins on its cell surface."^^xsd:string ;
      rdfs:subClassOf <http://mdacc.org/ClinicalLatha#Lymphocyte> ;
      label:correspondsTo label:TLymphocyte_NCIURI ;
      label:designNote "This concept is directly related to the T Cell concept in NCI Thesaurus"^^xsd:string , "This concept is extensible."^^xsd:string , "This concept may have instances of it's own or may be a superclass for concept refinements."^^xsd:string ;
      dc:creator foaf:JimLomax .

<http://mdacc.org/ClinicalLatha#TIF>
      rdf:type <http://mdacc.org/ClinicalLatha#ImageFormat> .

<http://mdacc.org/ClinicalLatha#TMNOVTumorStage>
      rdf:type owl:Class ;
      rdfs:subClassOf <http://mdacc.org/ClinicalLatha#OVTumorStage> ;
      rdfs:subClassOf
              [ rdf:type owl:Restriction ;
                owl:onProperty <http://mdacc.org/ClinicalLatha#diseaseStagingSystem> ;
                owl:someValuesFrom <http://mdacc.org/ClinicalLatha#TNMDiseaseStagingSystem>
              ] ;
      rdfs:subClassOf
              [ rdf:type owl:Restriction ;
                owl:onProperty <http://mdacc.org/ClinicalLatha#cancer> ;
                owl:someValuesFrom <http://mdacc.org/ClinicalLatha#OvarianCancer>
              ] .

<http://mdacc.org/ClinicalLatha#TNMDiseaseStagingSystem>
      rdf:type owl:Class ;
      rdfs:comment "A systematic method for clinicopathologic evaluation of tumors. The TNM staging system is a general framework with some guidelines for classification, however the system can, and in most cases must be made more specific to be useful. Materialization of a TMN system can specific to a cancer type, institutional, pathologist or clinician requirements. For example the TNM classification system for lung cancer (small cell carcinoma) is very well defined. However, this does not mean that a specific pathologist will follow the classification guidelines."^^xsd:string ;
      rdfs:subClassOf <http://mdacc.org/ClinicalLatha#DiseaseStagingSystem> ;
      rdfs:subClassOf
              [ rdf:type owl:Restriction ;
                owl:onProperty <http://mdacc.org/ClinicalLatha#disease> ;
                owl:someValuesFrom <http://mdacc.org/ClinicalLatha#Disease>
              ] ;
      rdfs:subClassOf
              [ rdf:type owl:Restriction ;
                owl:onProperty <http://mdacc.org/ClinicalLatha#specifier> ;
                owl:someValuesFrom foaf:Agent
              ] ;
      label:correspondsTo label:TNMStagingSystem_NCIURI ;
      label:designNote "This concept is extensible."^^xsd:string , "specifier property should come from Oraganization Package"^^xsd:string , "This concept is directly related to the TNM Disease Staging System concept in NCI Thesaurus"^^xsd:string ;
      dc:creator foaf:JimLomax .

<http://mdacc.org/ClinicalLatha#TNMOvarianNeoplasmStagingSystem>
      rdf:type owl:Class ;
      rdfs:comment "A system for specific evaluation of tumors of the ovaries."^^xsd:string ;
      rdfs:subClassOf <http://mdacc.org/ClinicalLatha#TNMDiseaseStagingSystem> ;
      rdfs:subClassOf
              [ rdf:type owl:Restriction ;
                owl:onProperty <http://mdacc.org/ClinicalLatha#cancer> ;
                owl:someValuesFrom
                        [ rdf:type owl:Class ;
                          owl:unionOf (<http://mdacc.org/ClinicalLatha#OvarianCancer> <http://mdacc.org/ClinicalLatha#OvarianSerousCarcinoma>)
                        ]
              ] ;
      label:designNote "THis concept may be demoted to instance"^^xsd:string , "This concept could not be found in BioPortal"^^xsd:string ;
      dc:creator foaf:JimLomax .

<http://mdacc.org/ClinicalLatha#TargetedMolecularTherapy>
      rdf:type owl:Class ;
      rdfs:comment "Cancer therapies designed to act upon specific molecules in metabolic pathways or processes involved in carcinogenesis, tumor growth, or tumor spread."^^xsd:string ;
      rdfs:subClassOf <http://mdacc.org/ClinicalLatha#DrugTherapy> ;
      rdfs:subClassOf
              [ rdf:type owl:Restriction ;
                owl:onProperty <http://mdacc.org/ClinicalLatha#administersTherapeuticAgent> ;
                owl:someValuesFrom <http://mdacc.org/Drug#TargetedMolecularTherapyDrug>
              ] ;
      label:correspondsTo label:TargetedMolecularTherapy_NCIURI ;
      label:designNote "This concept is extensible."^^xsd:string , "This concept is directly related to the Targeted Molecular Therapy concept in NCI Thesaurus."^^xsd:string , "This concept may have instances of it's own or may be a superclass for concept refinements."^^xsd:string ;
      dc:creator foaf:JimLomax .

<http://mdacc.org/ClinicalLatha#TargetedMolecularTherapyExistentialEvent>
      rdf:type owl:Class ;
      rdfs:comment "This concept represents the existential nature of a targeted molecular therapy; the concept is not concerned with spatio-temporal aspects of the event, only that it occurred."^^xsd:string ;
      rdfs:subClassOf <http://mdacc.org/ClinicalLatha#TherapeuticProcedureExistentialEvent> ;
      label:designNote "This concept may be domoted to an instance"^^xsd:string , "This existential concept is a product of TCGA's need to capture just the existence of a targeted molecular therapy."^^xsd:string , "This concept is related to the Targeted Molecular Therapy concept under Therapeutic Procedure"^^xsd:string ;
      dc:creator foaf:JimLomax .

<http://mdacc.org/ClinicalLatha#TargetedMolecularTherapy_TherapeuticProcedure>
      rdf:type <http://mdacc.org/ClinicalLatha#TargetedMolecularTherapy> .

<http://mdacc.org/ClinicalLatha#Taxomifen_175mgm2_TherapeuticPrescription>
      rdf:type <http://mdacc.org/ClinicalLatha#TherapeuticPrescription> ;
      <http://mdacc.org/ClinicalLatha#administersTherapeuticAgent>
              <http://mdacc.org/Drug#Taxomifen_ChemotherapyDrug> ;
      <http://mdacc.org/ClinicalLatha#dosage>
              <http://mdacc.org/ClinicalLatha#MgM2_175_Dosage> .

<http://mdacc.org/ClinicalLatha#Taxomifen_Chemotherapy>
      rdf:type <http://mdacc.org/ClinicalLatha#Chemotherapy> ;
      <http://mdacc.org/ClinicalLatha#administersTherapeuticAgent>
              <http://mdacc.org/Drug#Taxomifen_ChemotherapyDrug> ;
      <http://mdacc.org/ClinicalLatha#dosage>
              <http://mdacc.org/ClinicalLatha#MgM2_175_Dosage> ;
      <http://mdacc.org/ClinicalLatha#therapeuticDelivery>
              <http://mdacc.org/ClinicalLatha#Intravenous_TherapeuticAgentDelivery> ;
      label:creator foaf:JimLomax ;
      label:notes "Notes on the therapy"^^xsd:string .

<http://mdacc.org/ClinicalLatha#Temozolomide_Chemotherapy>
      rdf:type <http://mdacc.org/ClinicalLatha#Chemotherapy> ;
      <http://mdacc.org/ClinicalLatha#administersTherapeuticAgent>
              <http://mdacc.org/Drug#Temozolomide_ChemotherapyDrug> ;
      <http://mdacc.org/ClinicalLatha#dosage>
              <http://mdacc.org/ClinicalLatha#MgM2_175_Dosage> ;
      <http://mdacc.org/ClinicalLatha#initialCourse>
              <http://mdacc.org/ClinicalLatha#TrueExample_InitialCourseEvent> ;
      <http://mdacc.org/ClinicalLatha#numberOfCycles>
              3 ;
      label:creator foaf:JimLomax ;
      temporal:endedOn temporal:DrugTreatment1_EndDateTime ;
      temporal:numberOfDaysToTherapyEnd
              "44"^^xsd:int ;
      temporal:numberOfDaysToTherapyStart
              "23"^^xsd:int ;
      temporal:startedOn temporal:DrugTreatment1_StartDateTime .

<http://mdacc.org/ClinicalLatha#Template>
      rdf:type spin:SelectTemplate ;
      rdfs:subClassOf spin:SelectTemplates .

<http://mdacc.org/ClinicalLatha#TenM_Concentration>
      rdf:type <http://mdacc.org/ClinicalLatha#Concentration> ;
      <http://mdacc.org/ClinicalLatha#units>
              <http://mdacc.org/ClinicalLatha#Molarity_ConcentrationUnits> ;
      <http://mdacc.org/ClinicalLatha#value>
              "10"^^xsd:string .

<http://mdacc.org/ClinicalLatha#TesticularCancer>
      rdf:type owl:Class ;
      rdfs:label "Testicular cancer"^^xsd:string ;
      rdfs:subClassOf <http://mdacc.org/ClinicalLatha#Cancer> ;
      label:creator foaf:LathaRamdas .

<http://mdacc.org/ClinicalLatha#TesticularCancer_TesticularCancer>
      rdf:type <http://mdacc.org/ClinicalLatha#TesticularCancer> ;
      rdfs:label "Testicular Cancer"^^xsd:string .

<http://mdacc.org/ClinicalLatha#TherapeuticAgent>
      rdf:type owl:Class ;
      rdfs:comment "The action or administration of therapeutic agents to produce an effect that is intended to alter the course of a pathologic process."^^xsd:string ;
      rdfs:subClassOf skos:Concept , <http://mdacc.org/ClinicalLatha#ClinicalPackage> ;
      rdfs:subClassOf
              [ rdf:type owl:Restriction ;
                owl:onProperty skos-xl:prefLabel ;
                owl:someValuesFrom label:TherapeuticAgentLabel
              ] ;
      label:correspondsTo label:TherapeuticProcedure_NCIURI ;
      label:designNote "This concept is extensible."^^xsd:string , "This concept is directly related to the Therapeutic Procedure concept in NCI Thesaurus."^^xsd:string , "This concept may have instances of it's own or may be a superclass for concept refinements."^^xsd:string ;
      dc:creator foaf:JimLomax .

<http://mdacc.org/ClinicalLatha#TherapeuticAgentDelivery>
      rdf:type owl:Class ;
      rdfs:comment "The route of administration for therapeutic agents."^^xsd:string ;
      rdfs:subClassOf skos:Concept , <http://mdacc.org/ClinicalLatha#ClinicalPackage> ;
      rdfs:subClassOf
              [ rdf:type owl:Restriction ;
                owl:onProperty skos-xl:prefLabel ;
                owl:someValuesFrom label:TherapeuticAgentDeliveryLabel
              ] ;
      label:designNote "This concept is extensible."^^xsd:string , "This concept may have instances of it's own or may be a superclass for concept refinements."^^xsd:string ;
      dc:creator foaf:JimLomax .

<http://mdacc.org/ClinicalLatha#TherapeuticPrescription>
      rdf:type owl:Class ;
      rdfs:comment "The action or administration of therapeutic agents to produce an effect that is intended to alter the course of a pathologic process."^^xsd:string ;
      rdfs:subClassOf skos:Concept , <http://mdacc.org/ClinicalLatha#ClinicalPackage> ;
      rdfs:subClassOf
              [ rdf:type owl:Restriction ;
                owl:maxCardinality "1"^^xsd:int ;
                owl:onProperty <http://mdacc.org/ClinicalLatha#administersTherapeuticAgent>
              ] ;
      rdfs:subClassOf
              [ rdf:type owl:Restriction ;
                owl:onProperty <http://mdacc.org/ClinicalLatha#administersTherapeuticAgent> ;
                owl:someValuesFrom <http://mdacc.org/ClinicalLatha#TherapeuticAgent>
              ] ;
      rdfs:subClassOf
              [ rdf:type owl:Restriction ;
                owl:maxCardinality "1"^^xsd:int ;
                owl:onProperty <http://mdacc.org/ClinicalLatha#dosage>
              ] ;
      rdfs:subClassOf
              [ rdf:type owl:Restriction ;
                owl:onProperty <http://mdacc.org/ClinicalLatha#dosage> ;
                owl:someValuesFrom <http://mdacc.org/ClinicalLatha#Dosage>
              ] ;
      label:designNote "A therapeutic prescription is the pairing of a therapeutic agent and its dosage."^^xsd:string ;
      dc:creator foaf:JimLomax .

<http://mdacc.org/ClinicalLatha#TherapeuticProcedure>
      rdf:type owl:Class ;
      rdfs:comment "The action or administration of therapeutic agents to produce an effect that is intended to alter the course of a pathologic process."^^xsd:string ;
      rdfs:subClassOf skos:Concept , <http://mdacc.org/ClinicalLatha#ClinicalPackage> ;
      rdfs:subClassOf
              [ rdf:type owl:Restriction ;
                owl:onProperty skos-xl:prefLabel ;
                owl:someValuesFrom label:TherapeuticProcedureLabel
              ] ;
      label:correspondsTo label:TherapeuticProcedure_NCIURI ;
      label:designNote "This concept is extensible."^^xsd:string , "This concept is directly related to the Therapeutic Procedure concept in NCI Thesaurus."^^xsd:string , "This concept may have instances of it's own or may be a superclass for concept refinements."^^xsd:string ;
      dc:creator foaf:JimLomax .

<http://mdacc.org/ClinicalLatha#TherapeuticProcedureExistentialEvent>
      rdf:type owl:Class ;
      rdfs:subClassOf <http://mdacc.org/ClinicalLatha#ExistentialEvent> ;
      rdfs:subClassOf
              [ rdf:type owl:Restriction ;
                owl:cardinality "1"^^xsd:int ;
                owl:onProperty <http://mdacc.org/ClinicalLatha#occurred>
              ] ;
      rdfs:subClassOf
              [ rdf:type owl:Restriction ;
                owl:onProperty <http://mdacc.org/ClinicalLatha#occurred> ;
                owl:someValuesFrom xsd:boolean
              ] ;
      label:creator foaf:JimLomax ;
      label:designNote "The existential event captures whether or not it occurred."^^xsd:string .

<http://mdacc.org/ClinicalLatha#TherapeuticProcedureList1_Item_Chemotherapy1>
      rdf:type collections:ListItem ;
      collections:itemContent
              <http://mdacc.org/ClinicalLatha#Taxomifen_Chemotherapy> ;
      collections:nextItem
              <http://mdacc.org/ClinicalLatha#TherapeuticProcedureList1_Item_Chemotherpay2> .

<http://mdacc.org/ClinicalLatha#TherapeuticProcedureList1_Item_Chemotherpay2>
      rdf:type collections:ListItem ;
      collections:itemContent
              <http://mdacc.org/ClinicalLatha#Temozolomide_Chemotherapy> ;
      collections:nextItem
              <http://mdacc.org/ClinicalLatha#TherapeuticProcedureList1_Item_Radiation1> .

<http://mdacc.org/ClinicalLatha#TherapeuticProcedureList1_Item_Radiation1>
      rdf:type collections:ListItem ;
      collections:itemContent
              <http://mdacc.org/ClinicalLatha#TargetedMolecularTherapy_TherapeuticProcedure> .

<http://mdacc.org/ClinicalLatha#TherapeuticProcedureOutcome>
      rdf:type owl:Class ;
      rdfs:comment "The result of a therpeutic procedure (therapy). There are most likely members to this concept that are defined by NCI Thesaurus."^^xsd:string ;
      rdfs:subClassOf <http://mdacc.org/ClinicalLatha#Outcome> ;
      rdfs:subClassOf
              [ rdf:type owl:Restriction ;
                owl:onProperty <http://mdacc.org/ClinicalLatha#outcomeOf> ;
                owl:someValuesFrom <http://mdacc.org/ClinicalLatha#TherapeuticProcedure>
              ] ;
      label:correspondsTo label:TherapeuticProcedureOutcome_NCIURI ;
      label:designNote "This concept is extensible."^^xsd:string , "This concept is directly related to the Therapeutic Procedure Outcome concept in NCI Thesaurus."^^xsd:string , "This concept may have instances of it's own or may be a superclass for concept refinements."^^xsd:string ;
      dc:creator foaf:JimLomax .

<http://mdacc.org/ClinicalLatha#TherpaeuticProcedures1_Collection>
      rdf:type collections:List ;
      collections:firstItem
              <http://mdacc.org/ClinicalLatha#TherapeuticProcedureList1_Item_Chemotherapy1> ;
      collections:lastItem
              <http://mdacc.org/ClinicalLatha#TherapeuticProcedureList1_Item_Radiation1> .

<http://mdacc.org/ClinicalLatha#TherpaeuticProcedures1_Collection_1>
      rdf:type collections:List ;
      collections:firstItem
              <http://mdacc.org/ClinicalLatha#TherapeuticProcedureList1_Item_Chemotherapy1> ;
      collections:lastItem
              <http://mdacc.org/ClinicalLatha#TherapeuticProcedureList1_Item_Radiation1> .

<http://mdacc.org/ClinicalLatha#ThreeM_Concentration>
      rdf:type <http://mdacc.org/ClinicalLatha#Concentration> ;
      <http://mdacc.org/ClinicalLatha#units>
              <http://mdacc.org/ClinicalLatha#Molarity_ConcentrationUnits> ;
      <http://mdacc.org/ClinicalLatha#value>
              "3"^^xsd:string .

<http://mdacc.org/ClinicalLatha#ThyroidAnatomicSite>
      rdf:type owl:Class ;
      rdfs:comment "LR:  Please correct the label:correspondsTo"^^xsd:string ;
      rdfs:subClassOf <http://mdacc.org/ClinicalLatha#AnatomicSite> ;
      label:correspondsTo label:Stomach_NCIURI ;
      label:designNote "This concept is extensible; more specific anatomic location within the thyroid."^^xsd:string , "This concept may have specific instances"^^xsd:string , "This concept is directly related to the Thyroid concept in NCI Thesaurus."^^xsd:string ;
      dc:creator foaf:JimLomax .

<http://mdacc.org/ClinicalLatha#ThyroidCancer>
      rdf:type owl:Class ;
      rdfs:subClassOf <http://mdacc.org/ClinicalLatha#Cancer> ;
      rdfs:subClassOf
              [ rdf:type owl:Restriction ;
                owl:onProperty <http://mdacc.org/ClinicalLatha#anatomicLocation> ;
                owl:someValuesFrom <http://mdacc.org/ClinicalLatha#ThyroidAnatomicSite>
              ] ;
      label:correspondsTo label:ThyroidCancer_MEDRAURI ;
      label:creator foaf:JimLomax .

<http://mdacc.org/ClinicalLatha#ThyroidCancer_ThyroidCancer>
      rdf:type <http://mdacc.org/ClinicalLatha#ThyroidCancer> ;
      <http://mdacc.org/ClinicalLatha#anatomicLocation>
              <http://mdacc.org/ClinicalLatha#Thyroid_ThyroidAnatomicSite> ;
      label:correspondsTo label:ThyroidCancer_MEDRAURI ;
      label:creator foaf:JimLomax ;
      skos-xl:prefLabel label:ThyroidCancer_ThyroidCancerDiseaseLabel .

<http://mdacc.org/ClinicalLatha#ThyroidCarcinoma_ThyroidTumor>
      rdf:type <http://mdacc.org/ClinicalLatha#ThyroidTumor> ;
      <http://mdacc.org/ClinicalLatha#anatomicLocation>
              <http://mdacc.org/ClinicalLatha#Thyroid_ThyroidAnatomicSite> ;
      <http://mdacc.org/ClinicalLatha#manifestedBy>
              <http://mdacc.org/ClinicalLatha#ThyroidCancer_ThyroidCancer> ;
      label:correspondsTo label:ThyroidCarcinoma_NCIURI ;
      label:creator foaf:JimLomax ;
      skos-xl:prefLabel label:ThyroidCarcinoma_ThyroidTumorLabel .

<http://mdacc.org/ClinicalLatha#ThyroidTumor>
      rdf:type owl:Class ;
      rdfs:comment "Tumor anatomically located within Thyroid"^^xsd:string ;
      rdfs:subClassOf <http://mdacc.org/ClinicalLatha#TumorType> ;
      rdfs:subClassOf
              [ rdf:type owl:Restriction ;
                owl:onProperty <http://mdacc.org/ClinicalLatha#anatomicLocation> ;
                owl:someValuesFrom <http://mdacc.org/ClinicalLatha#ThyroidAnatomicSite>
              ] ;
      label:designNote "This concept is extensible."^^xsd:string , "This concept may have instances of it's own or may be a superclass for concept refinements."^^xsd:string ;
      dc:creator foaf:JimLomax .

<http://mdacc.org/ClinicalLatha#Thyroid_ThyroidAnatomicSite>
      rdf:type <http://mdacc.org/ClinicalLatha#ThyroidAnatomicSite> ;
      label:correspondsTo label:Thyroid_NCIURI ;
      label:creator foaf:JimLomax ;
      skos-xl:prefLabel label:Thyroid_AnatomicSiteLabel .

<http://mdacc.org/ClinicalLatha#Tissue>
      rdf:type owl:Class ;
      rdfs:comment "A group or layer of cells that are alike and that work together to perform a specific function."^^xsd:string ;
      rdfs:subClassOf <http://mdacc.org/ClinicalLatha#BioMaterial> ;
      rdfs:subClassOf
              [ rdf:type owl:Restriction ;
                owl:onProperty <http://mdacc.org/ClinicalLatha#composedOf> ;
                owl:someValuesFrom <http://mdacc.org/ClinicalLatha#Cell>
              ] ;
      label:correspondsTo label:Tissue_NCIURI ;
      label:designNote "This concept is extensible; there are different types of tissues (connective, nerve, muscle, etc.) each of which will have different properties."^^xsd:string , "This concept is directly related to the Tissue concept in NCI Thesaurus."^^xsd:string , "Tissues are composed of cells of the same type."^^xsd:string , "This concept may have instances of it's own or may be a superclass for concept refinements."^^xsd:string ;
      dc:creator foaf:JimLomax .

<http://mdacc.org/ClinicalLatha#TissueSamplesDisjoint>
      rdf:type rdfs:Class ;
      rdfs:subClassOf rdf:Statement .

<http://mdacc.org/ClinicalLatha#Top_Side>
      rdf:type <http://mdacc.org/ClinicalLatha#Side> ;
      label:creator foaf:JimLomax ;
      skos-xl:prefLabel label:Top_SideLabel .

<http://mdacc.org/ClinicalLatha#TotalRNA>
      rdf:type owl:Class ;
      rdfs:comment "Total RNA is a designation for a sample that contains all forms of RNA, not just mRNA, which is the most commonly collected."^^xsd:string ;
      rdfs:subClassOf <http://mdacc.org/ClinicalLatha#BioMaterial> ;
      label:designNote "There is no known corresponding concept of TotalRNA in BioPortal"^^xsd:string , "It is unclear if there are specific instance of Total RNA or if Total RNA is an instance of Bio Material"^^xsd:string ;
      dc:creator foaf:JimLomax .

<http://mdacc.org/ClinicalLatha#TranslationaCellBladderCancer_BladderCancer>
      rdf:type <http://mdacc.org/ClinicalLatha#BladderCancer> ;
      rdfs:comment "LR: cancer that begins in cells that normally make up the inner lining of the bladder - From NCI thesaurus"^^xsd:string ;
      rdfs:label "TranslationaCellBladder cancer"^^xsd:string ;
      <http://mdacc.org/ClinicalLatha#anatomicLocation>
              <http://mdacc.org/ClinicalLatha#Bladder_BladderAnatomicSite> ;
      <http://mdacc.org/ClinicalLatha#manifests>
              <http://mdacc.org/ClinicalLatha#BladderTumor_BladderTumor> ;
      label:creator foaf:LathaRamdas .

<http://mdacc.org/ClinicalLatha#Treatment>
      rdf:type owl:Class ;
      rdfs:comment "An action or administration of therapeutic agents to produce an effect that is intended to alter the course of a pathologic process."^^xsd:string ;
      rdfs:subClassOf <http://mdacc.org/ClinicalLatha#ClinicalPackage> ;
      dc:creator foaf:JimLomax ;
      owl:equivalentClass <http://mdacc.org/ClinicalLatha#TherapeuticProcedure> .

<http://mdacc.org/ClinicalLatha#TrueExample_InitialCourseEvent>
      rdf:type <http://mdacc.org/ClinicalLatha#InitialCourseExistentialEvent> ;
      <http://mdacc.org/ClinicalLatha#occurred>
              "true"^^xsd:boolean ;
      label:creator foaf:JimLomax .

<http://mdacc.org/ClinicalLatha#Tumor>
      rdf:type owl:Class ;
      rdfs:comment "An abnormal tissue growth resulted from uncontrolled cell proliferation"^^xsd:string ;
      rdfs:subClassOf skos:Concept , <http://mdacc.org/ClinicalLatha#ClinicalPackage> ;
      rdfs:subClassOf
              [ rdf:type owl:Restriction ;
                owl:onProperty <http://mdacc.org/ClinicalLatha#tumorClassification> ;
                owl:someValuesFrom <http://mdacc.org/ClinicalLatha#TumorType>
              ] ;
      rdfs:subClassOf
              [ rdf:type owl:Restriction ;
                owl:onProperty skos-xl:prefLabel ;
                owl:someValuesFrom label:TumorLabel
              ] ;
      label:architect foaf:MoSanyang ;
      label:creator foaf:JimLomax ;
      label:designNote "This concept is extensible."^^xsd:string , "This concept is directly related to the Tumor concept in NCI Thesaurus."^^xsd:string , "The concept is equivalent to neoplasm"^^xsd:string , "This concept may have instances of it's own or may be a superclass for concept refinements."^^xsd:string ;
      label:developer foaf:PradheepRaju , foaf:JimLomax , foaf:DawitGebremichael .

<http://mdacc.org/ClinicalLatha#TumorGrade>
      rdf:type owl:Class ;
      rdfs:comment "A tumor grade is a measure of how abnormal cancer cells appear and how fast they are growing."^^xsd:string , "Tumor grades cannot be designated universally; there are many different tumor grading systems, some involving only malignant tumor, other involving malignant and benign. Some are specific to an anatomic location. Not all tumor grading systems are respresented with the same tumor grade designations, however most of them use a single letter combined with a single number to indicate the (destructive) progression of the disease."^^xsd:string ;
      rdfs:subClassOf <http://mdacc.org/ClinicalLatha#ClinicalPackage> ;
      rdfs:subClassOf
              [ rdf:type owl:Restriction ;
                owl:onProperty dc:identifier ;
                owl:someValuesFrom xsd:string
              ] ;
      label:designNote "There is no corresponding concept in BioPortal to represent a tumor grade outside of a particular grading system."^^xsd:string ;
      dc:creator foaf:JimLomax .

<http://mdacc.org/ClinicalLatha#TumorMarker>
      rdf:type owl:Class ;
      rdfs:comment "A substance present in or produced by a tumor or by the host, that can be used for differentiating neoplastic from normal tissue based on measurements in body fluids, secretions, cells, and/or tissues. Markers are used in diagnosis, staging and prognosis of cancer, provide an estimation of tumor burden, and serve for monitoring effects of therapy, detecting recurrence, localization of tumors, and screening in general populations."^^xsd:string ;
      rdfs:subClassOf <http://mdacc.org/ClinicalLatha#DiseaseMarker> ;
      label:correspondsTo label:TumorMarker_NCIURI ;
      label:designNote "This concept is extensible."^^xsd:string , "This concept is directly related to the Tumor Marker concept in NCI Thesaurus."^^xsd:string , "This concept may have instances of it's own or may be a superclass for concept refinements."^^xsd:string ;
      dc:creator foaf:JimLomax .

<http://mdacc.org/ClinicalLatha#TumorProgressionFinding>
      rdf:type owl:Class ;
      rdfs:comment "An indication that a tumor has progressed since its last observed state."^^xsd:string ;
      rdfs:subClassOf <http://mdacc.org/ClinicalLatha#Finding> ;
      label:correspondsTo label:CancerProgression_NCIURI ;
      label:designNote "This concept directly corresponds to the Cancer Progression concept in NCI Thesaurus."^^xsd:string ;
      dc:creator foaf:JimLomax .

<http://mdacc.org/ClinicalLatha#TumorRecurrenceFinding>
      rdf:type owl:Class ;
      rdfs:comment "An indication that a tumor has reappeared after having been in an indectable state."^^xsd:string ;
      rdfs:subClassOf <http://mdacc.org/ClinicalLatha#Finding> ;
      label:correspondsTo label:NeoplasmRecurrence_MEDRAURI ;
      label:designNote "This concept directly corresponds to the Neoplasm Recurrence concept in MEDRA."^^xsd:string ;
      dc:creator foaf:JimLomax .

<http://mdacc.org/ClinicalLatha#TumorResection_DiagnosticProcedure>
      rdf:type <http://mdacc.org/ClinicalLatha#DiagnosticProcedure> ;
      label:creator foaf:JimLomax ;
      skos-xl:prefLabel label:TumorResection_DiagnosticProcedureLabel .

<http://mdacc.org/ClinicalLatha#TumorStage>
      rdf:type owl:Class ;
      rdfs:comment "This concept is extensible."^^xsd:string , "A tumor stage is a designation given to a particular incidence of cancer based on a particular staging scheme."^^xsd:string , "This concept may have instances of it's own or may be a superclass for concept refinements."^^xsd:string ;
      rdfs:subClassOf <http://mdacc.org/ClinicalLatha#ClinicalPackage> ;
      rdfs:subClassOf
              [ rdf:type owl:Restriction ;
                owl:onProperty dc:identifier ;
                owl:someValuesFrom xsd:string
              ] ;
      rdfs:subClassOf
              [ rdf:type owl:Restriction ;
                owl:onProperty <http://mdacc.org/ClinicalLatha#diseaseStagingSystem> ;
                owl:someValuesFrom <http://mdacc.org/ClinicalLatha#DiseaseStagingSystem>
              ] ;
      rdfs:subClassOf
              [ rdf:type owl:Restriction ;
                owl:onProperty <http://mdacc.org/ClinicalLatha#cancer> ;
                owl:someValuesFrom <http://mdacc.org/ClinicalLatha#Cancer>
              ] ;
      label:correspondsTo label:TumorStage_SNOMEDURI ;
      label:designNote "This concept is directly related to the Tumor Stage concept in NCI Thesaurus."^^xsd:string ;
      dc:creator foaf:JimLomax .

<http://mdacc.org/ClinicalLatha#TumorTissueSite>
      rdf:type owl:Class ;
      rdfs:comment "The tissue site? of a tumor"^^xsd:string ;
      rdfs:subClassOf <http://mdacc.org/ClinicalLatha#ClinicalPackage> ;
      label:domainQuestion
              "Is this the same as anatomic location?"^^xsd:string ;
      dc:creator foaf:JimLomax .

<http://mdacc.org/ClinicalLatha#TumorType>
      rdf:type owl:Class ;
      rdfs:comment "An abnormal tissue growth resulted from uncontrolled cell proliferation"^^xsd:string ;
      rdfs:subClassOf skos:Concept , <http://mdacc.org/ClinicalLatha#ClinicalPackage> ;
      rdfs:subClassOf
              [ rdf:type owl:Restriction ;
                owl:onProperty <http://mdacc.org/ClinicalLatha#manifestedBy> ;
                owl:someValuesFrom <http://mdacc.org/ClinicalLatha#Cancer>
              ] ;
      rdfs:subClassOf
              [ rdf:type owl:Restriction ;
                owl:onProperty skos-xl:prefLabel ;
                owl:someValuesFrom label:TumorLabel
              ] ;
      label:architect foaf:MoSanyang ;
      label:creator foaf:JimLomax ;
      label:designNote "This concept is extensible."^^xsd:string , "This concept is directly related to the Tumor concept in NCI Thesaurus."^^xsd:string , "The concept is equivalent to neoplasm"^^xsd:string , "This concept may have instances of it's own or may be a superclass for concept refinements."^^xsd:string ;
      label:developer foaf:PradheepRaju , foaf:JimLomax , foaf:DawitGebremichael .

<http://mdacc.org/ClinicalLatha#TwentyThreeGray_RadiationDosage>
      rdf:type <http://mdacc.org/ClinicalLatha#RadiationDosage> ;
      <http://mdacc.org/ClinicalLatha#units>
              <http://mdacc.org/ClinicalLatha#Gray_DosageUnits> ;
      <http://mdacc.org/ClinicalLatha#value>
              "23"^^xsd:string .

<http://mdacc.org/ClinicalLatha#TwoPills_Dosage>
      rdf:type <http://mdacc.org/ClinicalLatha#DrugDosage> ;
      <http://mdacc.org/ClinicalLatha#units>
              <http://mdacc.org/ClinicalLatha#Pill_DosageUnits> ;
      <http://mdacc.org/ClinicalLatha#value>
              "2"^^xsd:string .

<http://mdacc.org/ClinicalLatha#UnitOfMeasure>
      rdf:type owl:Class ;
      rdfs:comment "A named quantity in terms of which other quantities are measured or specified, used as a standard measurement of like kinds."^^xsd:string ;
      rdfs:subClassOf skos:Concept , <http://mdacc.org/ClinicalLatha#ClinicalPackage> ;
      rdfs:subClassOf
              [ rdf:type owl:Restriction ;
                owl:onProperty skos-xl:prefLabel ;
                owl:someValuesFrom label:UnitsLabel
              ] ;
      label:domainQuestion
              "Is this Units?"^^xsd:string ;
      dc:creator foaf:JimLomax .

<http://mdacc.org/ClinicalLatha#Units>
      rdf:type owl:Class ;
      rdfs:comment "A named quantity in terms of which other quantities are measured or specified, used as a standard measurement of like kinds."^^xsd:string ;
      rdfs:subClassOf skos:Concept , <http://mdacc.org/ClinicalLatha#ClinicalPackage> ;
      rdfs:subClassOf
              [ rdf:type owl:Restriction ;
                owl:onProperty skos-xl:prefLabel ;
                owl:someValuesFrom label:UnitsLabel
              ] ;
      label:correspondsTo label:Unit_NCIURI ;
      label:designNote "This concept is directly related to the Units concept in NCI Thesaurus."^^xsd:string ;
      dc:creator foaf:JimLomax ;
      owl:equivalentClass <http://mdacc.org/ClinicalLatha#UnitOfMeasure> .

<http://mdacc.org/ClinicalLatha#UterineCancer>
      rdf:type owl:Class ;
      rdfs:subClassOf <http://mdacc.org/ClinicalLatha#Cancer> ;
      rdfs:subClassOf
              [ rdf:type owl:Restriction ;
                owl:onProperty <http://mdacc.org/ClinicalLatha#anatomicLocation> ;
                owl:someValuesFrom <http://mdacc.org/ClinicalLatha#UterusAnatomicSite>
              ] ;
      label:correspondsTo label:UterineCancer_MEDRAURI ;
      label:creator foaf:JimLomax .

<http://mdacc.org/ClinicalLatha#UterineCancer_UterineCancer>
      rdf:type <http://mdacc.org/ClinicalLatha#UterineCancer> ;
      <http://mdacc.org/ClinicalLatha#anatomicLocation>
              <http://mdacc.org/ClinicalLatha#Uterus_UterusAnatomicSite> ;
      label:correspondsTo label:UterineCancer_MEDRAURI ;
      label:creator foaf:JimLomax ;
      skos-xl:prefLabel label:UterineCancer_UterineCancerDiseaseLabel .

<http://mdacc.org/ClinicalLatha#UterineCorpusEndometrioidCarcinoma_UterineCancer>
      rdf:type <http://mdacc.org/ClinicalLatha#UterineTumor> ;
      <http://mdacc.org/ClinicalLatha#anatomicLocation>
              <http://mdacc.org/ClinicalLatha#Uterus_UterusAnatomicSite> ;
      <http://mdacc.org/ClinicalLatha#manifestedBy>
              <http://mdacc.org/ClinicalLatha#UterineCancer_UterineCancer> ;
      label:creator foaf:JimLomax ;
      skos-xl:prefLabel label:UterineEndometrioidCarcinoma_UterineTumorLabel .

<http://mdacc.org/ClinicalLatha#UterineTumor>
      rdf:type owl:Class ;
      rdfs:comment "Tumor anatomically located within Uterus"^^xsd:string ;
      rdfs:subClassOf <http://mdacc.org/ClinicalLatha#TumorType> ;
      rdfs:subClassOf
              [ rdf:type owl:Restriction ;
                owl:onProperty <http://mdacc.org/ClinicalLatha#anatomicLocation> ;
                owl:someValuesFrom <http://mdacc.org/ClinicalLatha#UterusAnatomicSite>
              ] ;
      label:designNote "This concept is extensible."^^xsd:string , "This concept may have instances of it's own or may be a superclass for concept refinements."^^xsd:string ;
      dc:creator foaf:JimLomax .

<http://mdacc.org/ClinicalLatha#UterusAnatomicSite>
      rdf:type owl:Class ;
      rdfs:subClassOf <http://mdacc.org/ClinicalLatha#AnatomicSite> ;
      label:correspondsTo label:Uterus_NCIURI ;
      label:designNote "This concept is extensible; more specific anatomic location within the uterus."^^xsd:string , "This concept may have specific instances"^^xsd:string , "This concept is directly related to the Uterus concept in NCI Thesaurus."^^xsd:string ;
      dc:creator foaf:JimLomax .

<http://mdacc.org/ClinicalLatha#Uterus_UterusAnatomicSite>
      rdf:type <http://mdacc.org/ClinicalLatha#UterusAnatomicSite> ;
      label:correspondsTo label:Uterus_NCIURI ;
      label:creator foaf:JimLomax ;
      skos-xl:prefLabel label:Uterus_AnatomicSiteLabel .

<http://mdacc.org/ClinicalLatha#Virus>
      rdf:type owl:Class ;
      rdfs:comment "A virus is a small infectious agent that can replicate only inside the living cells of organisms"^^xsd:string ;
      rdfs:subClassOf <http://mdacc.org/ClinicalLatha#BioMaterial> ;
      label:correspondsTo label:Virus_NCIURI ;
      label:designNote "This concept is directly related to the Virus concept in NCI Thesaurus."^^xsd:string , "This concept is extensible; there are different types of viruses each of which will have different properties."^^xsd:string , "This concept may have instances of it's own or may be a superclass for concept refinements."^^xsd:string ;
      dc:creator foaf:JimLomax .

<http://mdacc.org/ClinicalLatha#VitalStatus>
      rdf:type owl:Class ;
      rdfs:comment "Indicates a vital status of a subject; living or not."^^xsd:string ;
      rdfs:subClassOf <http://mdacc.org/ClinicalLatha#PopulationCharacteristic> ;
      rdfs:subClassOf
              [ rdf:type owl:Restriction ;
                owl:onProperty skos-xl:prefLabel ;
                owl:someValuesFrom label:VitalStatusLabel
              ] ;
      dc:creator foaf:JimLomax .

<http://mdacc.org/ClinicalLatha#Volume>
      rdf:type owl:Class ;
      rdfs:subClassOf <http://mdacc.org/ClinicalLatha#Quantity> ;
      rdfs:subClassOf
              [ rdf:type owl:Restriction ;
                owl:onProperty skos-xl:prefLabel ;
                owl:someValuesFrom label:VolumeLabel
              ] ;
      label:designNote "This concept is extensible."^^xsd:string , "This concept may have instances of it's own or may be a superclass for concept refinements."^^xsd:string ;
      dc:creator foaf:JimLomax .

<http://mdacc.org/ClinicalLatha#VolumeUnits>
      rdf:type owl:Class ;
      rdfs:subClassOf <http://mdacc.org/ClinicalLatha#Units> ;
      label:creator foaf:JimLomax .

<http://mdacc.org/ClinicalLatha#Weight>
      rdf:type owl:Class ;
      rdfs:comment "The vertical force exerted by a mass as a result of gravity"^^xsd:string ;
      rdfs:subClassOf <http://mdacc.org/ClinicalLatha#Quantity> ;
      rdfs:subClassOf
              [ rdf:type owl:Restriction ;
                owl:onProperty skos-xl:prefLabel ;
                owl:someValuesFrom label:WeightLabel
              ] ;
      label:correspondsTo label:Weight_NCIURI ;
      label:designNote "This concept is extensible."^^xsd:string , "This concept is directly related to the Weight concept in NCI Thesaurus."^^xsd:string , "This concept may have instances of it's own or may be a superclass for concept refinements."^^xsd:string ;
      dc:creator foaf:JimLomax .

<http://mdacc.org/ClinicalLatha#WeightUnits>
      rdf:type owl:Class ;
      rdfs:subClassOf <http://mdacc.org/ClinicalLatha#Units> ;
      label:creator foaf:JimLomax .

<http://mdacc.org/ClinicalLatha#WhiteBloodCell>
      rdf:type owl:Class ;
      rdfs:subClassOf <http://mdacc.org/ClinicalLatha#Cell> ;
      dc:creator foaf:JimLomax ;
      owl:equivalentClass <http://mdacc.org/ClinicalLatha#Leukocyte> .

<http://mdacc.org/ClinicalLatha#White_Adipocyte>
      rdf:type <http://mdacc.org/ClinicalLatha#Adipocyte> ;
      rdfs:comment "Fat cells with light coloration and few mitochondria. They contain a scant ring of cytoplasm surrounding a single large lipid droplet or vacuole."^^xsd:string ;
      label:correspondsTo label:WhiteAdipocyte_MESHURI ;
      label:creator foaf:JimLomax ;
      label:designNote "This instance directly corresponds to the Brown Apidocyte concept in MESH."^^xsd:string .

<http://mdacc.org/ClinicalLatha#White_Race>
      rdf:type <http://mdacc.org/ClinicalLatha#Race> ;
      label:correspondsTo label:WhiteRace_NCIURI ;
      label:designNote "This concept is directly related to the White/Caucasian Race concept in NCI Thesaurus."^^xsd:string ;
      dc:creator foaf:JimLomax .

<http://mdacc.org/ClinicalLatha#WilmsTumor_KidneyTumor>
      rdf:type <http://mdacc.org/ClinicalLatha#KidneyTumor> ;
      rdfs:comment "LR: An embryonal neoplasm characterized by the presence of epithelial, mesenchymal, and blastema components.  The vast majority of cases arise from the kidney.  A small number of cases with morphologic features resembling Wilms tumor of the kidney have been reported arising from the ovary and the cervix. NCI Thesaurus"^^xsd:string ;
      rdfs:label "Wilm's tumor_Kidney tumor"^^xsd:string ;
      <http://mdacc.org/ClinicalLatha#anatomicLocation>
              <http://mdacc.org/ClinicalLatha#Kidney_KidneyAnatomicSite> ;
      <http://mdacc.org/ClinicalLatha#manifestedBy>
              <http://mdacc.org/ClinicalLatha#Kidney_KidneyCancer> ;
      label:creator foaf:LathaRamdas .

<http://mdacc.org/ClinicalLatha#aDNAPreparation_Protocol>
      rdf:type <http://mdacc.org/ClinicalLatha#Protocol> ;
      archive:fileLocation
              archive:ExampleProtocol_FileLocation ;
      <http://mdacc.org/ClinicalLatha#protocolType>
              <http://mdacc.org/ClinicalLatha#aDNA_Preparation_Type_ProtocolType> ;
      dc:identifier "aDNA Preparation Protocol"^^xsd:string ;
      skos-xl:prefLabel label:aDNAPreparation_ProtocolLabel .

<http://mdacc.org/ClinicalLatha#aDNA_Preparation_Type_ProtocolType>
      rdf:type <http://mdacc.org/ClinicalLatha#ProtocolType> ;
      dc:identifier "aDNA Preparation Type"^^xsd:string ;
      skos-xl:prefLabel label:aDNAPreparation_ProtocolTypeLabel .

<http://mdacc.org/ClinicalLatha#accessionNumberOf>
      rdf:type owl:ObjectProperty ;
      rdfs:subPropertyOf <http://mdacc.org/ClinicalLatha#hasAccessionNumber> .

<http://mdacc.org/ClinicalLatha#administeredBy>
      rdf:type owl:ObjectProperty .

<http://mdacc.org/ClinicalLatha#administers>
      rdf:type owl:ObjectProperty ;
      owl:inverseOf <http://mdacc.org/ClinicalLatha#administeredBy> .

<http://mdacc.org/ClinicalLatha#administersTherapeuticAgent>
      rdf:type owl:ObjectProperty ;
      rdfs:range <http://mdacc.org/ClinicalLatha#TherapeuticAgent> ;
      rdfs:subPropertyOf <http://mdacc.org/ClinicalLatha#administers> .

<http://mdacc.org/ClinicalLatha#amount>
      rdf:type owl:ObjectProperty .

<http://mdacc.org/ClinicalLatha#anaplasia>
      rdf:type owl:ObjectProperty ;
      rdfs:range <http://mdacc.org/ClinicalLatha#AnaplasiaFinding> .

<http://mdacc.org/ClinicalLatha#anatomicLocation>
      rdf:type owl:ObjectProperty ;
      rdfs:range <http://mdacc.org/ClinicalLatha#AnatomicSite> ;
      label:designNote "Relates the subject to an anatomic site."^^xsd:string ;
      dc:creator foaf:JimLomax ;
      owl:inverseOf <http://mdacc.org/ClinicalLatha#anatomicLocationOf> .

<http://mdacc.org/ClinicalLatha#anatomicLocationOf>
      rdf:type owl:ObjectProperty ;
      rdfs:domain <http://mdacc.org/ClinicalLatha#AnatomicSite> .

<http://mdacc.org/ClinicalLatha#appliedTo>
      rdf:type owl:ObjectProperty .

<http://mdacc.org/ClinicalLatha#birth>
      rdf:type owl:ObjectProperty ;
      rdfs:comment "Relates the subject to an existential birth; the birth occurred but no details are provided."^^xsd:string ;
      rdfs:range <http://mdacc.org/ClinicalLatha#BirthExistentialEvent> ;
      dc:creator foaf:JimLomax .

<http://mdacc.org/ClinicalLatha#birthDate>
      rdf:type owl:ObjectProperty ;
      rdfs:comment "Relates the subject to their date of birth"^^xsd:string ;
      rdfs:range temporal:BirthDateTime ;
      dc:creator foaf:JimLomax ;
      owl:inverseOf <http://mdacc.org/ClinicalLatha#birthDateOf> .

<http://mdacc.org/ClinicalLatha#birthDateOf>
      rdf:type owl:ObjectProperty .

<http://mdacc.org/ClinicalLatha#cancer>
      rdf:type owl:ObjectProperty ;
      rdfs:comment "Contingent on acceptance of Cancer into the ontology"^^xsd:string ;
      rdfs:range <http://mdacc.org/ClinicalLatha#Cancer> ;
      rdfs:subPropertyOf <http://mdacc.org/ClinicalLatha#disease> ;
      owl:inverseOf <http://mdacc.org/ClinicalLatha#cancerOf> .

<http://mdacc.org/ClinicalLatha#cancerId>
      rdf:type owl:ObjectProperty .

<http://mdacc.org/ClinicalLatha#cancerName>
      rdf:type owl:ObjectProperty ;
      rdfs:comment "Contingent on acceptance of Cancer into the ontology"^^xsd:string .

<http://mdacc.org/ClinicalLatha#cancerOf>
      rdf:type owl:ObjectProperty ;
      rdfs:comment "Contingent on acceptance of Cancer into the ontology"^^xsd:string ;
      rdfs:range <http://mdacc.org/ClinicalLatha#Cancer> .

<http://mdacc.org/ClinicalLatha#cellularDifferentiation>
      rdf:type owl:ObjectProperty ;
      rdfs:comment "The property creates a relationship between the subject, which detects/notes/observes an occurence of cellular differentiation of the object. The object in this case is scientifically determined to a Cell."^^xsd:string ;
      rdfs:range <http://mdacc.org/ClinicalLatha#Cell> ;
      dc:creator foaf:JimLomax .

<http://mdacc.org/ClinicalLatha#cellularOrigin>
      rdf:type owl:ObjectProperty .

<http://mdacc.org/ClinicalLatha#chemotherapyApplied>
      rdf:type owl:ObjectProperty ;
      rdfs:range <http://mdacc.org/ClinicalLatha#Chemotherapy> ;
      rdfs:subPropertyOf <http://mdacc.org/ClinicalLatha#therapyApplied> .

<http://mdacc.org/ClinicalLatha#code>
      rdf:type owl:DatatypeProperty ;
      rdfs:range rdfs:Literal .

<http://mdacc.org/ClinicalLatha#collectionSiteId>
      rdf:type owl:FunctionalProperty ;
      rdfs:subPropertyOf dc:identifier .

<http://mdacc.org/ClinicalLatha#composedOf>
      rdf:type owl:ObjectProperty ;
      owl:inverseOf <http://mdacc.org/ClinicalLatha#composes> .

<http://mdacc.org/ClinicalLatha#composes>
      rdf:type owl:ObjectProperty .

<http://mdacc.org/ClinicalLatha#compressionAlgorithmOf>
      rdf:type owl:ObjectProperty .

<http://mdacc.org/ClinicalLatha#concentration>
      rdf:type owl:ObjectProperty ;
      rdfs:range <http://mdacc.org/ClinicalLatha#Concentration> ;
      rdfs:subPropertyOf <http://mdacc.org/ClinicalLatha#amount> .

<http://mdacc.org/ClinicalLatha#currentWeight>
      rdf:type rdf:Property ;
      rdfs:range <http://mdacc.org/ClinicalLatha#Weight> ;
      rdfs:subPropertyOf <http://mdacc.org/ClinicalLatha#weight> ;
      dc:creator foaf:JimLomax .

<http://mdacc.org/ClinicalLatha#cy3LabelingProtocol1>
      rdf:type mage:Protocol .

<http://mdacc.org/ClinicalLatha#cy3LabelingTreatment1>
      rdf:type mage:Treatment .

<http://mdacc.org/ClinicalLatha#cy3PreWashProtocol1>
      rdf:type mage:Protocol .

<http://mdacc.org/ClinicalLatha#cy3PreWashTreatment1>
      rdf:type mage:Treatment .

<http://mdacc.org/ClinicalLatha#death>
      rdf:type owl:ObjectProperty ;
      rdfs:comment "Relates the subject to an existential death; death occurred but no details are provided."^^xsd:string ;
      rdfs:range <http://mdacc.org/ClinicalLatha#DeathExistentialEvent> ;
      dc:creator foaf:JimLomax .

<http://mdacc.org/ClinicalLatha#deathDate>
      rdf:type owl:ObjectProperty ;
      rdfs:comment "Relates the subject to their date of death."^^xsd:string ;
      rdfs:range temporal:DeathDateTime ;
      dc:creator foaf:JimLomax ;
      owl:inverseOf <http://mdacc.org/ClinicalLatha#deathDateOf> .

<http://mdacc.org/ClinicalLatha#deathDateOf>
      rdf:type owl:ObjectProperty ;
      label:creator foaf:JimLomax .

<http://mdacc.org/ClinicalLatha#descriptionOf>
      rdf:type rdf:Property .

<http://mdacc.org/ClinicalLatha#diagnosis>
      rdf:type owl:ObjectProperty ;
      rdfs:range <http://mdacc.org/ClinicalLatha#Diagnosis> ;
      label:creator foaf:JimLomax .

<http://mdacc.org/ClinicalLatha#disease>
      rdf:type owl:ObjectProperty ;
      rdfs:comment "Contingent on acceptance of Cancer into the ontology"^^xsd:string ;
      rdfs:range <http://mdacc.org/ClinicalLatha#Disease> ;
      owl:inverseOf <http://mdacc.org/ClinicalLatha#diseaseOf> .

<http://mdacc.org/ClinicalLatha#diseaseGrading>
      rdf:type owl:ObjectProperty ;
      rdfs:comment "comment placeholder"^^xsd:string ;
      dc:creator foaf:JimLomax .

<http://mdacc.org/ClinicalLatha#diseaseOf>
      rdf:type owl:ObjectProperty .

<http://mdacc.org/ClinicalLatha#diseaseScoringSystem>
      rdf:type owl:ObjectProperty ;
      rdfs:comment "Contingent on acceptance of Cancer into the ontology"^^xsd:string .

<http://mdacc.org/ClinicalLatha#diseaseStagingSystem>
      rdf:type rdf:Property ;
      rdfs:range <http://mdacc.org/ClinicalLatha#DiseaseStagingSystem> .

<http://mdacc.org/ClinicalLatha#dosage>
      rdf:type owl:ObjectProperty ;
      rdfs:range <http://mdacc.org/ClinicalLatha#Dosage> ;
      rdfs:subPropertyOf <http://mdacc.org/ClinicalLatha#amount> .

<http://mdacc.org/ClinicalLatha#emitsColor>
      rdf:type rdf:Property .

<http://mdacc.org/ClinicalLatha#eosinophilInfiltrationPercentage>
      rdf:type rdf:Property ;
      rdfs:subPropertyOf <http://mdacc.org/ClinicalLatha#percentage> ;
      dc:creator foaf:JimLomax .

<http://mdacc.org/ClinicalLatha#equipmentOf>
      rdf:type owl:ObjectProperty ;
      label:creator foaf:JimLomax .

<http://mdacc.org/ClinicalLatha#establishedBy>
      rdf:type owl:ObjectProperty .

<http://mdacc.org/ClinicalLatha#establishes>
      rdf:type owl:ObjectProperty ;
      rdfs:comment "Relates diagnostic procedure to the diagnosis it establishes"^^xsd:string ;
      rdfs:domain <http://mdacc.org/ClinicalLatha#DiagnosticProcedure> ;
      rdfs:range <http://mdacc.org/ClinicalLatha#Diagnosis> ;
      dc:creator foaf:JimLomax ;
      owl:inverseOf <http://mdacc.org/ClinicalLatha#establishedBy> .

<http://mdacc.org/ClinicalLatha#ethnicity>
      rdf:type owl:ObjectProperty ;
      rdfs:range <http://mdacc.org/ClinicalLatha#Ethnicity> ;
      rdfs:subPropertyOf <http://mdacc.org/ClinicalLatha#populationCharacteristic> ;
      label:designNote "Relates the subject to a ethnicity."^^xsd:string ;
      dc:creator foaf:JimLomax ;
      owl:inverseOf <http://mdacc.org/ClinicalLatha#ethnicityOf> .

<http://mdacc.org/ClinicalLatha#ethnicityOf>
      rdf:type owl:ObjectProperty ;
      rdfs:subPropertyOf <http://mdacc.org/ClinicalLatha#populationCharacteristicOf> .

<http://mdacc.org/ClinicalLatha#examinationApplied>
      rdf:type owl:ObjectProperty .

<http://mdacc.org/ClinicalLatha#examinationId>
      rdf:type owl:FunctionalProperty ;
      rdfs:subPropertyOf dc:identifier .

<http://mdacc.org/ClinicalLatha#examinationIdOf>
      rdf:type owl:ObjectProperty .

<http://mdacc.org/ClinicalLatha#exhibitsMorphology>
      rdf:type owl:ObjectProperty ;
      rdfs:comment "The subject exhibits a morphology, a structure and/or composition,  resembling the predicate. In a biological context this means that the subjects resembles the object in terms of its biological structure and composition."^^xsd:string ;
      dc:creator foaf:JimLomax .

<http://mdacc.org/ClinicalLatha#exhibitsTumorMorphology>
      rdf:type owl:ObjectProperty ;
      rdfs:comment "The diomain exhibits structural or compositional similarities to the range, which is a tumor."^^xsd:string ;
      rdfs:range <http://mdacc.org/ClinicalLatha#TumorType> ;
      rdfs:subPropertyOf <http://mdacc.org/ClinicalLatha#exhibitsMorphology> ;
      dc:creator foaf:JimLomax .

<http://mdacc.org/ClinicalLatha#finding>
      rdf:type owl:ObjectProperty ;
      rdfs:range <http://mdacc.org/ClinicalLatha#Finding> .

<http://mdacc.org/ClinicalLatha#followUpDate>
      rdf:type owl:ObjectProperty ;
      rdfs:comment "Relates the subject to a followup appointment date."^^xsd:string ;
      rdfs:range temporal:FollowUpDateTime ;
      dc:creator foaf:JimLomax ;
      owl:inverseOf <http://mdacc.org/ClinicalLatha#followUpDateOf> .

<http://mdacc.org/ClinicalLatha#followUpDateOf>
      rdf:type owl:ObjectProperty ;
      label:creator foaf:JimLomax .

<http://mdacc.org/ClinicalLatha#fractions>
      rdf:type owl:DatatypeProperty ;
      rdfs:range xsd:integer .

<http://mdacc.org/ClinicalLatha#gemistocytePresent>
      rdf:type owl:DatatypeProperty ;
      rdfs:domain sample:GBMTumorPathology ;
      rdfs:range xsd:boolean .

<http://mdacc.org/ClinicalLatha#gender>
      rdf:type owl:ObjectProperty ;
      rdfs:range <http://mdacc.org/ClinicalLatha#Gender> ;
      label:designNote "Relates the subject to a gender."^^xsd:string ;
      dc:creator foaf:JimLomax ;
      owl:inverseOf <http://mdacc.org/ClinicalLatha#genderOf> .

<http://mdacc.org/ClinicalLatha#genderOf>
      rdf:type owl:ObjectProperty .

<http://mdacc.org/ClinicalLatha#granulocyteInfiltrationPercentage>
      rdf:type rdf:Property ;
      rdfs:subPropertyOf <http://mdacc.org/ClinicalLatha#percentage> ;
      dc:creator foaf:JimLomax .

<http://mdacc.org/ClinicalLatha#hadCancer>
      rdf:type owl:DatatypeProperty ;
      label:designNote "Relates the subject to an boolean indicating if the subject had been diagnosed with cancer at one time and that the cancer previously diagnosed went into remission. This does not preclude that the subject has cancer currently."^^xsd:string ;
      dc:creator foaf:JimLomax .

<http://mdacc.org/ClinicalLatha#hasAccessionNumber>
      rdf:type owl:ObjectProperty ;
      rdfs:subPropertyOf <http://mdacc.org/ClinicalLatha#hasGenomicSequenceId> ;
      owl:inverseOf <http://mdacc.org/ClinicalLatha#accessionNumberOf> .

<http://mdacc.org/ClinicalLatha#hasArchiveVersion>
      rdf:type owl:ObjectProperty ;
      rdfs:subPropertyOf mage:has_version .

<http://mdacc.org/ClinicalLatha#hasCpgSiteId>
      rdf:type owl:ObjectProperty ;
      rdfs:subPropertyOf dc:identifier .

<http://mdacc.org/ClinicalLatha#hasGenomicSequenceId>
      rdf:type owl:ObjectProperty ;
      rdfs:subPropertyOf dc:identifier .

<http://mdacc.org/ClinicalLatha#hasPatientId>
      rdf:type owl:FunctionalProperty ;
      rdfs:subPropertyOf dc:identifier ;
      dc:creator foaf:JimLomax .

<http://mdacc.org/ClinicalLatha#has_platform_version>
      rdf:type owl:ObjectProperty ;
      rdfs:subPropertyOf mage:has_version .

<http://mdacc.org/ClinicalLatha#ietfTag>
      rdf:type rdf:Property ;
      rdfs:subPropertyOf dc:identifier .

<http://mdacc.org/ClinicalLatha#immortalizingAgent>
      rdf:type owl:ObjectProperty .

<http://mdacc.org/ClinicalLatha#indicates>
      rdf:type owl:ObjectProperty ;
      rdfs:comment "The subject indicates the presence of the object. Example: A Diagnosis indicates the presence of (disease,condition, injury)."^^xsd:string ;
      label:creator foaf:JimLomax .

<http://mdacc.org/ClinicalLatha#indicator>
      rdf:type owl:ObjectProperty ;
      rdfs:range <http://mdacc.org/ClinicalLatha#Indicator> ;
      label:creator foaf:JimLomax .

<http://mdacc.org/ClinicalLatha#inflammationInfiltrationPercentage>
      rdf:type rdf:Property ;
      rdfs:subPropertyOf <http://mdacc.org/ClinicalLatha#percentage> ;
      dc:creator foaf:JimLomax .

<http://mdacc.org/ClinicalLatha#informedConsentVerfied>
      rdf:type owl:ObjectProperty ;
      rdfs:range <http://mdacc.org/ClinicalLatha#PreTreatmentHistoryExistentialEvent> ;
      label:designNote "Relates the subject to an indication of whether or not a pretreatment history exists for the subject"^^xsd:string ;
      dc:creator foaf:JimLomax .

<http://mdacc.org/ClinicalLatha#initialCourse>
      rdf:type owl:ObjectProperty ;
      rdfs:range <http://mdacc.org/ClinicalLatha#InitialCourseExistentialEvent> ;
      dc:creator foaf:JimLomax .

<http://mdacc.org/ClinicalLatha#initialDiagnosis>
      rdf:type owl:ObjectProperty ;
      rdfs:subPropertyOf <http://mdacc.org/ClinicalLatha#diagnosis> ;
      label:creator foaf:JimLomax .

<http://mdacc.org/ClinicalLatha#initialWeight>
      rdf:type rdf:Property ;
      rdfs:range <http://mdacc.org/ClinicalLatha#Weight> ;
      rdfs:subPropertyOf <http://mdacc.org/ClinicalLatha#weight> ;
      dc:creator foaf:JimLomax .

<http://mdacc.org/ClinicalLatha#labProcedure>
      rdf:type owl:ObjectProperty ;
      rdfs:range <http://mdacc.org/ClinicalLatha#LabProcedure> .

<http://mdacc.org/ClinicalLatha#leptomeningialInvolvement>
      rdf:type owl:DatatypeProperty ;
      rdfs:domain sample:GBMTumorPathology ;
      rdfs:range xsd:boolean .

<http://mdacc.org/ClinicalLatha#lymphaticInvasion>
      rdf:type owl:DatatypeProperty ;
      rdfs:range xsd:boolean .

<http://mdacc.org/ClinicalLatha#lymphocyteInfiltrationPercentage>
      rdf:type rdf:Property ;
      rdfs:subPropertyOf <http://mdacc.org/ClinicalLatha#percentage> ;
      dc:creator foaf:JimLomax .

<http://mdacc.org/ClinicalLatha#mRNA>
      rdf:type owl:Class ;
      rdfs:comment "mRNA, messenger RNA, is a molecule of RNA encoding a chemical \"blueprint\" for a protein product. mRNA is transcribed from a DNA template, and carries coding information to the sites of protein synthesis: the ribosomes."^^xsd:string ;
      rdfs:subClassOf <http://mdacc.org/ClinicalLatha#RNA> ;
      label:correspondsTo label:mRNA_NCIURI ;
      label:designNote "This concept is directly related to the mRNA concept in NCI Thesaurus."^^xsd:string , "This concept may have instances of it's own or may be a superclass for concept refinements."^^xsd:string ;
      dc:creator foaf:JimLomax .

<http://mdacc.org/ClinicalLatha#manifestedBy>
      rdf:type owl:ObjectProperty .

<http://mdacc.org/ClinicalLatha#manifests>
      rdf:type owl:ObjectProperty ;
      owl:inverseOf <http://mdacc.org/ClinicalLatha#manifestedBy> .

<http://mdacc.org/ClinicalLatha#marginsInvolved>
      rdf:type owl:DatatypeProperty ;
      rdfs:range xsd:boolean .

<http://mdacc.org/ClinicalLatha#measurement>
      rdf:type rdf:Property .

<http://mdacc.org/ClinicalLatha#metastaticIndication>
      rdf:type owl:ObjectProperty ;
      rdfs:range <http://mdacc.org/ClinicalLatha#MetastaticIndication> .

<http://mdacc.org/ClinicalLatha#monocyteInfiltrationPercentage>
      rdf:type rdf:Property ;
      rdfs:subPropertyOf <http://mdacc.org/ClinicalLatha#percentage> ;
      dc:creator foaf:JimLomax .

<http://mdacc.org/ClinicalLatha#necrosisPercentage>
      rdf:type rdf:Property ;
      rdfs:subPropertyOf <http://mdacc.org/ClinicalLatha#percentage> ;
      dc:creator foaf:JimLomax .

<http://mdacc.org/ClinicalLatha#neutrophilInfiltrationPercentage>
      rdf:type rdf:Property ;
      rdfs:subPropertyOf <http://mdacc.org/ClinicalLatha#percentage> ;
      dc:creator foaf:JimLomax .

<http://mdacc.org/ClinicalLatha#normalCellsPercentage>
      rdf:type rdf:Property ;
      rdfs:subPropertyOf <http://mdacc.org/ClinicalLatha#percentage> ;
      dc:creator foaf:JimLomax .

<http://mdacc.org/ClinicalLatha#nuclearGrade>
      rdf:type owl:ObjectProperty ;
      rdfs:comment "Contingent on acceptance of Cancer into the ontology"^^xsd:string ;
      rdfs:range <http://mdacc.org/ClinicalLatha#NuclearGrade> ;
      rdfs:subPropertyOf <http://mdacc.org/ClinicalLatha#diseaseScoringSystem> .

<http://mdacc.org/ClinicalLatha#numberOfCycles>
      rdf:type owl:DatatypeProperty ;
      rdfs:range xsd:integer .

<http://mdacc.org/ClinicalLatha#numberOfRegionalLymphNodesExamined>
      rdf:type owl:DatatypeProperty ;
      rdfs:range xsd:integer .

<http://mdacc.org/ClinicalLatha#numberOfRegionalLymphNodesExaminedPositive>
      rdf:type owl:DatatypeProperty ;
      rdfs:range xsd:integer .

<http://mdacc.org/ClinicalLatha#numberProliferatingCells>
      rdf:type owl:DatatypeProperty ;
      rdfs:range xsd:integer .

<http://mdacc.org/ClinicalLatha#observationOf>
      rdf:type owl:ObjectProperty .

<http://mdacc.org/ClinicalLatha#occurred>
      rdf:type owl:DatatypeProperty ;
      rdfs:domain <http://mdacc.org/ClinicalLatha#ExistentialEvent> ;
      rdfs:range xsd:boolean ;
      label:designNote "Relates the subject to a boolean value indicating whether or not the subject occurred."^^xsd:string ;
      dc:creator foaf:JimLomax .

<http://mdacc.org/ClinicalLatha#oligodendroglialComponent>
      rdf:type owl:DatatypeProperty ;
      rdfs:domain sample:GBMTumorPathology ;
      rdfs:range xsd:boolean .

<http://mdacc.org/ClinicalLatha#ongoing>
      rdf:type owl:DatatypeProperty ;
      rdfs:range xsd:boolean .

<http://mdacc.org/ClinicalLatha#outcome>
      rdf:type owl:ObjectProperty ;
      rdfs:range <http://mdacc.org/ClinicalLatha#Outcome> ;
      owl:inverseOf <http://mdacc.org/ClinicalLatha#outcomeOf> .

<http://mdacc.org/ClinicalLatha#outcomeOf>
      rdf:type owl:ObjectProperty .

<http://mdacc.org/ClinicalLatha#patient>
      rdf:type owl:ObjectProperty ;
      rdfs:comment "Contingent on the acceptance of the Patient class into the ontology"^^xsd:string ;
      rdfs:range <http://mdacc.org/ClinicalLatha#Patient> ;
      owl:inverseOf <http://mdacc.org/ClinicalLatha#patientOf> .

<http://mdacc.org/ClinicalLatha#patientId>
      rdf:type owl:FunctionalProperty ;
      rdfs:range <http://mdacc.org/ClinicalLatha#PatientId> ;
      rdfs:subPropertyOf dc:identifier ;
      label:creator foaf:JimLomax ;
      label:designNote "A subject can only have one patient id to maintain patientId uniqueness."^^xsd:string ;
      owl:inverseOf <http://mdacc.org/ClinicalLatha#patientIdOf> .

<http://mdacc.org/ClinicalLatha#patientIdOf>
      rdf:type owl:ObjectProperty ;
      label:creator foaf:JimLomax .

<http://mdacc.org/ClinicalLatha#patientOf>
      rdf:type owl:ObjectProperty .

<http://mdacc.org/ClinicalLatha#percentEosinophilInfiltration>
      rdf:type owl:DatatypeProperty ;
      rdfs:range xsd:float .

<http://mdacc.org/ClinicalLatha#percentGranulocyteInfiltration>
      rdf:type owl:DatatypeProperty ;
      rdfs:range xsd:float .

<http://mdacc.org/ClinicalLatha#percentInflammationInfiltration>
      rdf:type owl:DatatypeProperty ;
      rdfs:range xsd:float .

<http://mdacc.org/ClinicalLatha#percentLymphocyteInfiltration>
      rdf:type owl:DatatypeProperty ;
      rdfs:range xsd:float .

<http://mdacc.org/ClinicalLatha#percentMonocyteInfiltration>
      rdf:type owl:DatatypeProperty ;
      rdfs:range xsd:float .

<http://mdacc.org/ClinicalLatha#percentNecrosis>
      rdf:type owl:DatatypeProperty ;
      rdfs:range xsd:float .

<http://mdacc.org/ClinicalLatha#percentNeutrophilInfiltration>
      rdf:type owl:DatatypeProperty ;
      rdfs:range xsd:float .

<http://mdacc.org/ClinicalLatha#percentNormalCells>
      rdf:type owl:DatatypeProperty ;
      rdfs:range xsd:float .

<http://mdacc.org/ClinicalLatha#percentTumorCells>
      rdf:type owl:DatatypeProperty ;
      rdfs:range xsd:float .

<http://mdacc.org/ClinicalLatha#percentTumorNuclei>
      rdf:type owl:DatatypeProperty ;
      rdfs:range xsd:float .

<http://mdacc.org/ClinicalLatha#percentage>
      rdf:type rdf:Property ;
      rdfs:subPropertyOf <http://mdacc.org/ClinicalLatha#quantity> .

<http://mdacc.org/ClinicalLatha#platformIdentifier>
      rdf:type owl:FunctionalProperty ;
      rdfs:subPropertyOf dc:identifier .

<http://mdacc.org/ClinicalLatha#populationCharacteristic>
      rdf:type owl:ObjectProperty ;
      rdfs:range <http://mdacc.org/ClinicalLatha#PopulationCharacteristic> ;
      label:designNote "Relates the subject to a population characteristic."^^xsd:string ;
      dc:creator foaf:JimLomax ;
      owl:inverseOf <http://mdacc.org/ClinicalLatha#populationCharacteristicOf> .

<http://mdacc.org/ClinicalLatha#populationCharacteristicOf>
      rdf:type owl:ObjectProperty .

<http://mdacc.org/ClinicalLatha#preTreatmentHistoryExists>
      rdf:type owl:ObjectProperty ;
      rdfs:range <http://mdacc.org/ClinicalLatha#PreTreatmentHistoryExistentialEvent> ;
      label:designNote "Relates the subject to an indication of whether or not a pretreatment history exists for the subject"^^xsd:string ;
      dc:creator foaf:JimLomax .

<http://mdacc.org/ClinicalLatha#proliferatingCellsQuantity>
      rdf:type rdf:Property ;
      rdfs:subPropertyOf <http://mdacc.org/ClinicalLatha#quantity> ;
      dc:creator foaf:JimLomax .

<http://mdacc.org/ClinicalLatha#protocol>
      rdf:type owl:ObjectProperty ;
      rdfs:range <http://mdacc.org/ClinicalLatha#Protocol> .

<http://mdacc.org/ClinicalLatha#protocolType>
      rdf:type owl:ObjectProperty ;
      rdfs:range <http://mdacc.org/ClinicalLatha#ProtocolType> .

<http://mdacc.org/ClinicalLatha#purityMeasurement>
      rdf:type rdf:Property ;
      rdfs:range <http://mdacc.org/ClinicalLatha#PurityMeasurment> ;
      rdfs:subPropertyOf <http://mdacc.org/ClinicalLatha#quantity> ;
      label:creator foaf:JimLomax .

<http://mdacc.org/ClinicalLatha#quantity>
      rdf:type rdf:Property ;
      rdfs:comment "The quantity property related a subject with literal value interpreted as its quantity according to some unit of measurement."^^xsd:string ;
      dc:creator foaf:JimLomax .

<http://mdacc.org/ClinicalLatha#rRNA>
      rdf:type owl:Class ;
      rdfs:comment "rRNA, ribosomal RNA,  is the RNA component of the ribosome, the protein manufacturing machinery of all living cells. Ribosomal RNA provides a mechanism for decoding mRNA into amino acids and interacts with tRNAs during translation by providing peptidyl transferase activity"^^xsd:string ;
      rdfs:subClassOf <http://mdacc.org/ClinicalLatha#RNA> ;
      label:correspondsTo label:rRNA_NCIURI ;
      label:designNote "This concept is directly related to the rRNA concept in NCI Thesaurus."^^xsd:string , "This concept may have instances of it's own or may be a superclass for concept refinements."^^xsd:string ;
      dc:creator foaf:JimLomax .

<http://mdacc.org/ClinicalLatha#race>
      rdf:type owl:ObjectProperty ;
      rdfs:range <http://mdacc.org/ClinicalLatha#Race> ;
      label:designNote "Relates the subject to a race."^^xsd:string ;
      dc:creator foaf:JimLomax ;
      owl:inverseOf <http://mdacc.org/ClinicalLatha#raceOf> .

<http://mdacc.org/ClinicalLatha#raceOf>
      rdf:type owl:ObjectProperty .

<http://mdacc.org/ClinicalLatha#radiationTherapyExists>
      rdf:type owl:ObjectProperty ;
      rdfs:range <http://mdacc.org/ClinicalLatha#RadiationTherapyExistentialEvent> ;
      label:designNote "Relates the subject to an indication of whether or not a radiation therapy  has been given to subject; no details of the radiation treatment are noted."^^xsd:string ;
      dc:creator foaf:JimLomax .

<http://mdacc.org/ClinicalLatha#regimen>
      rdf:type owl:ObjectProperty ;
      owl:inverseOf <http://mdacc.org/ClinicalLatha#regimenOf> .

<http://mdacc.org/ClinicalLatha#regimenModel>
      rdf:type owl:ObjectProperty ;
      rdfs:range <http://mdacc.org/ClinicalLatha#RegimenModel> ;
      owl:inverseOf <http://mdacc.org/ClinicalLatha#regimenModelOf> .

<http://mdacc.org/ClinicalLatha#regimenModelOf>
      rdf:type owl:ObjectProperty .

<http://mdacc.org/ClinicalLatha#regimenOf>
      rdf:type owl:ObjectProperty ;
      rdfs:domain <http://mdacc.org/ClinicalLatha#Regimen> .

<http://mdacc.org/ClinicalLatha#requiresEquipment>
      rdf:type owl:ObjectProperty ;
      rdfs:comment "The subject requires the object equipment for some reason; to function, to achieve its goal, etc."^^xsd:string ;
      rdfs:range <http://mdacc.org/ClinicalLatha#Equipment> ;
      label:creator foaf:JimLomax ;
      owl:inverseOf <http://mdacc.org/ClinicalLatha#equipmentOf> .

<http://mdacc.org/ClinicalLatha#sectionLocation>
      rdf:type owl:ObjectProperty ;
      rdfs:subPropertyOf <http://mdacc.org/ClinicalLatha#side> .

<http://mdacc.org/ClinicalLatha#side>
      rdf:type owl:ObjectProperty ;
      rdfs:comment "Locates the subject based on a fixed set of sides (left, right) (east, west, north, south)"^^xsd:string ;
      rdfs:range <http://mdacc.org/ClinicalLatha#Side> ;
      rdfs:subPropertyOf <http://mdacc.org/ClinicalLatha#spatiallyLocatedBy> .

<http://mdacc.org/ClinicalLatha#slide>
      rdf:type owl:ObjectProperty ;
      rdfs:range <http://mdacc.org/ClinicalLatha#Slide> .

<http://mdacc.org/ClinicalLatha#spatiallyLocatedBy>
      rdf:type owl:ObjectProperty ;
      rdfs:comment "Locates the subject based on a fixed set of sides (left, right) (east, west, north, south)"^^xsd:string ;
      rdfs:range <http://mdacc.org/ClinicalLatha#Side> .

<http://mdacc.org/ClinicalLatha#specifier>
      rdf:type rdf:Property ;
      rdfs:range foaf:Agent .

<http://mdacc.org/ClinicalLatha#stage>
      rdf:type owl:ObjectProperty ;
      rdfs:comment "The subject is attribute with a stage of progression; currently this is specific to domain TissueSample and range TumorStage"^^xsd:string ;
      rdfs:domain sample:TissueSample ;
      rdfs:range <http://mdacc.org/ClinicalLatha#TumorStage> ;
      label:creator foaf:JimLomax ;
      owl:inverseOf <http://mdacc.org/ClinicalLatha#stageOf> .

<http://mdacc.org/ClinicalLatha#stageOf>
      rdf:type owl:ObjectProperty .

<http://mdacc.org/ClinicalLatha#tRNA>
      rdf:type owl:Class ;
      rdfs:comment "tRNA, transfer RNA,  is a small RNA molecule  that transfers a specific active amino acid to a growing polypeptide chain at the ribosomal site of protein synthesis during translation"^^xsd:string ;
      rdfs:subClassOf <http://mdacc.org/ClinicalLatha#RNA> ;
      label:correspondsTo label:tRNA_NCIURI ;
      label:designNote "This concept is directly related to the tRNA concept in NCI Thesaurus."^^xsd:string , "This concept may have instances of it's own or may be a superclass for concept refinements."^^xsd:string ;
      dc:creator foaf:JimLomax .

<http://mdacc.org/ClinicalLatha#therapeuticDelivery>
      rdf:type owl:ObjectProperty ;
      rdfs:range <http://mdacc.org/ClinicalLatha#TherapeuticAgentDelivery> .

<http://mdacc.org/ClinicalLatha#therapeuticProcedure>
      rdf:type owl:ObjectProperty ;
      rdfs:range <http://mdacc.org/ClinicalLatha#TherapeuticProcedure> .

<http://mdacc.org/ClinicalLatha#therapeuticProcedures>
      rdf:type owl:ObjectProperty ;
      rdfs:range collections:Collection .

<http://mdacc.org/ClinicalLatha#therapyApplied>
      rdf:type owl:ObjectProperty ;
      rdfs:range <http://mdacc.org/ClinicalLatha#TherapeuticProcedure> ;
      owl:inverseOf <http://mdacc.org/ClinicalLatha#therapyAppliedTo> .

<http://mdacc.org/ClinicalLatha#therapyAppliedTo>
      rdf:type owl:ObjectProperty .

<http://mdacc.org/ClinicalLatha#tnmScheme>
      rdf:type rdf:Property ;
      rdfs:range <http://mdacc.org/ClinicalLatha#TNMDiseaseStagingSystem> .

<http://mdacc.org/ClinicalLatha#transformationOf>
      rdf:type owl:ObjectProperty .

<http://mdacc.org/ClinicalLatha#transformedBy>
      rdf:type owl:ObjectProperty ;
      owl:inverseOf <http://mdacc.org/ClinicalLatha#transformationOf> .

<http://mdacc.org/ClinicalLatha#treatedWith>
      rdf:type owl:ObjectProperty ;
      rdfs:range <http://mdacc.org/ClinicalLatha#TherapeuticProcedure> ;
      owl:inverseOf <http://mdacc.org/ClinicalLatha#appliedTo> .

<http://mdacc.org/ClinicalLatha#treatmentEventExists>
      rdf:type owl:ObjectProperty ;
      rdfs:comment "Relates the subject to an existential treatment (therapeutic procedure). The treatment was applied to the subject but no details were collected."^^xsd:string ;
      rdfs:range <http://mdacc.org/ClinicalLatha#TherapeuticProcedureExistentialEvent> ;
      label:creator foaf:JimLomax .

<http://mdacc.org/ClinicalLatha#treatmentSite>
      rdf:type owl:DatatypeProperty ;
      rdfs:range xsd:string .

<http://mdacc.org/ClinicalLatha#tumorCellsPercentage>
      rdf:type rdf:Property ;
      rdfs:subPropertyOf <http://mdacc.org/ClinicalLatha#percentage> ;
      dc:creator foaf:JimLomax .

<http://mdacc.org/ClinicalLatha#tumorClassification>
      rdf:type owl:ObjectProperty ;
      rdfs:range <http://mdacc.org/ClinicalLatha#TumorType> .

<http://mdacc.org/ClinicalLatha#tumorNucleiPercentage>
      rdf:type rdf:Property ;
      rdfs:subPropertyOf <http://mdacc.org/ClinicalLatha#percentage> ;
      dc:creator foaf:JimLomax .

<http://mdacc.org/ClinicalLatha#tumorOrigin>
      rdf:type owl:ObjectProperty ;
      rdfs:range <http://mdacc.org/ClinicalLatha#TumorType> .

<http://mdacc.org/ClinicalLatha#units>
      rdf:type owl:ObjectProperty ;
      rdfs:range <http://mdacc.org/ClinicalLatha#Units> .

<http://mdacc.org/ClinicalLatha#value>
      rdf:type owl:DatatypeProperty .

<http://mdacc.org/ClinicalLatha#venousInvasion>
      rdf:type owl:DatatypeProperty ;
      rdfs:range xsd:boolean .

<http://mdacc.org/ClinicalLatha#vitalStatus>
      rdf:type owl:ObjectProperty ;
      rdfs:range <http://mdacc.org/ClinicalLatha#VitalStatus> ;
      label:designNote "Relates the subject to a vital status."^^xsd:string ;
      dc:creator foaf:JimLomax .

<http://mdacc.org/ClinicalLatha#volume>
      rdf:type owl:ObjectProperty ;
      rdfs:range <http://mdacc.org/ClinicalLatha#Volume> ;
      rdfs:subPropertyOf <http://mdacc.org/ClinicalLatha#amount> .

<http://mdacc.org/ClinicalLatha#weight>
      rdf:type rdf:Property ;
      rdfs:range <http://mdacc.org/ClinicalLatha#Weight> ;
      rdfs:subPropertyOf <http://mdacc.org/ClinicalLatha#quantity> ;
      dc:creator foaf:JimLomax .

<http://mdacc.org/Drug#Example_ChemotherapyDrug>
      skos-xl:prefLabel label:Tamoxifen_ChemotherapyDrugLabel .

<http://mdacc.org/Drug#Radiation>
      rdf:type owl:Class ;
      rdfs:subClassOf <http://mdacc.org/ClinicalLatha#TherapeuticAgent> .

label:correspondsTo
      rdf:type owl:ObjectProperty ;
      rdfs:range label:URI .

organization:biologicalCollectionResource
      rdf:type owl:ObjectProperty ;
      rdfs:range organization:BiologicalCollectionResource .

sample:Patient1_PatientId
      dc:identifier "PatientId1"^^xsd:string .

sample:Patient2_PatientId
      dc:identifier "PatientId2"^^xsd:string .

tcga:10ml_AliquotAmount
      <http://mdacc.org/ClinicalLatha#quantity>
              "10"^^xsd:string .

dc:approvedDate
      rdf:type owl:AnnotationProperty ;
      rdfs:subPropertyOf dc:date .

dc:creator
      rdfs:range foaf:Person .

time-entry:TemporalThing
      rdf:type owl:Class ;
      rdfs:label "Temporal thing"^^xsd:string ;
      rdfs:subClassOf temporal:TemporalPackage .

time-entry:TemporalUnit
      rdf:type owl:Class ;
      rdfs:label "Temporal unit"^^xsd:string ;
      rdfs:subClassOf temporal:TemporalPackage .

<http://www.isi.edu/~pan/damltime/timezone-ont.owl#TimeZone>
      rdf:type owl:Class ;
      rdfs:label "Time zone"^^xsd:string ;
      rdfs:subClassOf temporal:TemporalPackage .

nco:Affiliation_1
      rdf:type nco:Affiliation .

foaf:DawitGebremichael
      rdf:type foaf:Person .

foaf:JimLomax
      rdf:type foaf:Person ;
      foaf:firstName "Jim"^^xsd:string ;
      foaf:surname "Lomax"^^xsd:string .

foaf:LathaRamdas
      rdf:type foaf:Person ;
      foaf:family_name "Ramdas"^^xsd:string ;
      foaf:firstName "Latha"^^xsd:string .

foaf:MoSanyang
      rdf:type foaf:Person ;
      foaf:family_name "Sanyang"^^xsd:string ;
      foaf:firstName "Mo"^^xsd:string .

foaf:ParsaMirhaji
      rdf:type foaf:Person .

foaf:PradheepRaju
      rdf:type foaf:Person .
